@prefix : <http://purl.allotrope.org/voc/adf/REC/2019/06/hdf#> .
@prefix dc: <http://purl.org/dc/elements/1.1/> .
@prefix dct: <http://purl.org/dc/terms/> .
@prefix hdf: <http://purl.allotrope.org/ontologies/hdf5/1.8#> .
@prefix owl: <http://www.w3.org/2002/07/owl#> .
@prefix rdf: <http://www.w3.org/1999/02/22-rdf-syntax-ns#> .
@prefix xml: <http://www.w3.org/XML/1998/namespace> .
@prefix xsd: <http://www.w3.org/2001/XMLSchema#> .
@prefix prov: <http://www.w3.org/ns/prov#> .
@prefix rdfs: <http://www.w3.org/2000/01/rdf-schema#> .
@prefix skos: <http://www.w3.org/2004/02/skos/core#> .
@base <http://purl.allotrope.org/voc/adf/REC/2019/06/hdf#> .

<http://purl.allotrope.org/voc/adf/REC/2024/12/hdf> rdf:type owl:Ontology ;
                                                     owl:versionIRI <http://purl.allotrope.org/voc/adf/REC/2024/12/hdf> ;
                                                     dc:title "The HDF5 data description ontology. (REC/2024/12)" ;
                                                     dct:contributor <http://www.allotrope.org> ;
                                                     dct:description """This ontology is based on the HDF5 specification.
Sources are the DDL file and the HDF5 User's and Reference Guide.""" ;
                                                     dct:issued "2024-12-18T12:00:00Z"^^xsd:dateTime ;
                                                     dct:license <http://purl.allotrope.org/voc/creative-commons-attribution-license> ,
                                                                 <http://purl.allotrope.org/voc/hdf-license> ;
                                                     dct:modified "2024-12-08T12:00:00Z"^^xsd:dateTime ;
                                                     dct:publisher <http://www.allotrope.org> ;
                                                     dct:rights <http://purl.allotrope.org/voc/attribution> ,
                                                                <http://purl.allotrope.org/voc/copyright> ,
                                                                <http://purl.allotrope.org/voc/hdf-copyright> ;
                                                     dct:source <https://support.hdfgroup.org/HDF5/doc/ddl.html> ,
                                                                <https://support.hdfgroup.org/HDF5/doc/RM/RM_H5Front.html> ,
                                                                <https://support.hdfgroup.org/HDF5/doc/UG/HDF5_Users_Guide-Responsive%20HTML5/index.html> ;
                                                     owl:priorVersion <http://purl.allotrope.org/voc/adf/REC/2020/06/hdf> ;
                                                     owl:versionInfo "REC/2024/12" ;
                                                     prov:wasDerivedFrom <https://support.hdfgroup.org/HDF5/doc/ddl.html> ,
                                                                         <https://support.hdfgroup.org/HDF5/doc/RM/RM_H5Front.html> ,
                                                                         <https://support.hdfgroup.org/HDF5/doc/UG/HDF5_Users_Guide-Responsive%20HTML5/index.html> .

#################################################################
#    Annotation properties
#################################################################

###  http://purl.org/dc/elements/1.1/title
dc:title rdf:type owl:AnnotationProperty .


###  http://purl.org/dc/terms/contributor
dct:contributor rdf:type owl:AnnotationProperty .


###  http://purl.org/dc/terms/description
dct:description rdf:type owl:AnnotationProperty .


###  http://purl.org/dc/terms/issued
dct:issued rdf:type owl:AnnotationProperty .


###  http://purl.org/dc/terms/license
dct:license rdf:type owl:AnnotationProperty .


###  http://purl.org/dc/terms/modified
dct:modified rdf:type owl:AnnotationProperty .


###  http://purl.org/dc/terms/publisher
dct:publisher rdf:type owl:AnnotationProperty .


###  http://purl.org/dc/terms/rights
dct:rights rdf:type owl:AnnotationProperty .


###  http://purl.org/dc/terms/rightsHolder
dct:rightsHolder rdf:type owl:AnnotationProperty .


###  http://purl.org/dc/terms/source
dct:source rdf:type owl:AnnotationProperty .


###  http://purl.org/dc/terms/title
dct:title rdf:type owl:AnnotationProperty .


###  http://www.w3.org/2001/XMLSchema#maxInclusive
xsd:maxInclusive rdf:type owl:AnnotationProperty .


###  http://www.w3.org/2001/XMLSchema#minInclusive
xsd:minInclusive rdf:type owl:AnnotationProperty .


###  http://www.w3.org/2004/02/skos/core#altLabel
skos:altLabel rdf:type owl:AnnotationProperty .


###  http://www.w3.org/2004/02/skos/core#definition
skos:definition rdf:type owl:AnnotationProperty .


###  http://www.w3.org/2004/02/skos/core#note
skos:note rdf:type owl:AnnotationProperty .


###  http://www.w3.org/2004/02/skos/core#prefLabel
skos:prefLabel rdf:type owl:AnnotationProperty .


###  http://www.w3.org/ns/prov#wasDerivedFrom
prov:wasDerivedFrom rdf:type owl:AnnotationProperty .


#################################################################
#    Datatypes
#################################################################

###  http://purl.allotrope.org/ontologies/hdf5/1.8#DimensionIndexType
hdf:DimensionIndexType rdf:type rdfs:Datatype ;
                       rdfs:comment "xsd:int based datatype restricted to the range of 0 to 31. Used for indexing dimensions. [Allotrope]" ;
                       rdfs:label "dimension index type" ;
                       skos:definition "xsd:int based datatype restricted to the range of 0 to 31. Used for indexing dimensions. [Allotrope]" ;
                       skos:prefLabel "dimension index type" ;
                       owl:equivalentClass [ rdf:type rdfs:Datatype ;
                                             owl:onDatatype xsd:int ;
                                             owl:withRestrictions ( [ xsd:minInclusive "0"^^xsd:int
                                                                    ]
                                                                    [ xsd:maxInclusive "31"^^xsd:int
                                                                    ]
                                                                  )
                                           ] .


###  http://purl.allotrope.org/ontologies/hdf5/1.8#IndexType
hdf:IndexType rdf:type rdfs:Datatype ;
              rdfs:comment "Non-negative xsd:long datatype. Used to address a point per dimension. [Allotrope]" ;
              rdfs:label "index type" ;
              skos:definition "Non-negative xsd:long datatype. Used to address a point per dimension. [Allotrope]" ;
              skos:prefLabel "index type" ;
              owl:equivalentClass [ rdf:type rdfs:Datatype ;
                                    owl:onDatatype xsd:long ;
                                    owl:withRestrictions ( [ xsd:minInclusive "0"^^xsd:long
                                                           ]
                                                         )
                                  ] .


###  http://www.w3.org/1999/02/22-rdf-syntax-ns#Literal
rdf:Literal rdf:type rdfs:Datatype .


#################################################################
#    Object Properties
#################################################################

###  http://purl.allotrope.org/ontologies/hdf5/1.8#allocationTime
hdf:allocationTime rdf:type owl:ObjectProperty ;
                   rdfs:domain hdf:Dataset ;
                   rdfs:range hdf:StorageAllocation ;
                   rdfs:label "allocation time" ;
                   skos:prefLabel "allocation time" .


###  http://purl.allotrope.org/ontologies/hdf5/1.8#and
hdf:and rdf:type owl:ObjectProperty ;
        rdfs:label "and" ;
        skos:prefLabel "and" .


###  http://purl.allotrope.org/ontologies/hdf5/1.8#attribute
hdf:attribute rdf:type owl:ObjectProperty ;
              rdfs:domain hdf:NamedObject ;
              rdfs:range hdf:Attribute ;
              rdfs:comment "Relation between an HDF object and its attributes. [Allotrope]" ;
              rdfs:label "attribute" ;
              skos:definition "Relation between an HDF object and its attributes. [Allotrope]" ;
              skos:prefLabel "attribute" .


###  http://purl.allotrope.org/ontologies/hdf5/1.8#characterSet
hdf:characterSet rdf:type owl:ObjectProperty ;
                 rdfs:domain [ rdf:type owl:Class ;
                               owl:unionOf ( hdf:Link
                                             hdf:StringDatatype
                                           )
                             ] ;
                 rdfs:range hdf:CharacterSet ;
                 rdfs:comment "Relation between link or string datatype and character set used. [Allotrope]" ;
                 rdfs:label "character set" ;
                 skos:definition "Relation between link or string datatype and character set used. [Allotrope]" ;
                 skos:prefLabel "character set" .


###  http://purl.allotrope.org/ontologies/hdf5/1.8#chunk
hdf:chunk rdf:type owl:ObjectProperty ;
          rdfs:domain hdf:Dataset ;
          rdfs:range hdf:Chunk ;
          rdfs:comment "Relation between dataset and chunk. [Allotrope]" ;
          rdfs:label "chunk" ;
          skos:definition "Relation between dataset and chunk. [Allotrope]" ;
          skos:prefLabel "chunk" .


###  http://purl.allotrope.org/ontologies/hdf5/1.8#chunkMode
hdf:chunkMode rdf:type owl:ObjectProperty ;
              rdfs:domain hdf:Dataset ;
              rdfs:range hdf:ChunkMode ;
              rdfs:comment """Specifies whether I/O is to be performed as linked-chunk I/O or as multi-chunk I/O.
When an application uses collective I/O with chunked storage, the HDF5 Library normally uses an internal algorithm to determine whether that I/O activity should be conducted as one linked-chunk I/O or as multi-chunk I/O. ChunkMode is provided so that an application can override the library's algorithm in circumstances where the library might lack the information needed to make an optimal decision. [HDF]""" ;
              rdfs:label "chunk mode" ;
              skos:definition """Specifies whether I/O is to be performed as linked-chunk I/O or as multi-chunk I/O.
When an application uses collective I/O with chunked storage, the HDF5 Library normally uses an internal algorithm to determine whether that I/O activity should be conducted as one linked-chunk I/O or as multi-chunk I/O. ChunkMode is provided so that an application can override the library's algorithm in circumstances where the library might lack the information needed to make an optimal decision. [HDF]""" ;
              skos:prefLabel "chunk mode" .


###  http://purl.allotrope.org/ontologies/hdf5/1.8#compositeFillValue
hdf:compositeFillValue rdf:type owl:ObjectProperty ;
                       rdfs:subPropertyOf hdf:compositeValue ;
                       rdf:type owl:FunctionalProperty ;
                       rdfs:domain hdf:Dataset ;
                       rdfs:comment "User defined fill value for a composite datatype (array, compound or variable length). [HDF]" ;
                       rdfs:label "composite fill value" ;
                       skos:definition "User defined fill value for a composite datatype (array, compound or variable length). [HDF]" ;
                       skos:prefLabel "composite fill value" .


###  http://purl.allotrope.org/ontologies/hdf5/1.8#compositeValue
hdf:compositeValue rdf:type owl:ObjectProperty ;
                   rdfs:range hdf:CompositeValue ;
                   rdfs:label "composite value" ;
                   skos:prefLabel "composite value" .


###  http://purl.allotrope.org/ontologies/hdf5/1.8#coordinate
hdf:coordinate rdf:type owl:ObjectProperty ;
               rdfs:range hdf:Coordinate ;
               rdfs:label "coordinate" ;
               skos:prefLabel "coordinate" .


###  http://purl.allotrope.org/ontologies/hdf5/1.8#dataSource
hdf:dataSource rdf:type owl:ObjectProperty ;
               rdfs:label "data source" ;
               skos:prefLabel "data source" .


###  http://purl.allotrope.org/ontologies/hdf5/1.8#dataTarget
hdf:dataTarget rdf:type owl:ObjectProperty ;
               rdfs:label "data target" ;
               skos:prefLabel "data target" .


###  http://purl.allotrope.org/ontologies/hdf5/1.8#dataspace
hdf:dataspace rdf:type owl:ObjectProperty ;
              rdfs:domain [ rdf:type owl:Class ;
                            owl:unionOf ( hdf:Attribute
                                          hdf:Dataset
                                        )
                          ] ;
              rdfs:range hdf:Dataspace ;
              rdfs:label "dataspace" ;
              skos:definition "Relation between an attribute or dataset with its used dataspace. [Allotrope]" ;
              skos:prefLabel "dataspace" .


###  http://purl.allotrope.org/ontologies/hdf5/1.8#datatype
hdf:datatype rdf:type owl:ObjectProperty ;
             rdfs:domain [ rdf:type owl:Class ;
                           owl:unionOf ( hdf:ArrayDatatype
                                         hdf:Attribute
                                         hdf:CompoundDatatypeMember
                                         hdf:Dataset
                                         hdf:VariableLengthDatatype
                                       )
                         ] ;
             rdfs:range hdf:Datatype ;
             rdfs:comment "Relation between an array datatype, a compound datatype member, a variable length datatype, an attribute or a dataset and its datatype. [Allotrope]" ;
             rdfs:label "datatype" ;
             skos:definition "Relation between an array datatype, a compound datatype member, a variable length datatype, an attribute or a dataset and its datatype. [Allotrope]" ;
             skos:prefLabel "datatype" .


###  http://purl.allotrope.org/ontologies/hdf5/1.8#dimension
hdf:dimension rdf:type owl:ObjectProperty ;
              rdfs:domain [ rdf:type owl:Class ;
                            owl:unionOf ( hdf:ArrayDatatype
                                          hdf:Chunk
                                          hdf:Dataspace
                                        )
                          ] ;
              rdfs:range hdf:Dimension ;
              rdfs:comment "Relation between an array datatype, chunk or dataspace with a dimension. [Allotrope]" ;
              rdfs:label "dimension" ;
              skos:definition "Relation between an array datatype, chunk or dataspace with a dimension. [Allotrope]" ;
              skos:prefLabel "dimension" .


###  http://purl.allotrope.org/ontologies/hdf5/1.8#dimensionSelection
hdf:dimensionSelection rdf:type owl:ObjectProperty ;
                       rdfs:domain hdf:HyperSlab ;
                       rdfs:range hdf:DimensionSelection ;
                       rdfs:comment "Relation between a hyper slab and its dimension selection. [Allotrope]" ;
                       rdfs:label "dimension selection" ;
                       skos:definition "Relation between a hyper slab and its dimension selection. [Allotrope]" ;
                       skos:prefLabel "dimension selection" .


###  http://purl.allotrope.org/ontologies/hdf5/1.8#errorDetectionCheck
hdf:errorDetectionCheck rdf:type owl:ObjectProperty ;
                        rdfs:domain hdf:Dataset ;
                        rdfs:range hdf:ErrorDetectionCheck ;
                        rdfs:comment "Error detection check property of a dataset. [Allotrope]" ;
                        rdfs:label "error detection check" ;
                        skos:definition "Error detection check property of a dataset. [Allotrope]" ;
                        skos:prefLabel "error detection check" .


###  http://purl.allotrope.org/ontologies/hdf5/1.8#exponentField
hdf:exponentField rdf:type owl:ObjectProperty ;
                  rdfs:subPropertyOf hdf:field ;
                  rdf:type owl:FunctionalProperty ;
                  rdfs:range hdf:ExponentField ;
                  rdfs:comment "Exponent field property of a field. [Allotrope]" ;
                  rdfs:label "exponent field" ;
                  skos:definition "Exponent field property of a field. [Allotrope]" ;
                  skos:prefLabel "exponent field" .


###  http://purl.allotrope.org/ontologies/hdf5/1.8#externalLinkAccess
hdf:externalLinkAccess rdf:type owl:ObjectProperty ;
                       rdfs:domain hdf:Link ;
                       rdfs:range hdf:FileAccessMode ;
                       rdfs:label "external link access" ;
                       skos:definition "File access mode property of a link. [Allotrope]" ;
                       skos:prefLabel "external link access" .


###  http://purl.allotrope.org/ontologies/hdf5/1.8#field
hdf:field rdf:type owl:ObjectProperty ;
          rdfs:domain hdf:FloatDatatype ;
          rdfs:range hdf:FieldSpecification ;
          rdfs:comment "Defines the location (bit position of least significant bit of the filed) and size (in bits) of the field. [Allotrope]" ;
          rdfs:label "field" ;
          skos:definition "Defines the location (bit position of least significant bit of the filed) and size (in bits) of the field. [Allotrope]" ;
          skos:prefLabel "field" .


###  http://purl.allotrope.org/ontologies/hdf5/1.8#fillTime
hdf:fillTime rdf:type owl:ObjectProperty ;
             rdfs:domain hdf:Dataset ;
             rdfs:range hdf:FillTime ;
             rdfs:comment "Fill time property of a dataset. [Allotrope]" ;
             rdfs:label "fill time" ;
             skos:definition "Fill time property of a dataset. [Allotrope]" ;
             skos:prefLabel "fill time" .


###  http://purl.allotrope.org/ontologies/hdf5/1.8#fillValueStatus
hdf:fillValueStatus rdf:type owl:ObjectProperty ;
                    rdfs:domain hdf:Dataset ;
                    rdfs:range hdf:FillValueStatus ;
                    rdfs:comment "Fill value status property of a dataset. [Allotrope]" ;
                    rdfs:label "fill value status" ;
                    skos:definition "Fill value status property of a dataset. [Allotrope]" ;
                    skos:prefLabel "fill value status" .


###  http://purl.allotrope.org/ontologies/hdf5/1.8#filter
hdf:filter rdf:type owl:ObjectProperty ;
           rdfs:domain hdf:Dataset ;
           rdfs:range hdf:Filter ;
           rdfs:comment "Filter property of a dataset. [Allotrope]" ;
           rdfs:label "filter" ;
           skos:definition "Filter property of a dataset. [Allotrope]" ;
           skos:prefLabel "filter" .


###  http://purl.allotrope.org/ontologies/hdf5/1.8#internalPadding
hdf:internalPadding rdf:type owl:ObjectProperty ;
                    rdfs:domain hdf:FloatDatatype ;
                    rdfs:range hdf:Padding ;
                    rdfs:comment "If any internal bits (that is, bits between the sign bit, the mantissa field, and the exponent field but within the precision field) are unused, they will be filled according to this property. [Allotrope]" ;
                    rdfs:label "internal padding" ;
                    skos:definition "If any internal bits (that is, bits between the sign bit, the mantissa field, and the exponent field but within the precision field) are unused, they will be filled according to this property. [Allotrope]" ;
                    skos:prefLabel "internal padding" .


###  http://purl.allotrope.org/ontologies/hdf5/1.8#layout
hdf:layout rdf:type owl:ObjectProperty ;
           rdfs:domain hdf:Dataset ;
           rdfs:range hdf:StorageLayout ;
           rdfs:comment "Relation between a dataset and its storage layout. [Allotrope]" ;
           rdfs:label "layout" ;
           skos:definition "Relation between a dataset and its storage layout. [Allotrope]" ;
           skos:prefLabel "layout" .


###  http://purl.allotrope.org/ontologies/hdf5/1.8#link
hdf:link rdf:type owl:ObjectProperty ;
         rdfs:domain hdf:Group ;
         rdfs:range hdf:Link ;
         rdfs:comment "Relation between a group and link. [Allotrope]" ;
         rdfs:label "link" ;
         skos:definition "Relation between a group and link. [Allotrope]" ;
         skos:prefLabel "link" .


###  http://purl.allotrope.org/ontologies/hdf5/1.8#linkedTo
hdf:linkedTo rdf:type owl:ObjectProperty ;
             rdfs:subPropertyOf owl:topObjectProperty ;
             rdfs:domain hdf:Link ;
             rdfs:range hdf:NamedObject ;
             rdfs:comment "Relation between a link and its target named object. [Allotrope]" ;
             rdfs:label "linked to" ;
             skos:definition "Relation between a link and its target named object. [Allotrope]" ;
             skos:prefLabel "linked to" .


###  http://purl.allotrope.org/ontologies/hdf5/1.8#lsbPadding
hdf:lsbPadding rdf:type owl:ObjectProperty ;
               rdfs:domain hdf:AtomicDatatype ;
               rdfs:range hdf:Padding ;
               rdfs:comment "Least significant bit padding property of an atomic datatype. [Allotrope]" ;
               rdfs:label "least significant bit padding" ;
               skos:definition "Least significant bit padding property of an atomic datatype. [Allotrope]" ;
               skos:prefLabel "least significant bit padding" .


###  http://purl.allotrope.org/ontologies/hdf5/1.8#mantissaField
hdf:mantissaField rdf:type owl:ObjectProperty ;
                  rdfs:subPropertyOf hdf:field ;
                  rdf:type owl:FunctionalProperty ;
                  rdfs:range hdf:MantissaField ;
                  rdfs:comment "Mantissa field property of a field. [Allotrope]" ;
                  rdfs:label "mantissa field" ;
                  skos:definition "Mantissa field property of a field. [Allotrope]" ;
                  skos:prefLabel "mantissa field" .


###  http://purl.allotrope.org/ontologies/hdf5/1.8#member
hdf:member rdf:type owl:ObjectProperty ;
           rdfs:comment "Relation between collection and the members of it. [Allotrope]" ;
           rdfs:label "member" ;
           skos:definition "Relation between collection and the members of it. [Allotrope]" ;
           skos:prefLabel "member" .


###  http://purl.allotrope.org/ontologies/hdf5/1.8#msbPadding
hdf:msbPadding rdf:type owl:ObjectProperty ;
               rdfs:domain hdf:AtomicDatatype ;
               rdfs:range hdf:Padding ;
               rdfs:label "most significant bit padding" ;
               skos:definition "Most significant bit padding property of an atomic datatype. [Allotrope]" ;
               skos:prefLabel "most significant bit padding" .


###  http://purl.allotrope.org/ontologies/hdf5/1.8#multiDimensionalIndex
hdf:multiDimensionalIndex rdf:type owl:ObjectProperty ;
                          rdfs:label "multi index" ;
                          skos:prefLabel "multi index" .


###  http://purl.allotrope.org/ontologies/hdf5/1.8#normalization
hdf:normalization rdf:type owl:ObjectProperty ;
                  rdfs:domain hdf:FloatDatatype ;
                  rdfs:range hdf:FloatingPointNormalization ;
                  rdfs:label "normalization" ;
                  skos:definition "Normalization property of a float datatype. [Allotrope]" ;
                  skos:prefLabel "normalization" .


###  http://purl.allotrope.org/ontologies/hdf5/1.8#notA
hdf:notA rdf:type owl:ObjectProperty ;
         rdfs:label "not A" ;
         skos:prefLabel "not A" .


###  http://purl.allotrope.org/ontologies/hdf5/1.8#notB
hdf:notB rdf:type owl:ObjectProperty ;
         rdfs:label "not B" ;
         skos:prefLabel "not B" .


###  http://purl.allotrope.org/ontologies/hdf5/1.8#or
hdf:or rdf:type owl:ObjectProperty ;
       rdfs:label "or" ;
       skos:prefLabel "or" .


###  http://purl.allotrope.org/ontologies/hdf5/1.8#order
hdf:order rdf:type owl:ObjectProperty ;
          rdfs:domain hdf:Datatype ;
          rdfs:range hdf:Order ;
          rdfs:label "order" ;
          skos:definition "Order property of a datatype. [Allotrope]" ;
          skos:prefLabel "order" .


###  http://purl.allotrope.org/ontologies/hdf5/1.8#point
hdf:point rdf:type owl:ObjectProperty ;
          rdfs:range hdf:Point ;
          rdfs:label "point" ;
          skos:prefLabel "point" .


###  http://purl.allotrope.org/ontologies/hdf5/1.8#previous
hdf:previous rdf:type owl:ObjectProperty ;
             rdfs:comment "In a combined selection the predicate points to the existing selection that the combination operator is applied on. [Allotrope]" ;
             rdfs:label "previous" ;
             skos:definition "In a combined selection the predicate points to the existing selection that the combination operator is applied on. [Allotrope]" ;
             skos:prefLabel "previous" .


###  http://purl.allotrope.org/ontologies/hdf5/1.8#rootGroup
hdf:rootGroup rdf:type owl:ObjectProperty ;
              rdfs:domain hdf:File ;
              rdfs:range hdf:Group ;
              rdfs:label "root group" ;
              skos:definition "Relation between the HDF file and its root group. [Allotrope]" ;
              skos:prefLabel "root group" .


###  http://purl.allotrope.org/ontologies/hdf5/1.8#scaleType
hdf:scaleType rdf:type owl:ObjectProperty ;
              rdfs:domain hdf:Dataset ;
              rdfs:range hdf:ScaleType ;
              rdfs:label "scale type" ;
              skos:definition "Scale type property of a dataset. [Allotrope]" ;
              skos:prefLabel "scale type" .


###  http://purl.allotrope.org/ontologies/hdf5/1.8#selectionOn
hdf:selectionOn rdf:type owl:ObjectProperty ;
                rdfs:domain hdf:Selection ;
                rdfs:range [ rdf:type owl:Class ;
                             owl:unionOf ( hdf:Dataspace
                                           hdf:Selection
                                         )
                           ] ;
                rdfs:label "selection on" ;
                skos:definition "Relation between a selection and its target, either a dataspace or another selection. [Allotrope]" ;
                skos:prefLabel "selection on" .


###  http://purl.allotrope.org/ontologies/hdf5/1.8#sign
hdf:sign rdf:type owl:ObjectProperty ;
         rdfs:domain hdf:IntegerDatatype ;
         rdfs:range hdf:Sign ;
         rdfs:label "sign" ;
         skos:definition "Sign property of an integer datatype. [Allotrope]" ;
         skos:prefLabel "sign" .


###  http://purl.allotrope.org/ontologies/hdf5/1.8#signField
hdf:signField rdf:type owl:ObjectProperty ;
              rdfs:subPropertyOf hdf:field ;
              rdf:type owl:FunctionalProperty ;
              rdfs:range hdf:SignField ;
              rdfs:label "sign field" ;
              skos:definition "Sign field property of a field. [Allotrope]" ;
              skos:prefLabel "sign field" .


###  http://purl.allotrope.org/ontologies/hdf5/1.8#stringPadding
hdf:stringPadding rdf:type owl:ObjectProperty ;
                  rdfs:domain hdf:StringDatatype ;
                  rdfs:range hdf:StringPadding ;
                  rdfs:label "string padding" ;
                  skos:definition "String padding property of a string datatype. [Allotrope]" ;
                  skos:prefLabel "string padding" .


###  http://purl.allotrope.org/ontologies/hdf5/1.8#szipEncoding
hdf:szipEncoding rdf:type owl:ObjectProperty ;
                 rdfs:domain hdf:FilterSZip ;
                 rdfs:range hdf:SZipCoding ;
                 rdfs:label "SZip encoding" ;
                 skos:definition "SZip encoding property of a SZip filter. [Allotrope]" ;
                 skos:prefLabel "SZip encoding" .


###  http://purl.allotrope.org/ontologies/hdf5/1.8#transferMode
hdf:transferMode rdf:type owl:ObjectProperty ;
                 rdfs:domain hdf:Dataset ;
                 rdfs:range hdf:TransferMode ;
                 rdfs:label "transfer mode" ;
                 skos:definition "Transfer mode property of a dataset. [Allotrope]" ;
                 skos:prefLabel "transfer mode" .


###  http://purl.allotrope.org/ontologies/hdf5/1.8#typeClass
hdf:typeClass rdf:type owl:ObjectProperty ;
              rdfs:range hdf:TypeClass ;
              rdfs:label "type class" ;
              skos:prefLabel "type class" .


###  http://purl.allotrope.org/ontologies/hdf5/1.8#writtenRegion
hdf:writtenRegion rdf:type owl:ObjectProperty ;
                  rdfs:comment "The region of a dataset that has ever been written to. This typically only encompasses the maximum index in the dimensions, exact tracking is impossible in current HDF because empty positions are indistinguishable from positions with the fill value. [Allotrope]" ;
                  rdfs:label "written region" ;
                  skos:definition "The region of a dataset that has ever been written to. This typically only encompasses the maximum index in the dimensions, exact tracking is impossible in current HDF because empty positions are indistinguishable from positions with the fill value. [Allotrope]" ;
                  skos:prefLabel "written region" .


###  http://purl.allotrope.org/ontologies/hdf5/1.8#xor
hdf:xor rdf:type owl:ObjectProperty ;
        rdfs:label "xor" ;
        skos:altLabel "exclusive or" ;
        skos:prefLabel "xor" .


#################################################################
#    Data properties
#################################################################

###  http://purl.allotrope.org/ontologies/hdf5/1.8#atomicFillValue
hdf:atomicFillValue rdf:type owl:DatatypeProperty ;
                    rdfs:subPropertyOf hdf:value ;
                    rdf:type owl:FunctionalProperty ;
                    rdfs:domain hdf:Dataset ;
                    rdfs:comment "User defined fill value for an atomic datatype. [Allotrope]" ;
                    rdfs:label "atomic fill value" ;
                    skos:definition "User defined fill value for an atomic datatype. [Allotrope]" ;
                    skos:prefLabel "atomic fill value" .


###  http://purl.allotrope.org/ontologies/hdf5/1.8#block
hdf:block rdf:type owl:DatatypeProperty ;
          rdfs:range xsd:nonNegativeInteger ;
          rdfs:comment "The block is a count on the number of repetitions of the hyperslab. [Allotrope]" ;
          rdfs:label "block" ;
          skos:definition "The block is a count on the number of repetitions of the hyperslab. [Allotrope]" ;
          skos:prefLabel "block" .


###  http://purl.allotrope.org/ontologies/hdf5/1.8#btreeIStoreSize
hdf:btreeIStoreSize rdf:type owl:DatatypeProperty ;
                    rdfs:domain hdf:File ;
                    rdfs:range xsd:unsignedInt ;
                    rdfs:label "btree istore size" ;
                    skos:prefLabel "btree istore size" .


###  http://purl.allotrope.org/ontologies/hdf5/1.8#btreeLeaf
hdf:btreeLeaf rdf:type owl:DatatypeProperty ;
              rdfs:domain hdf:File ;
              rdfs:range xsd:nonNegativeInteger ;
              rdfs:label "btree leaf" ;
              skos:prefLabel "btree leaf" .


###  http://purl.allotrope.org/ontologies/hdf5/1.8#btreeRank
hdf:btreeRank rdf:type owl:DatatypeProperty ;
              rdfs:domain hdf:File ;
              rdfs:range xsd:nonNegativeInteger ;
              rdfs:label "btree rank" ;
              skos:prefLabel "btree rank" .


###  http://purl.allotrope.org/ontologies/hdf5/1.8#btreeRatioLeft
hdf:btreeRatioLeft rdf:type owl:DatatypeProperty ;
                   rdfs:domain hdf:File ;
                   rdfs:range xsd:double ;
                   rdfs:label "btree left ratio" ;
                   skos:prefLabel "btree left ratio" .


###  http://purl.allotrope.org/ontologies/hdf5/1.8#btreeRatioMiddle
hdf:btreeRatioMiddle rdf:type owl:DatatypeProperty ;
                     rdfs:domain hdf:File ;
                     rdfs:range xsd:double ;
                     rdfs:label "btree middle ratio" ;
                     skos:prefLabel "btree middle ratio" .


###  http://purl.allotrope.org/ontologies/hdf5/1.8#btreeRatioRight
hdf:btreeRatioRight rdf:type owl:DatatypeProperty ;
                    rdfs:domain hdf:File ;
                    rdfs:range xsd:double ;
                    rdfs:label "btree right ratio" ;
                    skos:prefLabel "btree right ratio" .


###  http://purl.allotrope.org/ontologies/hdf5/1.8#bufferSize
hdf:bufferSize rdf:type owl:DatatypeProperty ;
               rdfs:domain hdf:Dataset ;
               rdfs:range xsd:long ;
               rdfs:label "buffer size" ;
               skos:definition "Size, in bytes, of the type conversion and background buffers. [HDF]" ;
               skos:prefLabel "buffer size" .


###  http://purl.allotrope.org/ontologies/hdf5/1.8#chunkCachePreemptionPolicy
hdf:chunkCachePreemptionPolicy rdf:type owl:DatatypeProperty ;
                               rdfs:domain hdf:Dataset ;
                               rdfs:range [ rdf:type rdfs:Datatype ;
                                            owl:onDatatype xsd:double ;
                                            owl:withRestrictions ( [ xsd:minInclusive "0.0"^^xsd:double
                                                                   ]
                                                                   [ xsd:maxInclusive "1.0"^^xsd:double
                                                                   ]
                                                                 )
                                          ] ;
                               rdfs:comment "The chunk preemption policy for all datasets. This must be between 0 and 1 inclusive and indicates the weighting according to which chunks which have been fully read or written are penalized when determining which chunks to flush from cache. A value of 0 means fully read or written chunks are treated no differently than other chunks (the preemption is strictly LRU) while a value of 1 means fully read or written chunks are always preempted before other chunks. If your application only reads or writes data once, this can be safely set to 1. Otherwise, this should be set lower depending on how often you re-read or re-write the same data. [HDF]" ;
                               rdfs:label "chunk cache preemption policy" ;
                               skos:definition "The chunk preemption policy for all datasets. This must be between 0 and 1 inclusive and indicates the weighting according to which chunks which have been fully read or written are penalized when determining which chunks to flush from cache. A value of 0 means fully read or written chunks are treated no differently than other chunks (the preemption is strictly LRU) while a value of 1 means fully read or written chunks are always preempted before other chunks. If your application only reads or writes data once, this can be safely set to 1. Otherwise, this should be set lower depending on how often you re-read or re-write the same data. [HDF]" ;
                               skos:prefLabel "chunk cache preemption policy" .


###  http://purl.allotrope.org/ontologies/hdf5/1.8#chunkCacheSize
hdf:chunkCacheSize rdf:type owl:DatatypeProperty ;
                   rdfs:domain hdf:Dataset ;
                   rdfs:range xsd:long ;
                   rdfs:comment "The number of chunk slots in the raw data chunk cache hash table , the maximum possible number of bytes in the raw data chunk cache, and the preemption policy value. [HDF]" ;
                   rdfs:label "chunk cache size" ;
                   skos:definition "The number of chunk slots in the raw data chunk cache hash table , the maximum possible number of bytes in the raw data chunk cache, and the preemption policy value. [HDF]" ;
                   skos:prefLabel "chunk cache size" .


###  http://purl.allotrope.org/ontologies/hdf5/1.8#chunkCacheSlots
hdf:chunkCacheSlots rdf:type owl:DatatypeProperty ;
                    rdfs:domain hdf:Dataset ;
                    rdfs:range xsd:long ;
                    rdfs:label "chunk cache slots" ;
                    skos:prefLabel "chunk cache slots" .


###  http://purl.allotrope.org/ontologies/hdf5/1.8#collectiveIOThreshold
hdf:collectiveIOThreshold rdf:type owl:DatatypeProperty ;
                          rdfs:range [ rdf:type rdfs:Datatype ;
                                       owl:onDatatype xsd:int ;
                                       owl:withRestrictions ( [ xsd:minInclusive 0
                                                              ]
                                                              [ xsd:maxInclusive "100"^^xsd:int
                                                              ]
                                                            )
                                     ] ;
                          rdfs:label "collective I/O threshold" ;
                          skos:prefLabel "collective I/O threshold" .


###  http://purl.allotrope.org/ontologies/hdf5/1.8#compressionLevel
hdf:compressionLevel rdf:type owl:DatatypeProperty ;
                     rdfs:range xsd:int ;
                     rdfs:label "compression level" ;
                     skos:prefLabel "compression level" .


###  http://purl.allotrope.org/ontologies/hdf5/1.8#coordinateIndex
hdf:coordinateIndex rdf:type owl:DatatypeProperty ;
                    rdfs:subPropertyOf hdf:index ;
                    rdfs:comment "index in dimension. [Allotrope]" ;
                    skos:definition "index in dimension. [Allotrope]" ;
                    skos:prefLabel "coordinate index" .


###  http://purl.allotrope.org/ontologies/hdf5/1.8#count
hdf:count rdf:type owl:DatatypeProperty ;
          rdfs:range [ rdf:type rdfs:Datatype ;
                       owl:onDatatype xsd:integer ;
                       owl:withRestrictions ( [ xsd:minInclusive 0
                                              ]
                                            )
                     ] ;
          rdfs:comment "The count is the number of elements in the hyperslab selection. When the stride is 1, the selection is a hyper rectangle with a corner at the offset and size count[0] by count[1] by.... When stride is greater than one, the hyperslab bounded by the offset and the corners defined by stride[n] * count[n]. [Allotrope]" ;
          rdfs:label "count" ;
          skos:definition "The count is the number of elements in the hyperslab selection. When the stride is 1, the selection is a hyper rectangle with a corner at the offset and size count[0] by count[1] by.... When stride is greater than one, the hyperslab bounded by the offset and the corners defined by stride[n] * count[n]. [Allotrope]" ;
          skos:prefLabel "count" .


###  http://purl.allotrope.org/ontologies/hdf5/1.8#createIntermediateGroups
hdf:createIntermediateGroups rdf:type owl:DatatypeProperty ;
                             rdfs:domain hdf:Link ;
                             rdfs:range xsd:boolean ;
                             rdfs:label "create intermediate groups" .


###  http://purl.allotrope.org/ontologies/hdf5/1.8#currentSize
hdf:currentSize rdf:type owl:DatatypeProperty ;
                rdfs:subPropertyOf hdf:size ;
                rdfs:label "current size" ;
                skos:prefLabel "current size" .


###  http://purl.allotrope.org/ontologies/hdf5/1.8#data
hdf:data rdf:type owl:DatatypeProperty ;
         rdfs:domain hdf:Attribute ;
         rdfs:label "data" ;
         skos:prefLabel "data" .


###  http://purl.allotrope.org/ontologies/hdf5/1.8#deflateLevel
hdf:deflateLevel rdf:type owl:DatatypeProperty ;
                 rdfs:domain hdf:Dataset ;
                 rdfs:range [ rdf:type rdfs:Datatype ;
                              owl:onDatatype xsd:int ;
                              owl:withRestrictions ( [ xsd:minInclusive "0"^^xsd:int
                                                     ]
                                                     [ xsd:maxInclusive "9"^^xsd:int
                                                     ]
                                                   )
                            ] ;
                 rdfs:label "deflate level" ;
                 skos:prefLabel "deflate level" .


###  http://purl.allotrope.org/ontologies/hdf5/1.8#dimensionIndex
hdf:dimensionIndex rdf:type owl:DatatypeProperty ;
                   rdfs:subPropertyOf hdf:index ;
                   rdfs:range hdf:DimensionIndexType ;
                   rdfs:comment "index of the dimension. [Allotrope]" ;
                   rdfs:label "dimension index" ;
                   skos:definition "index of the dimension. [Allotrope]" ;
                   skos:prefLabel "dimension index" .


###  http://purl.allotrope.org/ontologies/hdf5/1.8#ebias
hdf:ebias rdf:type owl:DatatypeProperty ;
          rdfs:domain hdf:FloatDatatype ;
          rdfs:range xsd:nonNegativeInteger ;
          rdfs:label "ebias" ;
          skos:prefLabel "ebias" .


###  http://purl.allotrope.org/ontologies/hdf5/1.8#externalLinkCacheSize
hdf:externalLinkCacheSize rdf:type owl:DatatypeProperty ;
                          rdfs:domain hdf:Link ;
                          rdfs:range xsd:nonNegativeInteger ;
                          rdfs:label "external link cache size" ;
                          skos:prefLabel "external link cache size" .


###  http://purl.allotrope.org/ontologies/hdf5/1.8#externalLinkPrefix
hdf:externalLinkPrefix rdf:type owl:DatatypeProperty ;
                       rdfs:domain hdf:Link ;
                       rdfs:range xsd:string ;
                       rdfs:label "external link prefix" ;
                       skos:prefLabel "external link prefix" .


###  http://purl.allotrope.org/ontologies/hdf5/1.8#globalFreelistVersion
hdf:globalFreelistVersion rdf:type owl:DatatypeProperty ;
                          rdfs:domain hdf:File ;
                          rdfs:range xsd:int ;
                          rdfs:label "global freelist version" ;
                          skos:prefLabel "global freelist version" .


###  http://purl.allotrope.org/ontologies/hdf5/1.8#hyperVectorSize
hdf:hyperVectorSize rdf:type owl:DatatypeProperty ;
                    rdfs:domain hdf:Dataset ;
                    rdfs:range [ rdf:type rdfs:Datatype ;
                                 owl:onDatatype xsd:integer ;
                                 owl:withRestrictions ( [ xsd:minInclusive 0
                                                        ]
                                                      )
                               ] ;
                    rdfs:label "hyper vector size" ;
                    skos:prefLabel "hyper vector size" .


###  http://purl.allotrope.org/ontologies/hdf5/1.8#iStoreK
hdf:iStoreK rdf:type owl:DatatypeProperty ;
            rdfs:domain hdf:Dataset ;
            rdfs:range xsd:nonNegativeInteger ;
            rdfs:label "iStoreK" ;
            skos:prefLabel "iStoreK" .


###  http://purl.allotrope.org/ontologies/hdf5/1.8#index
hdf:index rdf:type owl:DatatypeProperty ;
          rdfs:range hdf:IndexType ;
          rdfs:label "index" ;
          skos:prefLabel "index" .


###  http://purl.allotrope.org/ontologies/hdf5/1.8#index_0
hdf:index_0 rdf:type owl:DatatypeProperty ;
            rdfs:subPropertyOf hdf:index ;
            rdfs:comment "Index in dimension 0. [Allotrope]" ;
            rdfs:label "index 0" ;
            skos:definition "Index in dimension 0. [Allotrope]" ;
            skos:prefLabel "index 0" .


###  http://purl.allotrope.org/ontologies/hdf5/1.8#index_1
hdf:index_1 rdf:type owl:DatatypeProperty ;
            rdfs:subPropertyOf hdf:index ;
            rdfs:comment "Index in dimension 1. [Allotrope]" ;
            rdfs:label "index 1" ;
            skos:definition "Index in dimension 1. [Allotrope]" ;
            skos:prefLabel "index 1" .


###  http://purl.allotrope.org/ontologies/hdf5/1.8#index_10
hdf:index_10 rdf:type owl:DatatypeProperty ;
             rdfs:subPropertyOf hdf:index ;
             rdfs:comment "Index in dimension 10. [Allotrope]" ;
             rdfs:label "index 10" ;
             skos:definition "Index in dimension 10. [Allotrope]" ;
             skos:prefLabel "index 10" .


###  http://purl.allotrope.org/ontologies/hdf5/1.8#index_11
hdf:index_11 rdf:type owl:DatatypeProperty ;
             rdfs:subPropertyOf hdf:index ;
             rdfs:comment "Index in dimension 11. [Allotrope]" ;
             rdfs:label "index 11" ;
             skos:definition "Index in dimension 11. [Allotrope]" ;
             skos:prefLabel "index 11" .


###  http://purl.allotrope.org/ontologies/hdf5/1.8#index_12
hdf:index_12 rdf:type owl:DatatypeProperty ;
             rdfs:subPropertyOf hdf:index ;
             rdfs:comment "Index in dimension 12. [Allotrope]" ;
             rdfs:label "index 12" ;
             skos:definition "Index in dimension 12. [Allotrope]" ;
             skos:prefLabel "index 12" .


###  http://purl.allotrope.org/ontologies/hdf5/1.8#index_13
hdf:index_13 rdf:type owl:DatatypeProperty ;
             rdfs:subPropertyOf hdf:index ;
             rdfs:comment "Index in dimension 13. [Allotrope]" ;
             rdfs:label "index 13" ;
             skos:definition "Index in dimension 13. [Allotrope]" ;
             skos:prefLabel "index 13" .


###  http://purl.allotrope.org/ontologies/hdf5/1.8#index_14
hdf:index_14 rdf:type owl:DatatypeProperty ;
             rdfs:subPropertyOf hdf:index ;
             rdfs:comment "Index in dimension 14. [Allotrope]" ;
             rdfs:label "index 14" ;
             skos:definition "Index in dimension 14. [Allotrope]" ;
             skos:prefLabel "index 14" .


###  http://purl.allotrope.org/ontologies/hdf5/1.8#index_15
hdf:index_15 rdf:type owl:DatatypeProperty ;
             rdfs:subPropertyOf hdf:index ;
             rdfs:comment "Index in dimension 15. [Allotrope]" ;
             rdfs:label "index 15" ;
             skos:definition "Index in dimension 15. [Allotrope]" ;
             skos:prefLabel "index 15" .


###  http://purl.allotrope.org/ontologies/hdf5/1.8#index_16
hdf:index_16 rdf:type owl:DatatypeProperty ;
             rdfs:subPropertyOf hdf:index ;
             rdfs:comment "Index in dimension 16. [Allotrope]" ;
             rdfs:label "index 16" ;
             skos:definition "Index in dimension 16. [Allotrope]" ;
             skos:prefLabel "index 16" .


###  http://purl.allotrope.org/ontologies/hdf5/1.8#index_17
hdf:index_17 rdf:type owl:DatatypeProperty ;
             rdfs:subPropertyOf hdf:index ;
             rdfs:comment "Index in dimension 17. [Allotrope]" ;
             rdfs:label "index 17" ;
             skos:definition "Index in dimension 17. [Allotrope]" ;
             skos:prefLabel "index 17" .


###  http://purl.allotrope.org/ontologies/hdf5/1.8#index_18
hdf:index_18 rdf:type owl:DatatypeProperty ;
             rdfs:subPropertyOf hdf:index ;
             rdfs:comment "Index in dimension 18. [Allotrope]" ;
             rdfs:label "index 18" ;
             skos:definition "Index in dimension 18. [Allotrope]" ;
             skos:prefLabel "index 18" .


###  http://purl.allotrope.org/ontologies/hdf5/1.8#index_19
hdf:index_19 rdf:type owl:DatatypeProperty ;
             rdfs:subPropertyOf hdf:index ;
             rdfs:comment "Index in dimension 19. [Allotrope]" ;
             rdfs:label "index 19" ;
             skos:definition "Index in dimension 19. [Allotrope]" ;
             skos:prefLabel "index 19" .


###  http://purl.allotrope.org/ontologies/hdf5/1.8#index_2
hdf:index_2 rdf:type owl:DatatypeProperty ;
            rdfs:subPropertyOf hdf:index ;
            rdfs:comment "Index in dimension 2. [Allotrope]" ;
            rdfs:label "index 2" ;
            skos:definition "Index in dimension 2. [Allotrope]" ;
            skos:prefLabel "index 2" .


###  http://purl.allotrope.org/ontologies/hdf5/1.8#index_20
hdf:index_20 rdf:type owl:DatatypeProperty ;
             rdfs:subPropertyOf hdf:index ;
             rdfs:comment "Index in dimension 20. [Allotrope]" ;
             rdfs:label "index 20" ;
             skos:definition "Index in dimension 20. [Allotrope]" ;
             skos:prefLabel "index 20" .


###  http://purl.allotrope.org/ontologies/hdf5/1.8#index_21
hdf:index_21 rdf:type owl:DatatypeProperty ;
             rdfs:subPropertyOf hdf:index ;
             rdfs:comment "Index in dimension 21. [Allotrope]" ;
             rdfs:label "index 21" ;
             skos:definition "Index in dimension 21. [Allotrope]" ;
             skos:prefLabel "index 21" .


###  http://purl.allotrope.org/ontologies/hdf5/1.8#index_22
hdf:index_22 rdf:type owl:DatatypeProperty ;
             rdfs:subPropertyOf hdf:index ;
             rdfs:comment "Index in dimension 22. [Allotrope]" ;
             rdfs:label "index 22" ;
             skos:definition "Index in dimension 22. [Allotrope]" ;
             skos:prefLabel "index 22" .


###  http://purl.allotrope.org/ontologies/hdf5/1.8#index_23
hdf:index_23 rdf:type owl:DatatypeProperty ;
             rdfs:subPropertyOf hdf:index ;
             rdfs:comment "Index in dimension 23. [Allotrope]" ;
             rdfs:label "index 23" ;
             skos:definition "Index in dimension 23. [Allotrope]" ;
             skos:prefLabel "index 23" .


###  http://purl.allotrope.org/ontologies/hdf5/1.8#index_24
hdf:index_24 rdf:type owl:DatatypeProperty ;
             rdfs:subPropertyOf hdf:index ;
             rdfs:comment "Index in dimension 24. [Allotrope]" ;
             rdfs:label "index 24" ;
             skos:definition "Index in dimension 24. [Allotrope]" ;
             skos:prefLabel "index 24" .


###  http://purl.allotrope.org/ontologies/hdf5/1.8#index_25
hdf:index_25 rdf:type owl:DatatypeProperty ;
             rdfs:subPropertyOf hdf:index ;
             rdfs:comment "Index in dimension 25. [Allotrope]" ;
             rdfs:label "index 25" ;
             skos:definition "Index in dimension 25. [Allotrope]" ;
             skos:prefLabel "index 25" .


###  http://purl.allotrope.org/ontologies/hdf5/1.8#index_26
hdf:index_26 rdf:type owl:DatatypeProperty ;
             rdfs:subPropertyOf hdf:index ;
             rdfs:comment "Index in dimension 26. [Allotrope]" ;
             rdfs:label "index 26" ;
             skos:definition "Index in dimension 26. [Allotrope]" ;
             skos:prefLabel "index 26" .


###  http://purl.allotrope.org/ontologies/hdf5/1.8#index_27
hdf:index_27 rdf:type owl:DatatypeProperty ;
             rdfs:subPropertyOf hdf:index ;
             rdfs:comment "index in dimension 27. [Allotrope]" ;
             rdfs:label "index 27" ;
             skos:definition "Index in dimension 27. [Allotrope]" ;
             skos:prefLabel "index 27" .


###  http://purl.allotrope.org/ontologies/hdf5/1.8#index_28
hdf:index_28 rdf:type owl:DatatypeProperty ;
             rdfs:subPropertyOf hdf:index ;
             rdfs:comment "index in dimension 28. [Allotrope]" ;
             rdfs:label "index 28" ;
             skos:definition "Index in dimension 28. [Allotrope]" ;
             skos:prefLabel "index 28" .


###  http://purl.allotrope.org/ontologies/hdf5/1.8#index_29
hdf:index_29 rdf:type owl:DatatypeProperty ;
             rdfs:subPropertyOf hdf:index ;
             rdfs:comment "index in dimension 29. [Allotrope]" ;
             rdfs:label "index 29" ;
             skos:definition "Index in dimension 29. [Allotrope]" ;
             skos:prefLabel "index 29" .


###  http://purl.allotrope.org/ontologies/hdf5/1.8#index_3
hdf:index_3 rdf:type owl:DatatypeProperty ;
            rdfs:subPropertyOf hdf:index ;
            rdfs:comment "Index in dimension 3. [Allotrope]" ;
            rdfs:label "index 3" ;
            skos:definition "Index in dimension 3. [Allotrope]" ;
            skos:prefLabel "index 3" .


###  http://purl.allotrope.org/ontologies/hdf5/1.8#index_30
hdf:index_30 rdf:type owl:DatatypeProperty ;
             rdfs:subPropertyOf hdf:index ;
             rdfs:comment "Index in dimension 30. [Allotrope]" ;
             rdfs:label "index 30" ;
             skos:definition "Index in dimension 30. [Allotrope]" ;
             skos:prefLabel "index 30" .


###  http://purl.allotrope.org/ontologies/hdf5/1.8#index_31
hdf:index_31 rdf:type owl:DatatypeProperty ;
             rdfs:subPropertyOf hdf:index ;
             rdfs:comment "Index in dimension 31. [Allotrope]" ;
             rdfs:label "index 31" ;
             skos:definition "Index in dimension 31. [Allotrope]" ;
             skos:prefLabel "index 31" .


###  http://purl.allotrope.org/ontologies/hdf5/1.8#index_4
hdf:index_4 rdf:type owl:DatatypeProperty ;
            rdfs:subPropertyOf hdf:index ;
            rdfs:comment "Index in dimension 4. [Allotrope]" ;
            rdfs:label "index 4" ;
            skos:definition "Index in dimension 4. [Allotrope]" ;
            skos:prefLabel "index 4" .


###  http://purl.allotrope.org/ontologies/hdf5/1.8#index_5
hdf:index_5 rdf:type owl:DatatypeProperty ;
            rdfs:subPropertyOf hdf:index ;
            rdfs:comment "Index in dimension 5. [Allotrope]" ;
            rdfs:label "index 5" ;
            skos:definition "Index in dimension 5. [Allotrope]" ;
            skos:prefLabel "index 5" .


###  http://purl.allotrope.org/ontologies/hdf5/1.8#index_6
hdf:index_6 rdf:type owl:DatatypeProperty ;
            rdfs:subPropertyOf hdf:index ;
            rdfs:comment "Index in dimension 6. [Allotrope]" ;
            rdfs:label "index 6" ;
            skos:definition "Index in dimension 6. [Allotrope]" ;
            skos:prefLabel "index 6" .


###  http://purl.allotrope.org/ontologies/hdf5/1.8#index_7
hdf:index_7 rdf:type owl:DatatypeProperty ;
            rdfs:subPropertyOf hdf:index ;
            rdfs:comment "Index in dimension 7. [Allotrope]" ;
            rdfs:label "index 7" ;
            skos:definition "Index in dimension 7. [Allotrope]" ;
            skos:prefLabel "index 7" .


###  http://purl.allotrope.org/ontologies/hdf5/1.8#index_8
hdf:index_8 rdf:type owl:DatatypeProperty ;
            rdfs:subPropertyOf hdf:index ;
            rdfs:comment "Index in dimension 8. [Allotrope]" ;
            rdfs:label "index 8" ;
            skos:definition "Index in dimension 8. [Allotrope]" ;
            skos:prefLabel "index 8" .


###  http://purl.allotrope.org/ontologies/hdf5/1.8#index_9
hdf:index_9 rdf:type owl:DatatypeProperty ;
            rdfs:subPropertyOf hdf:index ;
            rdfs:comment "Index in dimension 9. [Allotrope]" ;
            rdfs:label "index 9" ;
            skos:definition "Index in dimension 9. [Allotrope]" ;
            skos:prefLabel "index 9" .


###  http://purl.allotrope.org/ontologies/hdf5/1.8#initialSize
hdf:initialSize rdf:type owl:DatatypeProperty ;
                rdfs:subPropertyOf hdf:size ;
                rdfs:label "initial size" ;
                skos:prefLabel "initial size" .


###  http://purl.allotrope.org/ontologies/hdf5/1.8#isVariableLength
hdf:isVariableLength rdf:type owl:DatatypeProperty ;
                     rdfs:domain hdf:StringDatatype ;
                     rdfs:range xsd:boolean ;
                     rdfs:comment "flag indicating that a string type is of variable length. [Allotrope]" ;
                     rdfs:label "is variable length" ;
                     skos:definition "flag indicating that a string type is of variable length. [Allotrope]" ;
                     skos:prefLabel "is variable length" .


###  http://purl.allotrope.org/ontologies/hdf5/1.8#linkedChunkThreshold
hdf:linkedChunkThreshold rdf:type owl:DatatypeProperty ;
                         rdfs:range [ rdf:type rdfs:Datatype ;
                                      owl:onDatatype xsd:int ;
                                      owl:withRestrictions ( [ xsd:minInclusive "0"^^xsd:int
                                                             ]
                                                           )
                                    ] ;
                         rdfs:label "linked chunk threshold" ;
                         skos:prefLabel "linked chunk threshold" .


###  http://purl.allotrope.org/ontologies/hdf5/1.8#maximumLinkTraversals
hdf:maximumLinkTraversals rdf:type owl:DatatypeProperty ;
                          rdfs:range xsd:int ;
                          rdfs:label "maximum link traversals" ;
                          skos:prefLabel "maximum link traversals" .


###  http://purl.allotrope.org/ontologies/hdf5/1.8#maximumSize
hdf:maximumSize rdf:type owl:DatatypeProperty ;
                rdfs:subPropertyOf hdf:size ;
                rdfs:label "maximum size" ;
                skos:prefLabel "maximum size" .


###  http://purl.allotrope.org/ontologies/hdf5/1.8#metaBlockSize
hdf:metaBlockSize rdf:type owl:DatatypeProperty ;
                  rdfs:domain hdf:File ;
                  rdfs:range xsd:long ;
                  rdfs:label "meta block size" ;
                  skos:prefLabel "meta block size" .


###  http://purl.allotrope.org/ontologies/hdf5/1.8#minimumSize
hdf:minimumSize rdf:type owl:DatatypeProperty ;
                rdfs:subPropertyOf hdf:size ;
                rdfs:label "minimum size" ;
                skos:prefLabel "minimum size" .


###  http://purl.allotrope.org/ontologies/hdf5/1.8#name
hdf:name rdf:type owl:DatatypeProperty ;
         rdfs:range xsd:string ;
         rdfs:label "name" ;
         skos:prefLabel "name" .


###  http://purl.allotrope.org/ontologies/hdf5/1.8#offset
hdf:offset rdf:type owl:DatatypeProperty ;
           rdfs:domain hdf:AtomicDatatype ;
           rdfs:range xsd:int ;
           rdfs:comment "The bit offset of the first significant bit. The significant bits of an atomic datum can be offset from the beginning of the memory for that datum by an amount of padding. [Allotrope]" ;
           rdfs:label "offset size" ;
           skos:definition "The bit offset of the first significant bit. The significant bits of an atomic datum can be offset from the beginning of the memory for that datum by an amount of padding. [Allotrope]" ;
           skos:prefLabel "offset size" .


###  http://purl.allotrope.org/ontologies/hdf5/1.8#pixelsPerBlock
hdf:pixelsPerBlock rdf:type owl:DatatypeProperty ;
                   rdfs:domain hdf:FilterSZip ;
                   rdfs:range xsd:int ;
                   rdfs:label "pixels per block" ;
                   skos:prefLabel "pixels per block" .


###  http://purl.allotrope.org/ontologies/hdf5/1.8#position
hdf:position rdf:type owl:DatatypeProperty ;
             rdfs:domain hdf:FieldSpecification ;
             rdfs:range xsd:nonNegativeInteger ;
             rdfs:label "position" ;
             skos:prefLabel "position" .


###  http://purl.allotrope.org/ontologies/hdf5/1.8#precision
hdf:precision rdf:type owl:DatatypeProperty ;
              rdfs:domain hdf:AtomicDatatype ;
              rdfs:range [ rdf:type rdfs:Datatype ;
                           owl:onDatatype xsd:long ;
                           owl:withRestrictions ( [ xsd:minExclusive "0"^^xsd:long
                                                  ]
                                                )
                         ] ;
              rdfs:comment "The precision is the number of significant bits which, unless padding is present, is 8 times larger than the value returned by size. [Allotrope]" ,
                           "precision must be a multiple of 8" ;
              rdfs:label "precision" ;
              skos:definition "The precision is the number of significant bits which, unless padding is present, is 8 times larger than the value returned by size. [Allotrope]" ;
              skos:note "Precision must be a multiple of 8. [Allotrope]" ;
              skos:prefLabel "precision" .


###  http://purl.allotrope.org/ontologies/hdf5/1.8#preserve
hdf:preserve rdf:type owl:DatatypeProperty ;
             rdfs:range xsd:boolean ;
             rdfs:label "preserve" ;
             skos:prefLabel "preserve" .


###  http://purl.allotrope.org/ontologies/hdf5/1.8#rank
hdf:rank rdf:type owl:DatatypeProperty ;
         rdfs:domain [ rdf:type owl:Class ;
                       owl:unionOf ( hdf:ArrayDatatype
                                     hdf:Dataset
                                     hdf:Dataspace
                                   )
                     ] ;
         rdfs:range [ rdf:type rdfs:Datatype ;
                      owl:onDatatype xsd:int ;
                      owl:withRestrictions ( [ xsd:minInclusive "0"^^xsd:int
                                             ]
                                             [ xsd:maxInclusive "32"^^xsd:int
                                             ]
                                           )
                    ] ;
         rdfs:label "rank" ;
         skos:prefLabel "rank" .


###  http://purl.allotrope.org/ontologies/hdf5/1.8#scaleFactor
hdf:scaleFactor rdf:type owl:DatatypeProperty ;
                rdfs:range xsd:int ;
                rdfs:label "scale factor" ;
                skos:prefLabel "scale factor" .


###  http://purl.allotrope.org/ontologies/hdf5/1.8#sharedObjectHeaderVersion
hdf:sharedObjectHeaderVersion rdf:type owl:DatatypeProperty ;
                              rdfs:domain hdf:File ;
                              rdfs:range xsd:int ;
                              rdfs:label "shared object header version" ;
                              skos:prefLabel "shared object header version" .


###  http://purl.allotrope.org/ontologies/hdf5/1.8#sieveBufferSize
hdf:sieveBufferSize rdf:type owl:DatatypeProperty ;
                    rdfs:subPropertyOf owl:topDataProperty ;
                    rdfs:range xsd:long ;
                    rdfs:label "sieve buffer size" ;
                    skos:prefLabel "sieve buffer size" .


###  http://purl.allotrope.org/ontologies/hdf5/1.8#size
hdf:size rdf:type owl:DatatypeProperty ;
         rdfs:range [ rdf:type rdfs:Datatype ;
                      owl:onDatatype xsd:long ;
                      owl:withRestrictions ( [ xsd:minInclusive "0"^^xsd:long
                                             ]
                                           )
                    ] ;
         rdfs:comment "Size of a dimension or size a datatype in bytes. For variable length strings or variable length datatypes the size is the size of the structure holding the pointer to the variable length data, not the size of the data. [HDF]" ;
         rdfs:label "size" ;
         skos:altLabel "size of datatype" ,
                       "size of dimension" ;
         skos:definition "Size of a dimension or size a datatype in bytes. For variable length strings or variable length datatypes the size is the size of the structure holding the pointer to the variable length data, not the size of the data. [HDF]" ;
         skos:prefLabel "size" .


###  http://purl.allotrope.org/ontologies/hdf5/1.8#sizeOfAddress
hdf:sizeOfAddress rdf:type owl:DatatypeProperty ;
                  rdfs:domain hdf:File ;
                  rdfs:range xsd:unsignedInt ;
                  rdfs:label "size of address" ;
                  skos:prefLabel "size of address" .


###  http://purl.allotrope.org/ontologies/hdf5/1.8#sizeOfSize
hdf:sizeOfSize rdf:type owl:DatatypeProperty ;
               rdfs:domain hdf:File ;
               rdfs:range xsd:unsignedInt ;
               rdfs:label "size of size" ;
               skos:prefLabel "size of size" .


###  http://purl.allotrope.org/ontologies/hdf5/1.8#smallDataBlockSize
hdf:smallDataBlockSize rdf:type owl:DatatypeProperty ;
                       rdfs:domain hdf:File ;
                       rdfs:range xsd:long ,
                                  xsd:nonNegativeInteger ;
                       rdfs:comment """smallDataBlockSize reserves blocks of size bytes for the contiguous storage of the raw data portion of small datasets. The HDF5 library then writes the raw data from small datasets to this reserved space, thus reducing unnecessary discontinuities within blocks of meta data and improving I/O performance.

    A small data block is actually allocated the first time a qualifying small dataset is written to the file. Space for the raw data portion of this small dataset is suballocated within the small data block. The raw data from each subsequent small dataset is also written to the small data block until it is filled; additional small data blocks are allocated as required.

    The HDF5 library employs an algorithm that determines whether I/O performance is likely to benefit from the use of this mechanism with each dataset as storage space is allocated in the file. A larger size will result in this mechanism being employed with larger datasets.

    Setting size to zero (0) disables the small data block mechanism. [HDF]""" ;
                       rdfs:label "small datablock size" ;
                       skos:definition """smallDataBlockSize reserves blocks of size bytes for the contiguous storage of the raw data portion of small datasets. The HDF5 library then writes the raw data from small datasets to this reserved space, thus reducing unnecessary discontinuities within blocks of meta data and improving I/O performance.

    A small data block is actually allocated the first time a qualifying small dataset is written to the file. Space for the raw data portion of this small dataset is suballocated within the small data block. The raw data from each subsequent small dataset is also written to the small data block until it is filled; additional small data blocks are allocated as required.

    The HDF5 library employs an algorithm that determines whether I/O performance is likely to benefit from the use of this mechanism with each dataset as storage space is allocated in the file. A larger size will result in this mechanism being employed with larger datasets.

    Setting size to zero (0) disables the small data block mechanism. [HDF]""" ;
                       skos:prefLabel "small datablock size" .


###  http://purl.allotrope.org/ontologies/hdf5/1.8#start
hdf:start rdf:type owl:DatatypeProperty ;
          rdfs:subPropertyOf hdf:index ;
          rdfs:comment "The start offset defines the origin of the hyperslab in the original dataspace. [Allotrope]" ;
          rdfs:label "start" ;
          skos:definition "The start offset defines the origin of the hyperslab in the original dataspace. [Allotrope]" ;
          skos:prefLabel "start" .


###  http://purl.allotrope.org/ontologies/hdf5/1.8#stride
hdf:stride rdf:type owl:DatatypeProperty ;
           rdfs:range [ rdf:type rdfs:Datatype ;
                        owl:onDatatype xsd:integer ;
                        owl:withRestrictions ( [ xsd:minInclusive 0
                                               ]
                                             )
                      ] ;
           rdfs:comment "The stride is the number of elements to increment between selected elements. A stride of ‘1’ is every element, a stride of ‘2’ is every second element, etc. [Allotrope]" ;
           rdfs:label "stride" ;
           skos:definition "The stride is the number of elements to increment between selected elements. A stride of ‘1’ is every element, a stride of ‘2’ is every second element, etc. [Allotrope]" ;
           skos:prefLabel "stride" .


###  http://purl.allotrope.org/ontologies/hdf5/1.8#superBlockVersion
hdf:superBlockVersion rdf:type owl:DatatypeProperty ;
                      rdfs:label "super block version" ;
                      skos:prefLabel "super block version" .


###  http://purl.allotrope.org/ontologies/hdf5/1.8#symbolTableNodeSize
hdf:symbolTableNodeSize rdf:type owl:DatatypeProperty ;
                        rdfs:domain hdf:File ;
                        rdfs:range xsd:unsignedInt ;
                        rdfs:label "symbol table node size" ;
                        skos:prefLabel "symbol table node size" .


###  http://purl.allotrope.org/ontologies/hdf5/1.8#symbolTableTreeRank
hdf:symbolTableTreeRank rdf:type owl:DatatypeProperty ;
                        rdfs:domain hdf:File ;
                        rdfs:range xsd:unsignedInt ;
                        rdfs:label "symbol table tree rank" ;
                        skos:prefLabel "symbol table tree rank" .


###  http://purl.allotrope.org/ontologies/hdf5/1.8#symbolTableVersion
hdf:symbolTableVersion rdf:type owl:DatatypeProperty ;
                       rdfs:domain hdf:File ;
                       rdfs:range xsd:int ;
                       rdfs:label "symbol table version" ;
                       skos:prefLabel "symbol table version" .


###  http://purl.allotrope.org/ontologies/hdf5/1.8#trackTimes
hdf:trackTimes rdf:type owl:DatatypeProperty ;
               rdfs:range xsd:boolean ;
               rdfs:label "track times" ;
               skos:prefLabel "track times" .


###  http://purl.allotrope.org/ontologies/hdf5/1.8#userBlockSize
hdf:userBlockSize rdf:type owl:DatatypeProperty ;
                  rdfs:domain hdf:File ;
                  rdfs:range xsd:long ;
                  rdfs:label "user block size" ;
                  skos:prefLabel "user block size" .


###  http://purl.allotrope.org/ontologies/hdf5/1.8#value
hdf:value rdf:type owl:DatatypeProperty ;
          rdfs:label "value" ;
          skos:prefLabel "value" .


#################################################################
#    Classes
#################################################################

###  http://purl.allotrope.org/ontologies/hdf5/1.8#AllSelection
hdf:AllSelection rdf:type owl:Class ;
                 rdfs:subClassOf hdf:Selection ;
                 rdfs:comment "A selection of all the datapoints in the dataspace. [Allotrope]" ;
                 rdfs:label "all selection" ;
                 skos:definition "A selection of all the datapoints in the dataspace. [Allotrope]" ;
                 skos:prefLabel "all selection" .


###  http://purl.allotrope.org/ontologies/hdf5/1.8#AndSelection
hdf:AndSelection rdf:type owl:Class ;
                 rdfs:subClassOf hdf:Selection ,
                                 [ rdf:type owl:Restriction ;
                                   owl:onProperty hdf:and ;
                                   owl:qualifiedCardinality "1"^^xsd:nonNegativeInteger ;
                                   owl:onClass hdf:Selection
                                 ] ,
                                 [ rdf:type owl:Restriction ;
                                   owl:onProperty hdf:previous ;
                                   owl:qualifiedCardinality "1"^^xsd:nonNegativeInteger ;
                                   owl:onClass hdf:Selection
                                 ] ;
                 rdfs:comment "A selection that retains only the overlapping portions of the new selection and the existing selection (Binary AND) With the HDF API this is done by calling H5Sselect_hyperslab and select operation H5S_SELECT_AND. [Allotrope]" ;
                 rdfs:label "and selection" ;
                 skos:definition "A selection that retains only the overlapping portions of the new selection and the existing selection (Binary AND) With the HDF API this is done by calling H5Sselect_hyperslab and select operation H5S_SELECT_AND. [Allotrope]" ;
                 skos:prefLabel "and selection" .


###  http://purl.allotrope.org/ontologies/hdf5/1.8#ArrayDatatype
hdf:ArrayDatatype rdf:type owl:Class ;
                  rdfs:subClassOf hdf:CompositeDatatype ,
                                  [ owl:intersectionOf ( [ rdf:type owl:Restriction ;
                                                           owl:onProperty hdf:dimension ;
                                                           owl:minQualifiedCardinality "1"^^xsd:nonNegativeInteger ;
                                                           owl:onClass hdf:ArrayDimension
                                                         ]
                                                         [ rdf:type owl:Restriction ;
                                                           owl:onProperty hdf:dimension ;
                                                           owl:maxQualifiedCardinality "32"^^xsd:nonNegativeInteger ;
                                                           owl:onClass hdf:ArrayDimension
                                                         ]
                                                       ) ;
                                    rdf:type owl:Class
                                  ] ,
                                  [ rdf:type owl:Restriction ;
                                    owl:onProperty hdf:typeClass ;
                                    owl:hasValue hdf:H5T_ARRAY
                                  ] ,
                                  [ rdf:type owl:Restriction ;
                                    owl:onProperty hdf:datatype ;
                                    owl:qualifiedCardinality "1"^^xsd:nonNegativeInteger ;
                                    owl:onClass hdf:Datatype
                                  ] ,
                                  [ rdf:type owl:Restriction ;
                                    owl:onProperty hdf:rank ;
                                    owl:qualifiedCardinality "1"^^xsd:nonNegativeInteger ;
                                    owl:onDataRange [ rdf:type rdfs:Datatype ;
                                                      owl:onDatatype xsd:integer ;
                                                      owl:withRestrictions ( [ xsd:minExclusive 0
                                                                             ]
                                                                             [ xsd:maxInclusive 32
                                                                             ]
                                                                           )
                                                    ]
                                  ] ;
                  rdfs:label "array datatype" ;
                  skos:prefLabel "array datatype" .


###  http://purl.allotrope.org/ontologies/hdf5/1.8#ArrayDimension
hdf:ArrayDimension rdf:type owl:Class ;
                   rdfs:subClassOf hdf:Dimension ,
                                   [ rdf:type owl:Restriction ;
                                     owl:onProperty hdf:size ;
                                     owl:qualifiedCardinality "1"^^xsd:nonNegativeInteger ;
                                     owl:onDataRange [ rdf:type rdfs:Datatype ;
                                                       owl:onDatatype xsd:integer ;
                                                       owl:withRestrictions ( [ xsd:minExclusive 0
                                                                              ]
                                                                            )
                                                     ]
                                   ] ;
                   rdfs:label "array dimension" ;
                   skos:prefLabel "array dimension" .


###  http://purl.allotrope.org/ontologies/hdf5/1.8#ArrayValue
hdf:ArrayValue rdf:type owl:Class ;
               rdfs:subClassOf hdf:CompositeValue ,
                               [ rdf:type owl:Restriction ;
                                 owl:onProperty hdf:member ;
                                 owl:minQualifiedCardinality "1"^^xsd:nonNegativeInteger ;
                                 owl:onClass hdf:PointValuePair
                               ] ;
               owl:disjointWith hdf:CompoundValue ;
               rdfs:comment "Value representation for arrays or variable length types. [Allotrope]" ;
               rdfs:label "array value" ;
               skos:definition "Value representation for arrays or variable length types. [Allotrope]" ;
               skos:prefLabel "array value" .


###  http://purl.allotrope.org/ontologies/hdf5/1.8#AtomicDatatype
hdf:AtomicDatatype rdf:type owl:Class ;
                   rdfs:subClassOf hdf:Datatype ;
                   owl:disjointWith hdf:CompositeDatatype ;
                   rdfs:comment "Atomic datatypes are those that are not decomposed at the datatype interface level, such as integers and floats. [Allotrope]" ;
                   rdfs:label "atomic datatype" ;
                   skos:definition "Atomic datatypes are those that are not decomposed at the datatype interface level, such as integers and floats. [Allotrope]" ;
                   skos:prefLabel "atomic datatype" .


###  http://purl.allotrope.org/ontologies/hdf5/1.8#Attribute
hdf:Attribute rdf:type owl:Class ;
              rdfs:comment "Attributes are small named datasets that are attached to primary datasets, groups, or named datatypes. Attributes can be used to describe the nature and/or the intended usage of a dataset or group. An attribute has two parts: (1) a name and (2) a value. The value part contains one or more data entries of the same datatype. [Allotrope]" ;
              rdfs:label "attribute" ;
              skos:definition "Attributes are small named datasets that are attached to primary datasets, groups, or named datatypes. Attributes can be used to describe the nature and/or the intended usage of a dataset or group. An attribute has two parts: (1) a name and (2) a value. The value part contains one or more data entries of the same datatype. [Allotrope]" ;
              skos:prefLabel "attribute" .


###  http://purl.allotrope.org/ontologies/hdf5/1.8#BitfieldDatatype
hdf:BitfieldDatatype rdf:type owl:Class ;
                     rdfs:subClassOf hdf:AtomicDatatype ,
                                     [ rdf:type owl:Restriction ;
                                       owl:onProperty hdf:typeClass ;
                                       owl:hasValue hdf:H5T_BITFIELD
                                     ] ;
                     rdfs:label "bitfield" ;
                     skos:prefLabel "bitfield" .


###  http://purl.allotrope.org/ontologies/hdf5/1.8#CharacterSet
hdf:CharacterSet rdf:type owl:Class ;
                 rdfs:label "character set" ;
                 skos:prefLabel "character set" .


###  http://purl.allotrope.org/ontologies/hdf5/1.8#Chunk
hdf:Chunk rdf:type owl:Class ;
          rdfs:subClassOf [ rdf:type owl:Restriction ;
                            owl:onProperty hdf:dimension ;
                            owl:someValuesFrom hdf:ChunkDimension
                          ] ;
          rdfs:label "chunk" ;
          skos:prefLabel "chunk" .


###  http://purl.allotrope.org/ontologies/hdf5/1.8#ChunkDimension
hdf:ChunkDimension rdf:type owl:Class ;
                   rdfs:subClassOf hdf:Dimension ;
                   rdfs:label "chunk dimension" ;
                   skos:prefLabel "chunk dimension" .


###  http://purl.allotrope.org/ontologies/hdf5/1.8#ChunkMode
hdf:ChunkMode rdf:type owl:Class ;
              rdfs:comment """ChunkMode specifies whether I/O is to be performed as linked-chunk I/O or as multi-chunk I/O. This function overrides the HDF5 Library's internal algorithm for determining which mechanism to use.

When an application uses collective I/O with chunked storage, the HDF5 Library normally uses an internal algorithm to determine whether that I/O activity should be conducted as one linked-chunk I/O or as multi-chunk I/O. ChunkMode is provided so that an application can override the library's algorithm in circumstances where the library might lack the information needed to make an optimal decision. [HDF]""" ;
              rdfs:label "chunk mode" ;
              skos:definition """ChunkMode specifies whether I/O is to be performed as linked-chunk I/O or as multi-chunk I/O. This function overrides the HDF5 Library's internal algorithm for determining which mechanism to use.

When an application uses collective I/O with chunked storage, the HDF5 Library normally uses an internal algorithm to determine whether that I/O activity should be conducted as one linked-chunk I/O or as multi-chunk I/O. ChunkMode is provided so that an application can override the library's algorithm in circumstances where the library might lack the information needed to make an optimal decision. [HDF]""" ;
              skos:prefLabel "chunk mode" .


###  http://purl.allotrope.org/ontologies/hdf5/1.8#CompositeDatatype
hdf:CompositeDatatype rdf:type owl:Class ;
                      rdfs:subClassOf hdf:Datatype ;
                      rdfs:label "composite datatype" ;
                      skos:prefLabel "composite datatype" .


###  http://purl.allotrope.org/ontologies/hdf5/1.8#CompositeValue
hdf:CompositeValue rdf:type owl:Class ;
                   owl:equivalentClass [ rdf:type owl:Class ;
                                         owl:unionOf ( hdf:ArrayValue
                                                       hdf:CompoundValue
                                                     )
                                       ] ;
                   rdfs:label "composite value" ;
                   skos:prefLabel "composite value" .


###  http://purl.allotrope.org/ontologies/hdf5/1.8#CompoundDatatype
hdf:CompoundDatatype rdf:type owl:Class ;
                     rdfs:subClassOf hdf:CompositeDatatype ,
                                     [ rdf:type owl:Restriction ;
                                       owl:onProperty hdf:typeClass ;
                                       owl:hasValue hdf:H5T_COMPOUND
                                     ] ,
                                     [ rdf:type owl:Restriction ;
                                       owl:onProperty hdf:member ;
                                       owl:minQualifiedCardinality "1"^^xsd:nonNegativeInteger ;
                                       owl:onClass hdf:CompoundDatatypeMember
                                     ] ;
                     rdfs:comment "A collection of one or more atomic types or small arrays of such types. Similar to a struct in C or a common block in Fortran. [Allotrope]" ;
                     rdfs:label "compound datatype" ;
                     skos:definition "A collection of one or more atomic types or small arrays of such types. Similar to a struct in C or a common block in Fortran. [Allotrope]" ;
                     skos:prefLabel "compound datatype" .


###  http://purl.allotrope.org/ontologies/hdf5/1.8#CompoundDatatypeMember
hdf:CompoundDatatypeMember rdf:type owl:Class ;
                           rdfs:subClassOf [ owl:intersectionOf ( [ rdf:type owl:Restriction ;
                                                                    owl:onProperty hdf:datatype ;
                                                                    owl:qualifiedCardinality "1"^^xsd:nonNegativeInteger ;
                                                                    owl:onClass hdf:Datatype
                                                                  ]
                                                                  [ rdf:type owl:Restriction ;
                                                                    owl:onProperty hdf:name ;
                                                                    owl:qualifiedCardinality "1"^^xsd:nonNegativeInteger ;
                                                                    owl:onDataRange xsd:string
                                                                  ]
                                                                ) ;
                                             rdf:type owl:Class
                                           ] ;
                           rdfs:label "compound type member" ;
                           skos:prefLabel "compound type member" .


###  http://purl.allotrope.org/ontologies/hdf5/1.8#CompoundValue
hdf:CompoundValue rdf:type owl:Class ;
                  rdfs:subClassOf hdf:CompositeValue ,
                                  [ rdf:type owl:Restriction ;
                                    owl:onProperty hdf:member ;
                                    owl:minQualifiedCardinality "1"^^xsd:nonNegativeInteger ;
                                    owl:onClass hdf:NameValuePair
                                  ] ;
                  rdfs:comment "Value representation for compound types. [Allotrope]" ;
                  rdfs:label "compound value" ;
                  skos:definition "Value representation for compound types. [Allotrope]" ;
                  skos:prefLabel "compound value" .


###  http://purl.allotrope.org/ontologies/hdf5/1.8#Coordinate
hdf:Coordinate rdf:type owl:Class ;
               rdfs:subClassOf [ rdf:type owl:Restriction ;
                                 owl:onProperty hdf:coordinateIndex ;
                                 owl:qualifiedCardinality "1"^^xsd:nonNegativeInteger ;
                                 owl:onDataRange hdf:IndexType
                               ] ,
                               [ rdf:type owl:Restriction ;
                                 owl:onProperty hdf:dimensionIndex ;
                                 owl:qualifiedCardinality "1"^^xsd:nonNegativeInteger ;
                                 owl:onDataRange hdf:DimensionIndexType
                               ] ;
               rdfs:comment "Index coordinate of a point in multi-dimensional array. [Allotrope]" ;
               rdfs:label "coordinate" ;
               skos:definition "Index coordinate of a point in multi-dimensional array. [Allotrope]" ;
               skos:prefLabel "coordinate" .


###  http://purl.allotrope.org/ontologies/hdf5/1.8#DataStream
hdf:DataStream rdf:type owl:Class ;
               rdfs:comment "A data stream represents the bitstream of data flowing from source to target. The data stream may include data conversion if datatypes of source and target differ, and may include transformations like compression or encryption. Source and targets are hyperslabs on datasets. [Allotrope]" ;
               rdfs:label "data stream" ;
               skos:definition "A data stream represents the bitstream of data flowing from source to target. The data stream may include data conversion if datatypes of source and target differ, and may include transformations like compression or encryption. Source and targets are hyperslabs on datasets. [Allotrope]" ;
               skos:prefLabel "data stream" .


###  http://purl.allotrope.org/ontologies/hdf5/1.8#Dataset
hdf:Dataset rdf:type owl:Class ;
            rdfs:subClassOf hdf:NamedObject ,
                            [ rdf:type owl:Restriction ;
                              owl:onProperty hdf:dataspace ;
                              owl:qualifiedCardinality "1"^^xsd:nonNegativeInteger ;
                              owl:onClass hdf:Dataspace
                            ] ,
                            [ rdf:type owl:Restriction ;
                              owl:onProperty hdf:layout ;
                              owl:qualifiedCardinality "1"^^xsd:nonNegativeInteger ;
                              owl:onClass hdf:StorageLayout
                            ] ,
                            [ rdf:type owl:Restriction ;
                              owl:onProperty hdf:writtenRegion ;
                              owl:qualifiedCardinality "1"^^xsd:nonNegativeInteger ;
                              owl:onClass hdf:Selection
                            ] ,
                            [ rdf:type owl:Restriction ;
                              owl:onProperty hdf:rank ;
                              owl:qualifiedCardinality "1"^^xsd:nonNegativeInteger ;
                              owl:onDataRange [ rdf:type rdfs:Datatype ;
                                                owl:onDatatype xsd:integer ;
                                                owl:withRestrictions ( [ xsd:minInclusive 0
                                                                       ]
                                                                       [ xsd:maxInclusive 32
                                                                       ]
                                                                     )
                                              ]
                            ] ;
            owl:disjointWith hdf:Group ;
            rdfs:comment "A multi-dimensional array of data elements, together with supporting metadata. [Allotrope]" ;
            rdfs:label "dataset" ;
            skos:definition "A multi-dimensional array of data elements, together with supporting metadata. [Allotrope]" ;
            skos:prefLabel "dataset" .


###  http://purl.allotrope.org/ontologies/hdf5/1.8#Dataspace
hdf:Dataspace rdf:type owl:Class ;
              rdfs:subClassOf [ rdf:type owl:Restriction ;
                                owl:onProperty hdf:dimension ;
                                owl:maxQualifiedCardinality "32"^^xsd:nonNegativeInteger ;
                                owl:onClass hdf:DataspaceDimension
                              ] ,
                              [ rdf:type owl:Restriction ;
                                owl:onProperty hdf:rank ;
                                owl:qualifiedCardinality "1"^^xsd:nonNegativeInteger ;
                                owl:onDataRange [ rdf:type rdfs:Datatype ;
                                                  owl:onDatatype xsd:int ;
                                                  owl:withRestrictions ( [ xsd:minInclusive "0"^^xsd:int
                                                                         ]
                                                                         [ xsd:maxInclusive "32"^^xsd:int
                                                                         ]
                                                                       )
                                                ]
                              ] ;
              rdfs:comment "A dataset dataspace describes the dimensionality of the dataset. The dimensions of a dataset can be fixed (unchanging), or they may be unlimited, which means that they are extendible (i.e. they can grow larger). [Allotrope]" ;
              rdfs:label "dataspace" ;
              skos:definition "A dataset dataspace describes the dimensionality of the dataset. The dimensions of a dataset can be fixed (unchanging), or they may be unlimited, which means that they are extendible (i.e. they can grow larger). [Allotrope]" ;
              skos:prefLabel "dataspace" .


###  http://purl.allotrope.org/ontologies/hdf5/1.8#DataspaceDimension
hdf:DataspaceDimension rdf:type owl:Class ;
                       rdfs:subClassOf hdf:Dimension ,
                                       [ rdf:type owl:Restriction ;
                                         owl:onProperty hdf:initialSize ;
                                         owl:qualifiedCardinality "1"^^xsd:nonNegativeInteger ;
                                         owl:onDataRange [ rdf:type rdfs:Datatype ;
                                                           owl:onDatatype xsd:int ;
                                                           owl:withRestrictions ( [ xsd:minInclusive 0
                                                                                  ]
                                                                                )
                                                         ]
                                       ] ,
                                       [ rdf:type owl:Restriction ;
                                         owl:onProperty hdf:currentSize ;
                                         owl:maxQualifiedCardinality "1"^^xsd:nonNegativeInteger ;
                                         owl:onDataRange [ rdf:type rdfs:Datatype ;
                                                           owl:onDatatype xsd:integer ;
                                                           owl:withRestrictions ( [ xsd:minInclusive "0"^^xsd:int
                                                                                  ]
                                                                                )
                                                         ]
                                       ] ,
                                       [ rdf:type owl:Restriction ;
                                         owl:onProperty hdf:maximumSize ;
                                         owl:maxQualifiedCardinality "1"^^xsd:nonNegativeInteger ;
                                         owl:onDataRange [ rdf:type rdfs:Datatype ;
                                                           owl:onDatatype xsd:integer ;
                                                           owl:withRestrictions ( [ xsd:minInclusive -1
                                                                                  ]
                                                                                )
                                                         ]
                                       ] ;
                       rdfs:label "dataspace dimension" ;
                       skos:prefLabel "dataspace dimension" .


###  http://purl.allotrope.org/ontologies/hdf5/1.8#Datatype
hdf:Datatype rdf:type owl:Class ;
             rdfs:subClassOf [ rdf:type owl:Restriction ;
                               owl:onProperty hdf:typeClass ;
                               owl:qualifiedCardinality "1"^^xsd:nonNegativeInteger ;
                               owl:onClass hdf:TypeClass
                             ] ;
             rdfs:comment "An object that describes the storage format of the individual data points in a data set. There are two categories of datatypes: atomic and compound datatypes. An atomic type is a type which cannot be decomposed into smaller units at the API level. A compound datatype is a collection of one or more atomic types or small arrays of such types. [Allotrope]" ;
             rdfs:label "datatype" ;
             skos:definition "An object that describes the storage format of the individual data points in a data set. There are two categories of datatypes: atomic and compound datatypes. An atomic type is a type which cannot be decomposed into smaller units at the API level. A compound datatype is a collection of one or more atomic types or small arrays of such types. [Allotrope]" ;
             skos:prefLabel "datatype" .


###  http://purl.allotrope.org/ontologies/hdf5/1.8#Dimension
hdf:Dimension rdf:type owl:Class ;
              rdfs:subClassOf [ rdf:type owl:Restriction ;
                                owl:onProperty hdf:size ;
                                owl:someValuesFrom [ rdf:type rdfs:Datatype ;
                                                     owl:onDatatype xsd:integer ;
                                                     owl:withRestrictions ( [ xsd:minInclusive 0
                                                                            ]
                                                                          )
                                                   ]
                              ] ,
                              [ rdf:type owl:Restriction ;
                                owl:onProperty hdf:dimensionIndex ;
                                owl:qualifiedCardinality "1"^^xsd:nonNegativeInteger ;
                                owl:onDataRange hdf:DimensionIndexType
                              ] ;
              rdfs:label "dimension" ;
              skos:prefLabel "dimension" .


###  http://purl.allotrope.org/ontologies/hdf5/1.8#DimensionSelection
hdf:DimensionSelection rdf:type owl:Class ;
                       rdfs:label "dimension selection" ;
                       skos:prefLabel "dimension selection" .


###  http://purl.allotrope.org/ontologies/hdf5/1.8#EnumerationDatatype
hdf:EnumerationDatatype rdf:type owl:Class ;
                        rdfs:subClassOf hdf:CompositeDatatype ,
                                        [ rdf:type owl:Restriction ;
                                          owl:onProperty hdf:typeClass ;
                                          owl:hasValue hdf:H5T_ENUM
                                        ] ,
                                        [ rdf:type owl:Restriction ;
                                          owl:onProperty hdf:member ;
                                          owl:minQualifiedCardinality "1"^^xsd:nonNegativeInteger ;
                                          owl:onClass hdf:EnumerationDatatypeMember
                                        ] ;
                        rdfs:comment "A one-to-one mapping between a set of symbols and a set of integer values, and an order is imposed on the symbols by their integer values. The symbols are passed between the application and library as character strings and all the values for a particular enumeration datatype are of the same integer type, which is not necessary a native type. [Allotrope]" ;
                        rdfs:label "enumeration datatype" ;
                        skos:definition "A one-to-one mapping between a set of symbols and a set of integer values, and an order is imposed on the symbols by their integer values. The symbols are passed between the application and library as character strings and all the values for a particular enumeration datatype are of the same integer type, which is not necessary a native type. [Allotrope]" ;
                        skos:prefLabel "enumeration datatype" .


###  http://purl.allotrope.org/ontologies/hdf5/1.8#EnumerationDatatypeMember
hdf:EnumerationDatatypeMember rdf:type owl:Class ;
                              rdfs:subClassOf [ rdf:type owl:Restriction ;
                                                owl:onProperty hdf:name ;
                                                owl:qualifiedCardinality "1"^^xsd:nonNegativeInteger ;
                                                owl:onDataRange xsd:string
                                              ] ,
                                              [ rdf:type owl:Restriction ;
                                                owl:onProperty hdf:value ;
                                                owl:qualifiedCardinality "1"^^xsd:nonNegativeInteger ;
                                                owl:onDataRange xsd:integer
                                              ] ;
                              rdfs:label "enumeration type member" ;
                              skos:prefLabel "enumeration type member" .


###  http://purl.allotrope.org/ontologies/hdf5/1.8#ErrorDetectionCheck
hdf:ErrorDetectionCheck rdf:type owl:Class ;
                        rdfs:label "error detection check" ;
                        skos:prefLabel "error detection check" .


###  http://purl.allotrope.org/ontologies/hdf5/1.8#ExponentField
hdf:ExponentField rdf:type owl:Class ;
                  rdfs:subClassOf hdf:FieldSpecification ;
                  rdfs:label "exponent field" ;
                  skos:prefLabel "exponent field" .


###  http://purl.allotrope.org/ontologies/hdf5/1.8#ExternalFile
hdf:ExternalFile rdf:type owl:Class ;
                 rdfs:label "external file" ;
                 skos:prefLabel "external file" .


###  http://purl.allotrope.org/ontologies/hdf5/1.8#FieldSpecification
hdf:FieldSpecification rdf:type owl:Class ;
                       rdfs:subClassOf [ rdf:type owl:Restriction ;
                                         owl:onProperty hdf:size ;
                                         owl:qualifiedCardinality "1"^^xsd:nonNegativeInteger ;
                                         owl:onDataRange [ rdf:type rdfs:Datatype ;
                                                           owl:onDatatype xsd:integer ;
                                                           owl:withRestrictions ( [ xsd:minInclusive 0
                                                                                  ]
                                                                                )
                                                         ]
                                       ] ;
                       rdfs:label "field specialization" ;
                       skos:prefLabel "field specialization" .


###  http://purl.allotrope.org/ontologies/hdf5/1.8#File
hdf:File rdf:type owl:Class ;
         rdfs:subClassOf [ rdf:type owl:Restriction ;
                           owl:onProperty hdf:rootGroup ;
                           owl:qualifiedCardinality "1"^^xsd:nonNegativeInteger ;
                           owl:onClass hdf:Group
                         ] ;
         rdfs:comment "A container for storing grouped collections of multi-dimensional arrays containing scientific data following the HDF 5 specification. [Allotrope]" ;
         rdfs:label "file" ;
         skos:altLabel "HDF 5 file" ;
         skos:definition "A container for storing grouped collections of multi-dimensional arrays containing scientific data following the HDF 5 specification. [Allotrope]" ;
         skos:prefLabel "file" .


###  http://purl.allotrope.org/ontologies/hdf5/1.8#FileAccessMode
hdf:FileAccessMode rdf:type owl:Class ;
                   rdfs:comment "Determines whether an existing file will be overwritten, opened for read-only access, or opened for read/write access. All newly created files are opened for both reading and writing. [Allotrope]" ;
                   rdfs:label "file access mode" ;
                   skos:definition "Determines whether an existing file will be overwritten, opened for read-only access, or opened for read/write access. All newly created files are opened for both reading and writing. [Allotrope]" ;
                   skos:prefLabel "file access mode" .


###  http://purl.allotrope.org/ontologies/hdf5/1.8#FillTime
hdf:FillTime rdf:type owl:Class ;
             rdfs:label "fill time" ;
             skos:prefLabel "fill time" .


###  http://purl.allotrope.org/ontologies/hdf5/1.8#FillValueStatus
hdf:FillValueStatus rdf:type owl:Class ;
                    rdfs:label "fill value status" ;
                    skos:prefLabel "fill value status" .


###  http://purl.allotrope.org/ontologies/hdf5/1.8#Filter
hdf:Filter rdf:type owl:Class ;
           rdfs:label "filter" ;
           skos:prefLabel "filter" .


###  http://purl.allotrope.org/ontologies/hdf5/1.8#FilterDefault
hdf:FilterDefault rdf:type owl:Class ;
                  rdfs:subClassOf hdf:Filter ;
                  rdfs:label "default filter" ;
                  skos:prefLabel "default filter" .


###  http://purl.allotrope.org/ontologies/hdf5/1.8#FilterDeflate
hdf:FilterDeflate rdf:type owl:Class ;
                  rdfs:subClassOf hdf:Filter ;
                  rdfs:label "deflate filter" ;
                  skos:prefLabel "deflate filter" .


###  http://purl.allotrope.org/ontologies/hdf5/1.8#FilterFletcher
hdf:FilterFletcher rdf:type owl:Class ;
                   rdfs:subClassOf hdf:Filter ;
                   rdfs:label "Fletcher filter" ;
                   skos:prefLabel "Fletcher filter" .


###  http://purl.allotrope.org/ontologies/hdf5/1.8#FilterNBit
hdf:FilterNBit rdf:type owl:Class ;
               rdfs:subClassOf hdf:Filter ;
               rdfs:label "NBit filter" ;
               skos:prefLabel "NBit filter" .


###  http://purl.allotrope.org/ontologies/hdf5/1.8#FilterSZip
hdf:FilterSZip rdf:type owl:Class ;
               rdfs:subClassOf hdf:Filter ;
               rdfs:label "SZip filter" ;
               skos:prefLabel "SZip filter" .


###  http://purl.allotrope.org/ontologies/hdf5/1.8#FilterScaleOffset
hdf:FilterScaleOffset rdf:type owl:Class ;
                      rdfs:subClassOf hdf:Filter ;
                      rdfs:label "scale offset filter" ;
                      skos:prefLabel "scale offset filter" .


###  http://purl.allotrope.org/ontologies/hdf5/1.8#FilterShuffle
hdf:FilterShuffle rdf:type owl:Class ;
                  rdfs:subClassOf hdf:Filter ;
                  rdfs:label "shuffle filter" ;
                  skos:prefLabel "shuffle filter" .


###  http://purl.allotrope.org/ontologies/hdf5/1.8#FloatAttribute
hdf:FloatAttribute rdf:type owl:Class ;
                   rdfs:subClassOf hdf:Attribute ;
                   rdfs:label "float attribute" ;
                   skos:prefLabel "float attribute" .


###  http://purl.allotrope.org/ontologies/hdf5/1.8#FloatDatatype
hdf:FloatDatatype rdf:type owl:Class ;
                  rdfs:subClassOf hdf:AtomicDatatype ,
                                  [ rdf:type owl:Restriction ;
                                    owl:onProperty hdf:typeClass ;
                                    owl:hasValue hdf:H5T_FLOAT
                                  ] ;
                  rdfs:label "float" ;
                  skos:prefLabel "float" .


###  http://purl.allotrope.org/ontologies/hdf5/1.8#FloatingPointNormalization
hdf:FloatingPointNormalization rdf:type owl:Class ;
                               rdfs:label "floating-point normalization" ;
                               skos:prefLabel "floating-point normalization" .


###  http://purl.allotrope.org/ontologies/hdf5/1.8#Group
hdf:Group rdf:type owl:Class ;
          rdfs:subClassOf hdf:NamedObject ;
          rdfs:comment "A grouping structure containing instances of zero or more groups or datasets, together with supporting metadata. [Allotrope]" ;
          rdfs:label "group" ;
          skos:definition "A grouping structure containing instances of zero or more groups or datasets, together with supporting metadata. [Allotrope]" ;
          skos:prefLabel "group" .


###  http://purl.allotrope.org/ontologies/hdf5/1.8#HardLink
hdf:HardLink rdf:type owl:Class ;
             rdfs:subClassOf hdf:Link ,
                             [ rdf:type owl:Restriction ;
                               owl:onProperty hdf:linkedTo ;
                               owl:qualifiedCardinality "1"^^xsd:nonNegativeInteger ;
                               owl:onClass hdf:NamedObject
                             ] ;
             rdfs:comment "A direct association between a name and the object where both exist in a single HDF5 address space. [Allotrope]" ;
             rdfs:label "hard link" ;
             skos:definition "A direct association between a name and the object where both exist in a single HDF5 address space. [Allotrope]" ;
             skos:prefLabel "hard link" .


###  http://purl.allotrope.org/ontologies/hdf5/1.8#HyperSlab
hdf:HyperSlab rdf:type owl:Class ;
              rdfs:subClassOf hdf:Selection ;
              rdfs:comment "A portion of a dataset. A hyperslab selection can be a logically contiguous collection of points in a dataspace or a regular pattern of points or blocks in a dataspace. [Allotrope]" ;
              rdfs:label "hyperslab" ;
              skos:definition "A portion of a dataset. A hyperslab selection can be a logically contiguous collection of points in a dataspace or a regular pattern of points or blocks in a dataspace. [Allotrope]" ;
              skos:prefLabel "hyperslab" .


###  http://purl.allotrope.org/ontologies/hdf5/1.8#IntegerAttribute
hdf:IntegerAttribute rdf:type owl:Class ;
                     rdfs:subClassOf hdf:Attribute ;
                     rdfs:label "integer attribute" ;
                     skos:prefLabel "integer attribute" .


###  http://purl.allotrope.org/ontologies/hdf5/1.8#IntegerDatatype
hdf:IntegerDatatype rdf:type owl:Class ;
                    rdfs:subClassOf hdf:AtomicDatatype ,
                                    [ rdf:type owl:Restriction ;
                                      owl:onProperty hdf:typeClass ;
                                      owl:hasValue hdf:H5T_INTEGER
                                    ] ;
                    rdfs:label "integer" ;
                    skos:prefLabel "integer" .


###  http://purl.allotrope.org/ontologies/hdf5/1.8#Link
hdf:Link rdf:type owl:Class ;
         rdfs:comment "An association between a name and the object in an HDF5 file group. [Allotrope]" ;
         rdfs:label "link" ;
         skos:prefLabel "link" .


###  http://purl.allotrope.org/ontologies/hdf5/1.8#MantissaField
hdf:MantissaField rdf:type owl:Class ;
                  rdfs:subClassOf hdf:FieldSpecification ;
                  rdfs:label "mantissa field" ;
                  skos:prefLabel "mantissa field" .


###  http://purl.allotrope.org/ontologies/hdf5/1.8#MessageTypeFlag
hdf:MessageTypeFlag rdf:type owl:Class ;
                    rdfs:label "message time flag" ;
                    skos:prefLabel "message time flag" .


###  http://purl.allotrope.org/ontologies/hdf5/1.8#NameValuePair
hdf:NameValuePair rdf:type owl:Class ;
                  rdfs:subClassOf [ rdf:type owl:Class ;
                                    owl:unionOf ( [ owl:intersectionOf ( [ rdf:type owl:Restriction ;
                                                                           owl:onProperty hdf:compositeValue ;
                                                                           owl:maxQualifiedCardinality "0"^^xsd:nonNegativeInteger ;
                                                                           owl:onClass hdf:CompositeValue
                                                                         ]
                                                                         [ rdf:type owl:Restriction ;
                                                                           owl:onProperty hdf:value ;
                                                                           owl:maxQualifiedCardinality "1"^^xsd:nonNegativeInteger ;
                                                                           owl:onDataRange rdf:Literal
                                                                         ]
                                                                       ) ;
                                                    rdf:type owl:Class
                                                  ]
                                                  [ owl:intersectionOf ( [ rdf:type owl:Restriction ;
                                                                           owl:onProperty hdf:compositeValue ;
                                                                           owl:maxQualifiedCardinality "1"^^xsd:nonNegativeInteger ;
                                                                           owl:onClass hdf:CompositeValue
                                                                         ]
                                                                         [ rdf:type owl:Restriction ;
                                                                           owl:onProperty hdf:value ;
                                                                           owl:maxQualifiedCardinality "0"^^xsd:nonNegativeInteger ;
                                                                           owl:onDataRange rdf:Literal
                                                                         ]
                                                                       ) ;
                                                    rdf:type owl:Class
                                                  ]
                                                )
                                  ] ,
                                  [ rdf:type owl:Restriction ;
                                    owl:onProperty hdf:name ;
                                    owl:qualifiedCardinality "1"^^xsd:nonNegativeInteger ;
                                    owl:onDataRange xsd:string
                                  ] ;
                  rdfs:label "name-value pair" ;
                  skos:prefLabel "name-value pair" .


###  http://purl.allotrope.org/ontologies/hdf5/1.8#NamedDatatype
hdf:NamedDatatype rdf:type owl:Class ;
                  rdfs:subClassOf hdf:Datatype ,
                                  hdf:NamedObject ;
                  rdfs:comment "Named datatypes are either atomic or compound datatypes that have been specifically designated to be shared across datasets. [Allotrope]" ;
                  rdfs:label "named datatype" ;
                  skos:definition "Named datatypes are either atomic or compound datatypes that have been specifically designated to be shared across datasets. [Allotrope]" ;
                  skos:prefLabel "named datatype" .


###  http://purl.allotrope.org/ontologies/hdf5/1.8#NamedObject
hdf:NamedObject rdf:type owl:Class ;
                rdfs:subClassOf [ rdf:type owl:Restriction ;
                                  owl:onProperty hdf:name ;
                                  owl:maxQualifiedCardinality "1"^^xsd:nonNegativeInteger ;
                                  owl:onDataRange xsd:string
                                ] ;
                rdfs:label "named object" ;
                skos:prefLabel "named object" .


###  http://purl.allotrope.org/ontologies/hdf5/1.8#NoneSelection
hdf:NoneSelection rdf:type owl:Class ;
                  rdfs:subClassOf hdf:Selection ;
                  rdfs:label "none selection" ;
                  skos:prefLabel "none selection" .


###  http://purl.allotrope.org/ontologies/hdf5/1.8#NotASelection
hdf:NotASelection rdf:type owl:Class ;
                  rdfs:subClassOf hdf:Selection ,
                                  [ rdf:type owl:Restriction ;
                                    owl:onProperty hdf:notA ;
                                    owl:qualifiedCardinality "1"^^xsd:nonNegativeInteger ;
                                    owl:onClass hdf:Selection
                                  ] ,
                                  [ rdf:type owl:Restriction ;
                                    owl:onProperty hdf:previous ;
                                    owl:qualifiedCardinality "1"^^xsd:nonNegativeInteger ;
                                    owl:onClass hdf:Selection
                                  ] ;
                  rdfs:label "not A selection" ;
                  skos:prefLabel "not A selection" .


###  http://purl.allotrope.org/ontologies/hdf5/1.8#NotBSelection
hdf:NotBSelection rdf:type owl:Class ;
                  rdfs:subClassOf hdf:Selection ,
                                  [ rdf:type owl:Restriction ;
                                    owl:onProperty hdf:notB ;
                                    owl:qualifiedCardinality "1"^^xsd:nonNegativeInteger ;
                                    owl:onClass hdf:Selection
                                  ] ,
                                  [ rdf:type owl:Restriction ;
                                    owl:onProperty hdf:previous ;
                                    owl:qualifiedCardinality "1"^^xsd:nonNegativeInteger ;
                                    owl:onClass hdf:Selection
                                  ] ;
                  rdfs:label "not B selection" ;
                  skos:prefLabel "not B selection" .


###  http://purl.allotrope.org/ontologies/hdf5/1.8#OpaqueAttribute
hdf:OpaqueAttribute rdf:type owl:Class ;
                    rdfs:subClassOf hdf:Attribute ;
                    rdfs:label "opaque attribute" ;
                    skos:prefLabel "opaque attribute" .


###  http://purl.allotrope.org/ontologies/hdf5/1.8#OpaqueDatatype
hdf:OpaqueDatatype rdf:type owl:Class ;
                   rdfs:subClassOf hdf:AtomicDatatype ,
                                   [ rdf:type owl:Restriction ;
                                     owl:onProperty hdf:typeClass ;
                                     owl:hasValue hdf:H5T_OPAQUE
                                   ] ;
                   rdfs:comment "A mechanism for describing data which cannot be otherwise described by HDF5. The only properties associated with opaque types are a size in bytes and an ASCII tag. [Allotrope]" ;
                   rdfs:label "opaque datatype" ;
                   skos:definition "A mechanism for describing data which cannot be otherwise described by HDF5. The only properties associated with opaque types are a size in bytes and an ASCII tag. [Allotrope]" ;
                   skos:prefLabel "opaque datatype" .


###  http://purl.allotrope.org/ontologies/hdf5/1.8#OrSelection
hdf:OrSelection rdf:type owl:Class ;
                rdfs:subClassOf hdf:Selection ,
                                [ rdf:type owl:Restriction ;
                                  owl:onProperty hdf:or ;
                                  owl:qualifiedCardinality "1"^^xsd:nonNegativeInteger ;
                                  owl:onClass hdf:Selection
                                ] ,
                                [ rdf:type owl:Restriction ;
                                  owl:onProperty hdf:previous ;
                                  owl:qualifiedCardinality "1"^^xsd:nonNegativeInteger ;
                                  owl:onClass hdf:Selection
                                ] ;
                rdfs:label "or selection" ;
                skos:prefLabel "or selection" .


###  http://purl.allotrope.org/ontologies/hdf5/1.8#Order
hdf:Order rdf:type owl:Class ;
          rdfs:label "order" ;
          skos:prefLabel "order" .


###  http://purl.allotrope.org/ontologies/hdf5/1.8#Padding
hdf:Padding rdf:type owl:Class ;
            rdfs:label "padding" ;
            skos:prefLabel "padding" .


###  http://purl.allotrope.org/ontologies/hdf5/1.8#Point
hdf:Point rdf:type owl:Class ;
          rdfs:subClassOf [ rdf:type owl:Restriction ;
                            owl:onProperty hdf:coordinate ;
                            owl:maxQualifiedCardinality "32"^^xsd:nonNegativeInteger ;
                            owl:onClass hdf:Coordinate
                          ] ,
                          [ rdf:type owl:Restriction ;
                            owl:onProperty hdf:index_0 ;
                            owl:maxQualifiedCardinality "1"^^xsd:nonNegativeInteger ;
                            owl:onDataRange hdf:IndexType
                          ] ,
                          [ rdf:type owl:Restriction ;
                            owl:onProperty hdf:index_1 ;
                            owl:maxQualifiedCardinality "1"^^xsd:nonNegativeInteger ;
                            owl:onDataRange hdf:IndexType
                          ] ,
                          [ rdf:type owl:Restriction ;
                            owl:onProperty hdf:index_10 ;
                            owl:maxQualifiedCardinality "1"^^xsd:nonNegativeInteger ;
                            owl:onDataRange hdf:IndexType
                          ] ,
                          [ rdf:type owl:Restriction ;
                            owl:onProperty hdf:index_11 ;
                            owl:maxQualifiedCardinality "1"^^xsd:nonNegativeInteger ;
                            owl:onDataRange hdf:IndexType
                          ] ,
                          [ rdf:type owl:Restriction ;
                            owl:onProperty hdf:index_12 ;
                            owl:maxQualifiedCardinality "1"^^xsd:nonNegativeInteger ;
                            owl:onDataRange hdf:IndexType
                          ] ,
                          [ rdf:type owl:Restriction ;
                            owl:onProperty hdf:index_13 ;
                            owl:maxQualifiedCardinality "1"^^xsd:nonNegativeInteger ;
                            owl:onDataRange hdf:IndexType
                          ] ,
                          [ rdf:type owl:Restriction ;
                            owl:onProperty hdf:index_14 ;
                            owl:maxQualifiedCardinality "1"^^xsd:nonNegativeInteger ;
                            owl:onDataRange hdf:IndexType
                          ] ,
                          [ rdf:type owl:Restriction ;
                            owl:onProperty hdf:index_15 ;
                            owl:maxQualifiedCardinality "1"^^xsd:nonNegativeInteger ;
                            owl:onDataRange hdf:IndexType
                          ] ,
                          [ rdf:type owl:Restriction ;
                            owl:onProperty hdf:index_16 ;
                            owl:maxQualifiedCardinality "1"^^xsd:nonNegativeInteger ;
                            owl:onDataRange hdf:IndexType
                          ] ,
                          [ rdf:type owl:Restriction ;
                            owl:onProperty hdf:index_17 ;
                            owl:maxQualifiedCardinality "1"^^xsd:nonNegativeInteger ;
                            owl:onDataRange hdf:IndexType
                          ] ,
                          [ rdf:type owl:Restriction ;
                            owl:onProperty hdf:index_18 ;
                            owl:maxQualifiedCardinality "1"^^xsd:nonNegativeInteger ;
                            owl:onDataRange hdf:IndexType
                          ] ,
                          [ rdf:type owl:Restriction ;
                            owl:onProperty hdf:index_19 ;
                            owl:maxQualifiedCardinality "1"^^xsd:nonNegativeInteger ;
                            owl:onDataRange hdf:IndexType
                          ] ,
                          [ rdf:type owl:Restriction ;
                            owl:onProperty hdf:index_2 ;
                            owl:maxQualifiedCardinality "1"^^xsd:nonNegativeInteger ;
                            owl:onDataRange hdf:IndexType
                          ] ,
                          [ rdf:type owl:Restriction ;
                            owl:onProperty hdf:index_20 ;
                            owl:maxQualifiedCardinality "1"^^xsd:nonNegativeInteger ;
                            owl:onDataRange hdf:IndexType
                          ] ,
                          [ rdf:type owl:Restriction ;
                            owl:onProperty hdf:index_21 ;
                            owl:maxQualifiedCardinality "1"^^xsd:nonNegativeInteger ;
                            owl:onDataRange hdf:IndexType
                          ] ,
                          [ rdf:type owl:Restriction ;
                            owl:onProperty hdf:index_22 ;
                            owl:maxQualifiedCardinality "1"^^xsd:nonNegativeInteger ;
                            owl:onDataRange hdf:IndexType
                          ] ,
                          [ rdf:type owl:Restriction ;
                            owl:onProperty hdf:index_23 ;
                            owl:maxQualifiedCardinality "1"^^xsd:nonNegativeInteger ;
                            owl:onDataRange hdf:IndexType
                          ] ,
                          [ rdf:type owl:Restriction ;
                            owl:onProperty hdf:index_24 ;
                            owl:maxQualifiedCardinality "1"^^xsd:nonNegativeInteger ;
                            owl:onDataRange hdf:IndexType
                          ] ,
                          [ rdf:type owl:Restriction ;
                            owl:onProperty hdf:index_25 ;
                            owl:maxQualifiedCardinality "1"^^xsd:nonNegativeInteger ;
                            owl:onDataRange hdf:IndexType
                          ] ,
                          [ rdf:type owl:Restriction ;
                            owl:onProperty hdf:index_26 ;
                            owl:maxQualifiedCardinality "1"^^xsd:nonNegativeInteger ;
                            owl:onDataRange hdf:IndexType
                          ] ,
                          [ rdf:type owl:Restriction ;
                            owl:onProperty hdf:index_27 ;
                            owl:maxQualifiedCardinality "1"^^xsd:nonNegativeInteger ;
                            owl:onDataRange hdf:IndexType
                          ] ,
                          [ rdf:type owl:Restriction ;
                            owl:onProperty hdf:index_28 ;
                            owl:maxQualifiedCardinality "1"^^xsd:nonNegativeInteger ;
                            owl:onDataRange hdf:IndexType
                          ] ,
                          [ rdf:type owl:Restriction ;
                            owl:onProperty hdf:index_29 ;
                            owl:maxQualifiedCardinality "1"^^xsd:nonNegativeInteger ;
                            owl:onDataRange hdf:IndexType
                          ] ,
                          [ rdf:type owl:Restriction ;
                            owl:onProperty hdf:index_3 ;
                            owl:maxQualifiedCardinality "1"^^xsd:nonNegativeInteger ;
                            owl:onDataRange hdf:IndexType
                          ] ,
                          [ rdf:type owl:Restriction ;
                            owl:onProperty hdf:index_30 ;
                            owl:maxQualifiedCardinality "1"^^xsd:nonNegativeInteger ;
                            owl:onDataRange hdf:IndexType
                          ] ,
                          [ rdf:type owl:Restriction ;
                            owl:onProperty hdf:index_31 ;
                            owl:maxQualifiedCardinality "1"^^xsd:nonNegativeInteger ;
                            owl:onDataRange hdf:IndexType
                          ] ,
                          [ rdf:type owl:Restriction ;
                            owl:onProperty hdf:index_4 ;
                            owl:maxQualifiedCardinality "1"^^xsd:nonNegativeInteger ;
                            owl:onDataRange hdf:IndexType
                          ] ,
                          [ rdf:type owl:Restriction ;
                            owl:onProperty hdf:index_5 ;
                            owl:maxQualifiedCardinality "1"^^xsd:nonNegativeInteger ;
                            owl:onDataRange hdf:IndexType
                          ] ,
                          [ rdf:type owl:Restriction ;
                            owl:onProperty hdf:index_6 ;
                            owl:maxQualifiedCardinality "1"^^xsd:nonNegativeInteger ;
                            owl:onDataRange hdf:IndexType
                          ] ,
                          [ rdf:type owl:Restriction ;
                            owl:onProperty hdf:index_7 ;
                            owl:maxQualifiedCardinality "1"^^xsd:nonNegativeInteger ;
                            owl:onDataRange hdf:IndexType
                          ] ,
                          [ rdf:type owl:Restriction ;
                            owl:onProperty hdf:index_8 ;
                            owl:maxQualifiedCardinality "1"^^xsd:nonNegativeInteger ;
                            owl:onDataRange hdf:IndexType
                          ] ,
                          [ rdf:type owl:Restriction ;
                            owl:onProperty hdf:index_9 ;
                            owl:maxQualifiedCardinality "1"^^xsd:nonNegativeInteger ;
                            owl:onDataRange hdf:IndexType
                          ] ;
          rdfs:comment "Addresses a point in the dataspace. [Allotrope]" ;
          rdfs:label "point" ;
          skos:definition "Addresses a point in the dataspace. [Allotrope]" ;
          skos:prefLabel "point" .


###  http://purl.allotrope.org/ontologies/hdf5/1.8#PointSelection
hdf:PointSelection rdf:type owl:Class ;
                   rdfs:subClassOf hdf:Selection ,
                                   [ rdf:type owl:Restriction ;
                                     owl:onProperty hdf:point ;
                                     owl:someValuesFrom hdf:Point
                                   ] ;
                   rdfs:comment "A selection of individual datapoints in the dataspace. [Allotrope]" ;
                   rdfs:label "point selection" ;
                   skos:definition "A selection of individual datapoints in the dataspace. [Allotrope]" ;
                   skos:prefLabel "point selection" .


###  http://purl.allotrope.org/ontologies/hdf5/1.8#PointValuePair
hdf:PointValuePair rdf:type owl:Class ;
                   rdfs:subClassOf [ rdf:type owl:Class ;
                                     owl:unionOf ( [ owl:intersectionOf ( [ rdf:type owl:Restriction ;
                                                                            owl:onProperty hdf:compositeValue ;
                                                                            owl:maxQualifiedCardinality "0"^^xsd:nonNegativeInteger ;
                                                                            owl:onClass hdf:CompositeValue
                                                                          ]
                                                                          [ rdf:type owl:Restriction ;
                                                                            owl:onProperty hdf:value ;
                                                                            owl:maxQualifiedCardinality "1"^^xsd:nonNegativeInteger ;
                                                                            owl:onDataRange rdf:Literal
                                                                          ]
                                                                        ) ;
                                                     rdf:type owl:Class
                                                   ]
                                                   [ owl:intersectionOf ( [ rdf:type owl:Restriction ;
                                                                            owl:onProperty hdf:compositeValue ;
                                                                            owl:maxQualifiedCardinality "1"^^xsd:nonNegativeInteger ;
                                                                            owl:onClass hdf:CompositeValue
                                                                          ]
                                                                          [ rdf:type owl:Restriction ;
                                                                            owl:onProperty hdf:value ;
                                                                            owl:maxQualifiedCardinality "0"^^xsd:nonNegativeInteger ;
                                                                            owl:onDataRange rdf:Literal
                                                                          ]
                                                                        ) ;
                                                     rdf:type owl:Class
                                                   ]
                                                 )
                                   ] ,
                                   [ rdf:type owl:Restriction ;
                                     owl:onProperty hdf:coordinate ;
                                     owl:maxQualifiedCardinality "32"^^xsd:nonNegativeInteger ;
                                     owl:onClass hdf:Coordinate
                                   ] ,
                                   [ rdf:type owl:Restriction ;
                                     owl:onProperty hdf:index_0 ;
                                     owl:maxQualifiedCardinality "1"^^xsd:nonNegativeInteger ;
                                     owl:onDataRange hdf:IndexType
                                   ] ,
                                   [ rdf:type owl:Restriction ;
                                     owl:onProperty hdf:index_1 ;
                                     owl:maxQualifiedCardinality "1"^^xsd:nonNegativeInteger ;
                                     owl:onDataRange hdf:IndexType
                                   ] ,
                                   [ rdf:type owl:Restriction ;
                                     owl:onProperty hdf:index_10 ;
                                     owl:maxQualifiedCardinality "1"^^xsd:nonNegativeInteger ;
                                     owl:onDataRange hdf:IndexType
                                   ] ,
                                   [ rdf:type owl:Restriction ;
                                     owl:onProperty hdf:index_11 ;
                                     owl:maxQualifiedCardinality "1"^^xsd:nonNegativeInteger ;
                                     owl:onDataRange hdf:IndexType
                                   ] ,
                                   [ rdf:type owl:Restriction ;
                                     owl:onProperty hdf:index_12 ;
                                     owl:maxQualifiedCardinality "1"^^xsd:nonNegativeInteger ;
                                     owl:onDataRange hdf:IndexType
                                   ] ,
                                   [ rdf:type owl:Restriction ;
                                     owl:onProperty hdf:index_13 ;
                                     owl:maxQualifiedCardinality "1"^^xsd:nonNegativeInteger ;
                                     owl:onDataRange hdf:IndexType
                                   ] ,
                                   [ rdf:type owl:Restriction ;
                                     owl:onProperty hdf:index_14 ;
                                     owl:maxQualifiedCardinality "1"^^xsd:nonNegativeInteger ;
                                     owl:onDataRange hdf:IndexType
                                   ] ,
                                   [ rdf:type owl:Restriction ;
                                     owl:onProperty hdf:index_15 ;
                                     owl:maxQualifiedCardinality "1"^^xsd:nonNegativeInteger ;
                                     owl:onDataRange hdf:IndexType
                                   ] ,
                                   [ rdf:type owl:Restriction ;
                                     owl:onProperty hdf:index_16 ;
                                     owl:maxQualifiedCardinality "1"^^xsd:nonNegativeInteger ;
                                     owl:onDataRange hdf:IndexType
                                   ] ,
                                   [ rdf:type owl:Restriction ;
                                     owl:onProperty hdf:index_17 ;
                                     owl:maxQualifiedCardinality "1"^^xsd:nonNegativeInteger ;
                                     owl:onDataRange hdf:IndexType
                                   ] ,
                                   [ rdf:type owl:Restriction ;
                                     owl:onProperty hdf:index_18 ;
                                     owl:maxQualifiedCardinality "1"^^xsd:nonNegativeInteger ;
                                     owl:onDataRange hdf:IndexType
                                   ] ,
                                   [ rdf:type owl:Restriction ;
                                     owl:onProperty hdf:index_19 ;
                                     owl:maxQualifiedCardinality "1"^^xsd:nonNegativeInteger ;
                                     owl:onDataRange hdf:IndexType
                                   ] ,
                                   [ rdf:type owl:Restriction ;
                                     owl:onProperty hdf:index_2 ;
                                     owl:maxQualifiedCardinality "1"^^xsd:nonNegativeInteger ;
                                     owl:onDataRange hdf:IndexType
                                   ] ,
                                   [ rdf:type owl:Restriction ;
                                     owl:onProperty hdf:index_20 ;
                                     owl:maxQualifiedCardinality "1"^^xsd:nonNegativeInteger ;
                                     owl:onDataRange hdf:IndexType
                                   ] ,
                                   [ rdf:type owl:Restriction ;
                                     owl:onProperty hdf:index_21 ;
                                     owl:maxQualifiedCardinality "1"^^xsd:nonNegativeInteger ;
                                     owl:onDataRange hdf:IndexType
                                   ] ,
                                   [ rdf:type owl:Restriction ;
                                     owl:onProperty hdf:index_22 ;
                                     owl:maxQualifiedCardinality "1"^^xsd:nonNegativeInteger ;
                                     owl:onDataRange hdf:IndexType
                                   ] ,
                                   [ rdf:type owl:Restriction ;
                                     owl:onProperty hdf:index_23 ;
                                     owl:maxQualifiedCardinality "1"^^xsd:nonNegativeInteger ;
                                     owl:onDataRange hdf:IndexType
                                   ] ,
                                   [ rdf:type owl:Restriction ;
                                     owl:onProperty hdf:index_24 ;
                                     owl:maxQualifiedCardinality "1"^^xsd:nonNegativeInteger ;
                                     owl:onDataRange hdf:IndexType
                                   ] ,
                                   [ rdf:type owl:Restriction ;
                                     owl:onProperty hdf:index_25 ;
                                     owl:maxQualifiedCardinality "1"^^xsd:nonNegativeInteger ;
                                     owl:onDataRange hdf:IndexType
                                   ] ,
                                   [ rdf:type owl:Restriction ;
                                     owl:onProperty hdf:index_26 ;
                                     owl:maxQualifiedCardinality "1"^^xsd:nonNegativeInteger ;
                                     owl:onDataRange hdf:IndexType
                                   ] ,
                                   [ rdf:type owl:Restriction ;
                                     owl:onProperty hdf:index_27 ;
                                     owl:maxQualifiedCardinality "1"^^xsd:nonNegativeInteger ;
                                     owl:onDataRange hdf:IndexType
                                   ] ,
                                   [ rdf:type owl:Restriction ;
                                     owl:onProperty hdf:index_28 ;
                                     owl:maxQualifiedCardinality "1"^^xsd:nonNegativeInteger ;
                                     owl:onDataRange hdf:IndexType
                                   ] ,
                                   [ rdf:type owl:Restriction ;
                                     owl:onProperty hdf:index_29 ;
                                     owl:maxQualifiedCardinality "1"^^xsd:nonNegativeInteger ;
                                     owl:onDataRange hdf:IndexType
                                   ] ,
                                   [ rdf:type owl:Restriction ;
                                     owl:onProperty hdf:index_3 ;
                                     owl:maxQualifiedCardinality "1"^^xsd:nonNegativeInteger ;
                                     owl:onDataRange hdf:IndexType
                                   ] ,
                                   [ rdf:type owl:Restriction ;
                                     owl:onProperty hdf:index_30 ;
                                     owl:maxQualifiedCardinality "1"^^xsd:nonNegativeInteger ;
                                     owl:onDataRange hdf:IndexType
                                   ] ,
                                   [ rdf:type owl:Restriction ;
                                     owl:onProperty hdf:index_31 ;
                                     owl:maxQualifiedCardinality "1"^^xsd:nonNegativeInteger ;
                                     owl:onDataRange hdf:IndexType
                                   ] ,
                                   [ rdf:type owl:Restriction ;
                                     owl:onProperty hdf:index_4 ;
                                     owl:maxQualifiedCardinality "1"^^xsd:nonNegativeInteger ;
                                     owl:onDataRange hdf:IndexType
                                   ] ,
                                   [ rdf:type owl:Restriction ;
                                     owl:onProperty hdf:index_5 ;
                                     owl:maxQualifiedCardinality "1"^^xsd:nonNegativeInteger ;
                                     owl:onDataRange hdf:IndexType
                                   ] ,
                                   [ rdf:type owl:Restriction ;
                                     owl:onProperty hdf:index_6 ;
                                     owl:maxQualifiedCardinality "1"^^xsd:nonNegativeInteger ;
                                     owl:onDataRange hdf:IndexType
                                   ] ,
                                   [ rdf:type owl:Restriction ;
                                     owl:onProperty hdf:index_7 ;
                                     owl:maxQualifiedCardinality "1"^^xsd:nonNegativeInteger ;
                                     owl:onDataRange hdf:IndexType
                                   ] ,
                                   [ rdf:type owl:Restriction ;
                                     owl:onProperty hdf:index_8 ;
                                     owl:maxQualifiedCardinality "1"^^xsd:nonNegativeInteger ;
                                     owl:onDataRange hdf:IndexType
                                   ] ,
                                   [ rdf:type owl:Restriction ;
                                     owl:onProperty hdf:index_9 ;
                                     owl:maxQualifiedCardinality "1"^^xsd:nonNegativeInteger ;
                                     owl:onDataRange hdf:IndexType
                                   ] ;
                   rdfs:label "point-value pair" ;
                   skos:prefLabel "point-value pair" .


###  http://purl.allotrope.org/ontologies/hdf5/1.8#ReferenceDatatype
hdf:ReferenceDatatype rdf:type owl:Class ;
                      rdfs:subClassOf hdf:AtomicDatatype ,
                                      [ rdf:type owl:Restriction ;
                                        owl:onProperty hdf:typeClass ;
                                        owl:hasValue hdf:H5T_REFERENCE
                                      ] ;
                      rdfs:label "reference" ;
                      skos:prefLabel "reference" .


###  http://purl.allotrope.org/ontologies/hdf5/1.8#SZipCoding
hdf:SZipCoding rdf:type owl:Class ;
               rdfs:label "SZip encoding" ;
               skos:prefLabel "SZip encoding" .


###  http://purl.allotrope.org/ontologies/hdf5/1.8#ScalarDataspace
hdf:ScalarDataspace rdf:type owl:Class ;
                    rdfs:subClassOf hdf:Dataspace ,
                                    [ rdf:type owl:Restriction ;
                                      owl:onProperty hdf:dimension ;
                                      owl:qualifiedCardinality "0"^^xsd:nonNegativeInteger ;
                                      owl:onClass hdf:DataspaceDimension
                                    ] ;
                    rdfs:label "scalar dataspace" ;
                    skos:prefLabel "scalar dataspace" .


###  http://purl.allotrope.org/ontologies/hdf5/1.8#ScaleType
hdf:ScaleType rdf:type owl:Class ;
              rdfs:label "scale type" ;
              skos:prefLabel "scale type" .


###  http://purl.allotrope.org/ontologies/hdf5/1.8#Selection
hdf:Selection rdf:type owl:Class ;
              rdfs:subClassOf [ rdf:type owl:Restriction ;
                                owl:onProperty hdf:selectionOn ;
                                owl:qualifiedCardinality "1"^^xsd:nonNegativeInteger ;
                                owl:onClass hdf:Dataspace
                              ] ;
              rdfs:comment """(1) A subset of a dataset or a dataspace, up to the entire dataset of dataspace.
(2) The elements of an array or dataset that are marked for I/O. [HDF]""" ;
              rdfs:label "selection" ;
              skos:definition """(1) A subset of a dataset or a dataspace, up to the entire dataset of dataspace.
(2) The elements of an array or dataset that are marked for I/O. [HDF]""" ;
              skos:prefLabel "selection" .


###  http://purl.allotrope.org/ontologies/hdf5/1.8#Sign
hdf:Sign rdf:type owl:Class ;
         rdfs:label "sign" ;
         skos:prefLabel "sign" .


###  http://purl.allotrope.org/ontologies/hdf5/1.8#SignField
hdf:SignField rdf:type owl:Class ;
              rdfs:subClassOf hdf:FieldSpecification ;
              rdfs:label "sign field" ;
              skos:prefLabel "sign field" .


###  http://purl.allotrope.org/ontologies/hdf5/1.8#SimpleDataspace
hdf:SimpleDataspace rdf:type owl:Class ;
                    rdfs:subClassOf hdf:Dataspace ,
                                    [ rdf:type owl:Restriction ;
                                      owl:onProperty hdf:dimension ;
                                      owl:someValuesFrom hdf:DataspaceDimension
                                    ] ;
                    rdfs:label "simple dataspace" ;
                    skos:prefLabel "simple dataspace" .


###  http://purl.allotrope.org/ontologies/hdf5/1.8#SoftLink
hdf:SoftLink rdf:type owl:Class ;
             rdfs:subClassOf hdf:Link ,
                             [ rdf:type owl:Restriction ;
                               owl:onProperty hdf:linkedTo ;
                               owl:maxQualifiedCardinality "1"^^xsd:nonNegativeInteger ;
                               owl:onClass hdf:NamedObject
                             ] ;
             rdfs:comment "An indirect association between a name and an object in an HDF5 file. [Allotrope]" ;
             rdfs:label "soft link" ;
             skos:definition "An indirect association between a name and an object in an HDF5 file. [Allotrope]" ;
             skos:prefLabel "soft link" .


###  http://purl.allotrope.org/ontologies/hdf5/1.8#StorageAllocation
hdf:StorageAllocation rdf:type owl:Class ;
                      rdfs:label "storage allocation" ;
                      skos:prefLabel "storage allocation" .


###  http://purl.allotrope.org/ontologies/hdf5/1.8#StorageLayout
hdf:StorageLayout rdf:type owl:Class ;
                  rdfs:comment "The HDF5 format makes it possible to store data in a variety of ways. The default storage layout format is contiguous, meaning that data is stored in the same linear way that it is organized in memory. Two other storage layout formats are currently defined for HDF5: compact, and chunked. In the future, other storage layouts may be added. [Allotrope]" ;
                  rdfs:label "storage layout" ;
                  skos:definition "The HDF5 format makes it possible to store data in a variety of ways. The default storage layout format is contiguous, meaning that data is stored in the same linear way that it is organized in memory. Two other storage layout formats are currently defined for HDF5: compact, and chunked. In the future, other storage layouts may be added. [Allotrope]" ;
                  skos:prefLabel "storage layout" .


###  http://purl.allotrope.org/ontologies/hdf5/1.8#StringAttribute
hdf:StringAttribute rdf:type owl:Class ;
                    rdfs:subClassOf hdf:Attribute ;
                    rdfs:label "string attribute" ;
                    skos:prefLabel "string attribute" .


###  http://purl.allotrope.org/ontologies/hdf5/1.8#StringDatatype
hdf:StringDatatype rdf:type owl:Class ;
                   rdfs:subClassOf hdf:AtomicDatatype ,
                                   [ rdf:type owl:Restriction ;
                                     owl:onProperty hdf:typeClass ;
                                     owl:hasValue hdf:H5T_STRING
                                   ] ,
                                   [ rdf:type owl:Restriction ;
                                     owl:onProperty hdf:size ;
                                     owl:qualifiedCardinality "1"^^xsd:nonNegativeInteger ;
                                     owl:onDataRange [ rdf:type rdfs:Datatype ;
                                                       owl:onDatatype xsd:long ;
                                                       owl:withRestrictions ( [ xsd:minExclusive "-2"^^xsd:long
                                                                              ]
                                                                            )
                                                     ]
                                   ] ;
                   rdfs:label "string" ;
                   skos:prefLabel "string" .


###  http://purl.allotrope.org/ontologies/hdf5/1.8#StringPadding
hdf:StringPadding rdf:type owl:Class ;
                  rdfs:comment "The string datatype has a fixed length, but the string may be shorter than the length. The StringPadding defines the storage mechanism for the left over bytes. [Allotrope]" ;
                  rdfs:label "string padding" ;
                  skos:definition "The string datatype has a fixed length, but the string may be shorter than the length. The StringPadding defines the storage mechanism for the left over bytes. [Allotrope]" ;
                  skos:prefLabel "string padding" .


###  http://purl.allotrope.org/ontologies/hdf5/1.8#TimeDatatype
hdf:TimeDatatype rdf:type owl:Class ;
                 rdfs:subClassOf hdf:AtomicDatatype ,
                                 [ rdf:type owl:Restriction ;
                                   owl:onProperty hdf:typeClass ;
                                   owl:hasValue hdf:H5T_TIME
                                 ] ;
                 rdfs:label "time" ;
                 skos:prefLabel "time" .


###  http://purl.allotrope.org/ontologies/hdf5/1.8#TransferMode
hdf:TransferMode rdf:type owl:Class ;
                 rdfs:label "transfer mode" ;
                 skos:prefLabel "transfer mode" .


###  http://purl.allotrope.org/ontologies/hdf5/1.8#TypeClass
hdf:TypeClass rdf:type owl:Class ;
              rdfs:comment "HDF datatype class. [Allotrope]" ;
              rdfs:label "type class" ;
              skos:definition "HDF datatype class. [Allotrope]" ;
              skos:prefLabel "type class" .


###  http://purl.allotrope.org/ontologies/hdf5/1.8#VariableLengthDatatype
hdf:VariableLengthDatatype rdf:type owl:Class ;
                           rdfs:subClassOf hdf:CompositeDatatype ,
                                           [ rdf:type owl:Restriction ;
                                             owl:onProperty hdf:typeClass ;
                                             owl:hasValue hdf:H5T_VLEN
                                           ] ,
                                           [ rdf:type owl:Restriction ;
                                             owl:onProperty hdf:datatype ;
                                             owl:qualifiedCardinality "1"^^xsd:nonNegativeInteger ;
                                             owl:onClass hdf:Datatype
                                           ] ;
                           rdfs:comment "A sequence of an existing datatype (atomic, variable-length (VL), or compound) which are not fixed in length form one dataset location to another. [Allotrope]" ;
                           rdfs:label "variable-length datatype" ;
                           skos:definition "A sequence of an existing datatype (atomic, variable-length (VL), or compound) which are not fixed in length form one dataset location to another. [Allotrope]" ;
                           skos:prefLabel "variable-length datatype" .


###  http://purl.allotrope.org/ontologies/hdf5/1.8#XOrSelection
hdf:XOrSelection rdf:type owl:Class ;
                 rdfs:subClassOf hdf:Selection ,
                                 [ rdf:type owl:Restriction ;
                                   owl:onProperty hdf:previous ;
                                   owl:qualifiedCardinality "1"^^xsd:nonNegativeInteger ;
                                   owl:onClass hdf:Selection
                                 ] ,
                                 [ rdf:type owl:Restriction ;
                                   owl:onProperty hdf:xor ;
                                   owl:qualifiedCardinality "1"^^xsd:nonNegativeInteger ;
                                   owl:onClass hdf:Selection
                                 ] ;
                 rdfs:label "xor selection" ;
                 skos:altLabel "exclusive or selection" ;
                 skos:prefLabel "xor selection" .


###  http://purl.org/dc/terms/LicenseDocument
dct:LicenseDocument rdf:type owl:Class .


###  http://purl.org/dc/terms/RightsStatement
dct:RightsStatement rdf:type owl:Class .


#################################################################
#    Individuals
#################################################################

###  http://purl.allotrope.org/ontologies/hdf5/1.8#H5D_ALLOC_TIME_DEFAULT
hdf:H5D_ALLOC_TIME_DEFAULT rdf:type owl:NamedIndividual ,
                                    hdf:StorageAllocation ;
                           rdfs:comment "Allocate dataset storage space at the default time. Defaults differ by storage method. [HDF]" ;
                           rdfs:label "default" ;
                           skos:definition "Allocate dataset storage space at the default time. Defaults differ by storage method. [HDF]" ;
                           skos:prefLabel "default" .


###  http://purl.allotrope.org/ontologies/hdf5/1.8#H5D_ALLOC_TIME_EARLY
hdf:H5D_ALLOC_TIME_EARLY rdf:type owl:NamedIndividual ,
                                  hdf:StorageAllocation ;
                         rdfs:comment "Allocate all space when the dataset is created. Default for compact datasets. [HDF]" ;
                         rdfs:label "early" ;
                         skos:definition "Allocate all space when the dataset is created. Default for compact datasets. [HDF]" ;
                         skos:prefLabel "early" .


###  http://purl.allotrope.org/ontologies/hdf5/1.8#H5D_ALLOC_TIME_INCR
hdf:H5D_ALLOC_TIME_INCR rdf:type owl:NamedIndividual ,
                                 hdf:StorageAllocation ;
                        rdfs:comment "Allocate space incrementally, as data is written to the dataset. Default for chunked storage datasets. [HDF]" ;
                        rdfs:label "incremental" ;
                        skos:definition "Allocate space incrementally, as data is written to the dataset. Default for chunked storage datasets. [HDF]" ;
                        skos:prefLabel "incremental" .


###  http://purl.allotrope.org/ontologies/hdf5/1.8#H5D_ALLOC_TIME_LATE
hdf:H5D_ALLOC_TIME_LATE rdf:type owl:NamedIndividual ,
                                 hdf:StorageAllocation ;
                        rdfs:comment "Allocate all space when data is first written to the dataset. Default for contiguous datasets. [HDF]" ;
                        rdfs:label "late" ;
                        skos:definition "Allocate all space when data is first written to the dataset. Default for contiguous datasets. [HDF]" ;
                        skos:prefLabel "late" .


###  http://purl.allotrope.org/ontologies/hdf5/1.8#H5D_CHUNKED
hdf:H5D_CHUNKED rdf:type owl:NamedIndividual ,
                         hdf:StorageLayout ;
                rdfs:comment "Chunked storage involves dividing the dataset into equal-sized \"chunks\" that are stored separately. [Allotrope]" ;
                rdfs:label "chunked" ;
                skos:definition "Chunked storage involves dividing the dataset into equal-sized \"chunks\" that are stored separately. [Allotrope]" ;
                skos:prefLabel "chunked" .


###  http://purl.allotrope.org/ontologies/hdf5/1.8#H5D_COMPACT
hdf:H5D_COMPACT rdf:type owl:NamedIndividual ,
                         hdf:StorageLayout ;
                rdfs:comment "Compact storage is used when the amount of data is small and can be stored directly in the object header. [Allotrope]" ;
                rdfs:label "compact" ;
                skos:definition "Compact storage is used when the amount of data is small and can be stored directly in the object header. [Allotrope]" ;
                skos:prefLabel "compact" .


###  http://purl.allotrope.org/ontologies/hdf5/1.8#H5D_CONTIGUOUS
hdf:H5D_CONTIGUOUS rdf:type owl:NamedIndividual ,
                            hdf:StorageLayout ;
                   rdfs:label "contiguous" ;
                   skos:prefLabel "contiguous" .


###  http://purl.allotrope.org/ontologies/hdf5/1.8#H5D_FILL_TIME_ALLOC
hdf:H5D_FILL_TIME_ALLOC rdf:type owl:NamedIndividual ,
                                 hdf:FillTime ;
                        rdfs:comment "Fill values are written to the dataset when storage space is allocated. [Allotrope]" ;
                        rdfs:label "fill on allocation" ;
                        skos:definition "Fill values are written to the dataset when storage space is allocated. [Allotrope]" ;
                        skos:prefLabel "fill on allocation" .


###  http://purl.allotrope.org/ontologies/hdf5/1.8#H5D_FILL_TIME_IFSET
hdf:H5D_FILL_TIME_IFSET rdf:type owl:NamedIndividual ,
                                 hdf:FillTime ;
                        rdfs:comment "Fill values are written to the dataset when storage space is allocated only if there is a user-defined fill value, i.e., one set with H5Pset_fill_value. Default. [HDF]" ;
                        rdfs:label "fill if set" ;
                        skos:definition "Fill values are written to the dataset when storage space is allocated only if there is a user-defined fill value, i.e., one set with H5Pset_fill_value. Default. [HDF]" ;
                        skos:prefLabel "fill if set" .


###  http://purl.allotrope.org/ontologies/hdf5/1.8#H5D_FILL_TIME_NEVER
hdf:H5D_FILL_TIME_NEVER rdf:type owl:NamedIndividual ,
                                 hdf:FillTime ;
                        rdfs:comment "Fill values are never written to the dataset. [Allotrope]" ;
                        rdfs:label "fill never" ;
                        skos:definition "Fill values are never written to the dataset. [Allotrope]" ;
                        skos:prefLabel "fill never" .


###  http://purl.allotrope.org/ontologies/hdf5/1.8#H5D_FILL_VALUE_DEFAULT
hdf:H5D_FILL_VALUE_DEFAULT rdf:type owl:NamedIndividual ,
                                    hdf:FillValueStatus ;
                           rdfs:comment "Fill value is the library default. [Allotrope]" ;
                           rdfs:label "default" ;
                           skos:definition "Fill value is the library default. [Allotrope]" ;
                           skos:prefLabel "default" .


###  http://purl.allotrope.org/ontologies/hdf5/1.8#H5D_FILL_VALUE_UNDEFINED
hdf:H5D_FILL_VALUE_UNDEFINED rdf:type owl:NamedIndividual ,
                                      hdf:FillValueStatus ;
                             rdfs:comment "Fill value is undefined. [Allotrope]" ;
                             rdfs:label "undefined" ;
                             skos:definition "Fill value is undefined. [Allotrope]" ;
                             skos:prefLabel "undefined" .


###  http://purl.allotrope.org/ontologies/hdf5/1.8#H5D_FILL_VALUE_USER_DEFINED
hdf:H5D_FILL_VALUE_USER_DEFINED rdf:type owl:NamedIndividual ,
                                         hdf:FillValueStatus ;
                                rdfs:comment "Fill value is defined by the application. [Allotrope]" ;
                                rdfs:label "user defined" ;
                                skos:definition "Fill value is defined by the application. [Allotrope]" ;
                                skos:prefLabel "user defined" .


###  http://purl.allotrope.org/ontologies/hdf5/1.8#H5D_VIRTUAL
hdf:H5D_VIRTUAL rdf:type owl:NamedIndividual ,
                         hdf:StorageLayout ;
                rdfs:label "virtual" ;
                skos:prefLabel "virtual" .


###  http://purl.allotrope.org/ontologies/hdf5/1.8#H5FD_MPIO_CHUNK_MULTI_IO
hdf:H5FD_MPIO_CHUNK_MULTI_IO rdf:type owl:NamedIndividual ,
                                      hdf:ChunkMode ;
                             rdfs:label "multi-chunked I/O" ;
                             skos:prefLabel "multi-chunked I/O" .


###  http://purl.allotrope.org/ontologies/hdf5/1.8#H5FD_MPIO_CHUNK_ONE_IO
hdf:H5FD_MPIO_CHUNK_ONE_IO rdf:type owl:NamedIndividual ,
                                    hdf:ChunkMode ;
                           rdfs:label "one link chunked I/O" ;
                           skos:prefLabel "one link chunked I/O" .


###  http://purl.allotrope.org/ontologies/hdf5/1.8#H5FD_MPIO_COLLECTIVE
hdf:H5FD_MPIO_COLLECTIVE rdf:type owl:NamedIndividual ,
                                  hdf:TransferMode ;
                         rdfs:comment "Use collective I/O access. [Allotrope]" ;
                         rdfs:label "collective" ;
                         skos:definition "Use collective I/O access. [Allotrope]" ;
                         skos:prefLabel "collective" .


###  http://purl.allotrope.org/ontologies/hdf5/1.8#H5FD_MPIO_INDEPENDENT
hdf:H5FD_MPIO_INDEPENDENT rdf:type owl:NamedIndividual ,
                                   hdf:TransferMode ;
                          rdfs:comment "Use independent I/O access. Default. [Allotrope]" ;
                          rdfs:label "independent" ;
                          skos:definition "Use independent I/O access Default. [Allotrope]" ;
                          skos:prefLabel "independent" .


###  http://purl.allotrope.org/ontologies/hdf5/1.8#H5F_ACC_DEFAULT
hdf:H5F_ACC_DEFAULT rdf:type owl:NamedIndividual ,
                             hdf:FileAccessMode ;
                    rdfs:label "default" ;
                    skos:altLabel "default file access mode" ;
                    skos:prefLabel "default" .


###  http://purl.allotrope.org/ontologies/hdf5/1.8#H5F_ACC_RDONLY
hdf:H5F_ACC_RDONLY rdf:type owl:NamedIndividual ,
                            hdf:FileAccessMode ;
                   rdfs:label "read only" ;
                   skos:altLabel "read only file access mode" ;
                   skos:prefLabel "read only" .


###  http://purl.allotrope.org/ontologies/hdf5/1.8#H5F_ACC_RDWR
hdf:H5F_ACC_RDWR rdf:type owl:NamedIndividual ,
                          hdf:FileAccessMode ;
                 rdfs:label "read/write" ;
                 skos:altLabel "read/write file access mode" ;
                 skos:prefLabel "read/write" .


###  http://purl.allotrope.org/ontologies/hdf5/1.8#H5O_SHMESG_ALL_FLAG
hdf:H5O_SHMESG_ALL_FLAG rdf:type owl:NamedIndividual ,
                                 hdf:MessageTypeFlag ;
                        rdfs:label "all messages" ;
                        skos:prefLabel "all messages" .


###  http://purl.allotrope.org/ontologies/hdf5/1.8#H5O_SHMESG_ATTR_FLAG
hdf:H5O_SHMESG_ATTR_FLAG rdf:type owl:NamedIndividual ,
                                  hdf:MessageTypeFlag ;
                         rdfs:label "attribute message" ;
                         skos:prefLabel "attribute message" .


###  http://purl.allotrope.org/ontologies/hdf5/1.8#H5O_SHMESG_DTYPE_FLAG
hdf:H5O_SHMESG_DTYPE_FLAG rdf:type owl:NamedIndividual ,
                                   hdf:MessageTypeFlag ;
                          rdfs:label "datatype message" ;
                          skos:prefLabel "datatype message" .


###  http://purl.allotrope.org/ontologies/hdf5/1.8#H5O_SHMESG_FILL_FLAG
hdf:H5O_SHMESG_FILL_FLAG rdf:type owl:NamedIndividual ,
                                  hdf:MessageTypeFlag ;
                         rdfs:label "fill value message" ;
                         skos:prefLabel "fill value message" .


###  http://purl.allotrope.org/ontologies/hdf5/1.8#H5O_SHMESG_NONE_FLAG
hdf:H5O_SHMESG_NONE_FLAG rdf:type owl:NamedIndividual ,
                                  hdf:MessageTypeFlag ;
                         rdfs:label "no shared message" ;
                         skos:prefLabel "no shared message" .


###  http://purl.allotrope.org/ontologies/hdf5/1.8#H5O_SHMESG_PLINE_FLAG
hdf:H5O_SHMESG_PLINE_FLAG rdf:type owl:NamedIndividual ,
                                   hdf:MessageTypeFlag ;
                          rdfs:label "filter pipeline message" ;
                          skos:prefLabel "filter pipeline message" .


###  http://purl.allotrope.org/ontologies/hdf5/1.8#H5O_SHMESG_SDSPACE_FLAG
hdf:H5O_SHMESG_SDSPACE_FLAG rdf:type owl:NamedIndividual ,
                                     hdf:MessageTypeFlag ;
                            rdfs:label "simple dataspace message" ;
                            skos:prefLabel "simple dataspace message" .


###  http://purl.allotrope.org/ontologies/hdf5/1.8#H5P_DATASET_CREATE
hdf:H5P_DATASET_CREATE rdf:type owl:NamedIndividual .


###  http://purl.allotrope.org/ontologies/hdf5/1.8#H5P_DATASET_XFER
hdf:H5P_DATASET_XFER rdf:type owl:NamedIndividual .


###  http://purl.allotrope.org/ontologies/hdf5/1.8#H5P_FILE_ACCESS
hdf:H5P_FILE_ACCESS rdf:type owl:NamedIndividual .


###  http://purl.allotrope.org/ontologies/hdf5/1.8#H5P_FILE_CREATE
hdf:H5P_FILE_CREATE rdf:type owl:NamedIndividual .


###  http://purl.allotrope.org/ontologies/hdf5/1.8#H5P_FILE_MOUNT
hdf:H5P_FILE_MOUNT rdf:type owl:NamedIndividual .


###  http://purl.allotrope.org/ontologies/hdf5/1.8#H5T_ALPHA_B16
hdf:H5T_ALPHA_B16 rdf:type owl:NamedIndividual ,
                           hdf:BitfieldDatatype ;
                  hdf:order hdf:H5T_ORDER_LE ;
                  rdfs:label "DEC Alpha specific 16 bit bitfield" ;
                  skos:prefLabel "DEC Alpha specific 16 bit bitfield" .


###  http://purl.allotrope.org/ontologies/hdf5/1.8#H5T_ALPHA_B32
hdf:H5T_ALPHA_B32 rdf:type owl:NamedIndividual ,
                           hdf:BitfieldDatatype ;
                  hdf:order hdf:H5T_ORDER_LE ;
                  rdfs:label "DEC Alpha specific  32 bit bitfield" ;
                  skos:prefLabel "DEC Alpha specific  32 bit bitfield" .


###  http://purl.allotrope.org/ontologies/hdf5/1.8#H5T_ALPHA_B64
hdf:H5T_ALPHA_B64 rdf:type owl:NamedIndividual ,
                           hdf:BitfieldDatatype ;
                  hdf:order hdf:H5T_ORDER_LE ;
                  rdfs:label "DEC Alpha specific  64 bit bitfield" ;
                  skos:prefLabel "DEC Alpha specific  64 bit bitfield" .


###  http://purl.allotrope.org/ontologies/hdf5/1.8#H5T_ALPHA_B8
hdf:H5T_ALPHA_B8 rdf:type owl:NamedIndividual ,
                          hdf:BitfieldDatatype ;
                 hdf:order hdf:H5T_ORDER_LE ;
                 rdfs:label "DEC Alpha specific 8 bit bitfield" ;
                 skos:prefLabel "DEC Alpha specific 8 bit bitfield" .


###  http://purl.allotrope.org/ontologies/hdf5/1.8#H5T_ALPHA_F32
hdf:H5T_ALPHA_F32 rdf:type owl:NamedIndividual ,
                           hdf:FloatDatatype ;
                  hdf:order hdf:H5T_ORDER_LE ;
                  rdfs:label "DEC Alpha specific 32 bit floating point" ;
                  skos:prefLabel "DEC Alpha specific 32 bit floating point" .


###  http://purl.allotrope.org/ontologies/hdf5/1.8#H5T_ALPHA_F64
hdf:H5T_ALPHA_F64 rdf:type owl:NamedIndividual ,
                           hdf:FloatDatatype ;
                  hdf:order hdf:H5T_ORDER_LE ;
                  rdfs:label "DEC Alpha specific 64 bit floating point" ;
                  skos:prefLabel "DEC Alpha specific 64 bit floating point" .


###  http://purl.allotrope.org/ontologies/hdf5/1.8#H5T_ALPHA_I16
hdf:H5T_ALPHA_I16 rdf:type owl:NamedIndividual ,
                           hdf:IntegerDatatype ;
                  hdf:order hdf:H5T_ORDER_LE ;
                  hdf:sign hdf:H5T_SGN_2 ;
                  rdfs:label "DEC Alpha specific 8 bit signed integer" ;
                  skos:prefLabel "DEC Alpha specific 8 bit signed integer" .


###  http://purl.allotrope.org/ontologies/hdf5/1.8#H5T_ALPHA_I32
hdf:H5T_ALPHA_I32 rdf:type owl:NamedIndividual ,
                           hdf:IntegerDatatype ;
                  hdf:order hdf:H5T_ORDER_LE ;
                  hdf:sign hdf:H5T_SGN_2 ;
                  rdfs:label "DEC Alpha specific 8 bit signed integer" ;
                  skos:prefLabel "DEC Alpha specific 8 bit signed integer" .


###  http://purl.allotrope.org/ontologies/hdf5/1.8#H5T_ALPHA_I64
hdf:H5T_ALPHA_I64 rdf:type owl:NamedIndividual ,
                           hdf:IntegerDatatype ;
                  hdf:order hdf:H5T_ORDER_LE ;
                  hdf:sign hdf:H5T_SGN_2 ;
                  rdfs:label "DEC Alpha specific 8 bit signed integer" ;
                  skos:prefLabel "DEC Alpha specific 8 bit signed integer" .


###  http://purl.allotrope.org/ontologies/hdf5/1.8#H5T_ALPHA_I8
hdf:H5T_ALPHA_I8 rdf:type owl:NamedIndividual ,
                          hdf:IntegerDatatype ;
                 hdf:order hdf:H5T_ORDER_LE ;
                 hdf:sign hdf:H5T_SGN_2 ;
                 rdfs:label "DEC Alpha specific 8 bit signed integer" ;
                 skos:prefLabel "DEC Alpha specific 8 bit signed integer" .


###  http://purl.allotrope.org/ontologies/hdf5/1.8#H5T_ALPHA_U16
hdf:H5T_ALPHA_U16 rdf:type owl:NamedIndividual ,
                           hdf:IntegerDatatype ;
                  hdf:order hdf:H5T_ORDER_LE ;
                  hdf:sign hdf:H5T_SGN_NONE ;
                  rdfs:label "DEC Alpha 16 bit unsigned integer" ;
                  skos:prefLabel "DEC Alpha 16 bit unsigned integer" .


###  http://purl.allotrope.org/ontologies/hdf5/1.8#H5T_ALPHA_U32
hdf:H5T_ALPHA_U32 rdf:type owl:NamedIndividual ,
                           hdf:IntegerDatatype ;
                  hdf:order hdf:H5T_ORDER_LE ;
                  hdf:sign hdf:H5T_SGN_NONE ;
                  rdfs:label "DEC Alpha 32 bit unsigned integer" ;
                  skos:prefLabel "DEC Alpha 32 bit unsigned integer" .


###  http://purl.allotrope.org/ontologies/hdf5/1.8#H5T_ALPHA_U64
hdf:H5T_ALPHA_U64 rdf:type owl:NamedIndividual ,
                           hdf:IntegerDatatype ;
                  hdf:order hdf:H5T_ORDER_LE ;
                  hdf:sign hdf:H5T_SGN_NONE ;
                  rdfs:label "DEC Alpha 64 bit unsigned integer" ;
                  skos:prefLabel "DEC Alpha 64 bit unsigned integer" .


###  http://purl.allotrope.org/ontologies/hdf5/1.8#H5T_ALPHA_U8
hdf:H5T_ALPHA_U8 rdf:type owl:NamedIndividual ,
                          hdf:IntegerDatatype ;
                 hdf:order hdf:H5T_ORDER_LE ;
                 hdf:sign hdf:H5T_SGN_NONE ;
                 rdfs:label "DEC Alpha 8 bit unsigned integer" ;
                 skos:prefLabel "DEC Alpha 8 bit unsigned integer" .


###  http://purl.allotrope.org/ontologies/hdf5/1.8#H5T_ARRAY
hdf:H5T_ARRAY rdf:type owl:NamedIndividual ,
                       hdf:TypeClass ;
              rdfs:label "array" ;
              skos:prefLabel "array" .


###  http://purl.allotrope.org/ontologies/hdf5/1.8#H5T_BITFIELD
hdf:H5T_BITFIELD rdf:type owl:NamedIndividual ,
                          hdf:TypeClass ;
                 rdfs:label "bitfield" ;
                 skos:prefLabel "bitfield" .


###  http://purl.allotrope.org/ontologies/hdf5/1.8#H5T_COMPOUND
hdf:H5T_COMPOUND rdf:type owl:NamedIndividual ,
                          hdf:TypeClass ;
                 rdfs:label "compound" ;
                 skos:prefLabel "compound" .


###  http://purl.allotrope.org/ontologies/hdf5/1.8#H5T_CSET_ASCII
hdf:H5T_CSET_ASCII rdf:type owl:NamedIndividual ,
                            hdf:CharacterSet ;
                   rdfs:label "ASCII" ;
                   skos:prefLabel "ASCII" .


###  http://purl.allotrope.org/ontologies/hdf5/1.8#H5T_CSET_UTF8
hdf:H5T_CSET_UTF8 rdf:type owl:NamedIndividual ,
                           hdf:CharacterSet ;
                  rdfs:label "UTF-8" ;
                  skos:prefLabel "UTF-8" .


###  http://purl.allotrope.org/ontologies/hdf5/1.8#H5T_ENUM
hdf:H5T_ENUM rdf:type owl:NamedIndividual ,
                      hdf:TypeClass ;
             rdfs:label "enumeration" ;
             skos:prefLabel "enumeration" .


###  http://purl.allotrope.org/ontologies/hdf5/1.8#H5T_FLOAT
hdf:H5T_FLOAT rdf:type owl:NamedIndividual ,
                       hdf:TypeClass ;
              rdfs:label "floating point" ;
              skos:prefLabel "floating point" .


###  http://purl.allotrope.org/ontologies/hdf5/1.8#H5T_IEEE_F32BE
hdf:H5T_IEEE_F32BE rdf:type owl:NamedIndividual ,
                            hdf:FloatDatatype ;
                   hdf:order hdf:H5T_ORDER_BE ;
                   rdfs:label "IEEE 32 bit floating point big endian" ;
                   skos:prefLabel "IEEE 32 bit floating point big endian" .


###  http://purl.allotrope.org/ontologies/hdf5/1.8#H5T_IEEE_F32LE
hdf:H5T_IEEE_F32LE rdf:type owl:NamedIndividual ,
                            hdf:FloatDatatype ;
                   hdf:order hdf:H5T_ORDER_LE ;
                   rdfs:label "IEEE 32 bit floating point little endian" ;
                   skos:prefLabel "IEEE 32 bit floating point little endian" .


###  http://purl.allotrope.org/ontologies/hdf5/1.8#H5T_IEEE_F64BE
hdf:H5T_IEEE_F64BE rdf:type owl:NamedIndividual ,
                            hdf:FloatDatatype ;
                   hdf:order hdf:H5T_ORDER_BE ;
                   rdfs:label "IEEE 64 bit floating point big endian" ;
                   skos:prefLabel "IEEE 64 bit floating point big endian" .


###  http://purl.allotrope.org/ontologies/hdf5/1.8#H5T_IEEE_F64LE
hdf:H5T_IEEE_F64LE rdf:type owl:NamedIndividual ,
                            hdf:FloatDatatype ;
                   hdf:order hdf:H5T_ORDER_LE ;
                   rdfs:label "IEEE 64 bit floating point little endian" ;
                   skos:prefLabel "IEEE 64 bit floating point little endian" .


###  http://purl.allotrope.org/ontologies/hdf5/1.8#H5T_INTEGER
hdf:H5T_INTEGER rdf:type owl:NamedIndividual ,
                         hdf:TypeClass ;
                rdfs:label "integer" ;
                skos:prefLabel "integer" .


###  http://purl.allotrope.org/ontologies/hdf5/1.8#H5T_INTEL_B16
hdf:H5T_INTEL_B16 rdf:type owl:NamedIndividual ,
                           hdf:BitfieldDatatype ;
                  hdf:order hdf:H5T_ORDER_LE ;
                  rdfs:label "Intel specific 16 bit bitfield" ;
                  skos:prefLabel "Intel specific 16 bit bitfield" .


###  http://purl.allotrope.org/ontologies/hdf5/1.8#H5T_INTEL_B32
hdf:H5T_INTEL_B32 rdf:type owl:NamedIndividual ,
                           hdf:BitfieldDatatype ;
                  hdf:order hdf:H5T_ORDER_LE ;
                  rdfs:label "Intel specific  32 bit bitfield" ;
                  skos:prefLabel "Intel specific  32 bit bitfield" .


###  http://purl.allotrope.org/ontologies/hdf5/1.8#H5T_INTEL_B64
hdf:H5T_INTEL_B64 rdf:type owl:NamedIndividual ,
                           hdf:BitfieldDatatype ;
                  hdf:order hdf:H5T_ORDER_LE ;
                  rdfs:label "Intel specific  64 bit bitfield" ;
                  skos:prefLabel "Intel specific  64 bit bitfield" .


###  http://purl.allotrope.org/ontologies/hdf5/1.8#H5T_INTEL_B8
hdf:H5T_INTEL_B8 rdf:type owl:NamedIndividual ,
                          hdf:BitfieldDatatype ;
                 hdf:order hdf:H5T_ORDER_LE ;
                 rdfs:label "Intel specific 8 bit bitfield" ;
                 skos:prefLabel "Intel specific 8 bit bitfield" .


###  http://purl.allotrope.org/ontologies/hdf5/1.8#H5T_INTEL_F32
hdf:H5T_INTEL_F32 rdf:type owl:NamedIndividual ,
                           hdf:FloatDatatype ;
                  hdf:order hdf:H5T_ORDER_LE ;
                  rdfs:label "Intel specific 32 bit floating point" ;
                  skos:prefLabel "Intel specific 32 bit floating point" .


###  http://purl.allotrope.org/ontologies/hdf5/1.8#H5T_INTEL_F64
hdf:H5T_INTEL_F64 rdf:type owl:NamedIndividual ,
                           hdf:FloatDatatype ;
                  hdf:order hdf:H5T_ORDER_LE ;
                  rdfs:label "Intel specific 64 bit floating point" ;
                  skos:prefLabel "Intel specific 64 bit floating point" .


###  http://purl.allotrope.org/ontologies/hdf5/1.8#H5T_INTEL_I16
hdf:H5T_INTEL_I16 rdf:type owl:NamedIndividual ,
                           hdf:IntegerDatatype ;
                  hdf:order hdf:H5T_ORDER_LE ;
                  hdf:sign hdf:H5T_SGN_2 ;
                  rdfs:label "Intel specific 8 bit signed integer" ;
                  skos:prefLabel "Intel specific 8 bit signed integer" .


###  http://purl.allotrope.org/ontologies/hdf5/1.8#H5T_INTEL_I32
hdf:H5T_INTEL_I32 rdf:type owl:NamedIndividual ,
                           hdf:IntegerDatatype ;
                  hdf:order hdf:H5T_ORDER_LE ;
                  hdf:sign hdf:H5T_SGN_2 ;
                  rdfs:label "Intel specific 8 bit signed integer" ;
                  skos:prefLabel "Intel specific 8 bit signed integer" .


###  http://purl.allotrope.org/ontologies/hdf5/1.8#H5T_INTEL_I64
hdf:H5T_INTEL_I64 rdf:type owl:NamedIndividual ,
                           hdf:IntegerDatatype ;
                  hdf:order hdf:H5T_ORDER_LE ;
                  hdf:sign hdf:H5T_SGN_2 ;
                  rdfs:label "Intel specific 8 bit signed integer" ;
                  skos:prefLabel "Intel specific 8 bit signed integer" .


###  http://purl.allotrope.org/ontologies/hdf5/1.8#H5T_INTEL_I8
hdf:H5T_INTEL_I8 rdf:type owl:NamedIndividual ,
                          hdf:IntegerDatatype ;
                 hdf:order hdf:H5T_ORDER_LE ;
                 hdf:sign hdf:H5T_SGN_2 ;
                 rdfs:label "Intel specific 8 bit signed integer" ;
                 skos:prefLabel "Intel specific 8 bit signed integer" .


###  http://purl.allotrope.org/ontologies/hdf5/1.8#H5T_INTEL_U16
hdf:H5T_INTEL_U16 rdf:type owl:NamedIndividual ,
                           hdf:IntegerDatatype ;
                  hdf:order hdf:H5T_ORDER_LE ;
                  hdf:sign hdf:H5T_SGN_NONE ;
                  rdfs:label "Intel 16 bit unsigned integer" ;
                  skos:prefLabel "Intel 16 bit unsigned integer" .


###  http://purl.allotrope.org/ontologies/hdf5/1.8#H5T_INTEL_U32
hdf:H5T_INTEL_U32 rdf:type owl:NamedIndividual ,
                           hdf:IntegerDatatype ;
                  hdf:order hdf:H5T_ORDER_LE ;
                  hdf:sign hdf:H5T_SGN_NONE ;
                  rdfs:label "Intel 32 bit unsigned integer" ;
                  skos:prefLabel "Intel 32 bit unsigned integer" .


###  http://purl.allotrope.org/ontologies/hdf5/1.8#H5T_INTEL_U64
hdf:H5T_INTEL_U64 rdf:type owl:NamedIndividual ,
                           hdf:IntegerDatatype ;
                  hdf:order hdf:H5T_ORDER_LE ;
                  hdf:sign hdf:H5T_SGN_NONE ;
                  rdfs:label "Intel 64 bit unsigned integer" ;
                  skos:prefLabel "Intel 64 bit unsigned integer" .


###  http://purl.allotrope.org/ontologies/hdf5/1.8#H5T_INTEL_U8
hdf:H5T_INTEL_U8 rdf:type owl:NamedIndividual ,
                          hdf:IntegerDatatype ;
                 hdf:order hdf:H5T_ORDER_LE ;
                 hdf:sign hdf:H5T_SGN_NONE ;
                 rdfs:label "Intel 8 bit unsigned integer" ;
                 skos:prefLabel "Intel 8 bit unsigned integer" .


###  http://purl.allotrope.org/ontologies/hdf5/1.8#H5T_MIPS_B16
hdf:H5T_MIPS_B16 rdf:type owl:NamedIndividual ,
                          hdf:BitfieldDatatype ;
                 hdf:order hdf:H5T_ORDER_BE ;
                 rdfs:label "MIPS specific 16 bit bitfield" ;
                 skos:prefLabel "MIPS specific 16 bit bitfield" .


###  http://purl.allotrope.org/ontologies/hdf5/1.8#H5T_MIPS_B32
hdf:H5T_MIPS_B32 rdf:type owl:NamedIndividual ,
                          hdf:BitfieldDatatype ;
                 hdf:order hdf:H5T_ORDER_BE ;
                 rdfs:label "MIPS specific  32 bit bitfield" ;
                 skos:prefLabel "MIPS specific  32 bit bitfield" .


###  http://purl.allotrope.org/ontologies/hdf5/1.8#H5T_MIPS_B64
hdf:H5T_MIPS_B64 rdf:type owl:NamedIndividual ,
                          hdf:BitfieldDatatype ;
                 hdf:order hdf:H5T_ORDER_BE ;
                 rdfs:label "MIPS specific  64 bit bitfield" ;
                 skos:prefLabel "MIPS specific  64 bit bitfield" .


###  http://purl.allotrope.org/ontologies/hdf5/1.8#H5T_MIPS_B8
hdf:H5T_MIPS_B8 rdf:type owl:NamedIndividual ,
                         hdf:BitfieldDatatype ;
                hdf:order hdf:H5T_ORDER_BE ;
                rdfs:label "MIPS specific 8 bit bitfield" ;
                skos:prefLabel "MIPS specific 8 bit bitfield" .


###  http://purl.allotrope.org/ontologies/hdf5/1.8#H5T_MIPS_F32
hdf:H5T_MIPS_F32 rdf:type owl:NamedIndividual ,
                          hdf:FloatDatatype ;
                 hdf:order hdf:H5T_ORDER_BE ;
                 rdfs:label "MIPS specific 32 bit floating point" ;
                 skos:prefLabel "MIPS specific 32 bit floating point" .


###  http://purl.allotrope.org/ontologies/hdf5/1.8#H5T_MIPS_F64
hdf:H5T_MIPS_F64 rdf:type owl:NamedIndividual ,
                          hdf:FloatDatatype ;
                 hdf:order hdf:H5T_ORDER_BE ;
                 rdfs:label "MIPS specific 64 bit floating point" ;
                 skos:prefLabel "MIPS specific 64 bit floating point" .


###  http://purl.allotrope.org/ontologies/hdf5/1.8#H5T_MIPS_I16
hdf:H5T_MIPS_I16 rdf:type owl:NamedIndividual ,
                          hdf:IntegerDatatype ;
                 hdf:order hdf:H5T_ORDER_BE ;
                 hdf:sign hdf:H5T_SGN_2 ;
                 rdfs:label "MIPS specific 8 bit signed integer" ;
                 skos:prefLabel "MIPS specific 8 bit signed integer" .


###  http://purl.allotrope.org/ontologies/hdf5/1.8#H5T_MIPS_I32
hdf:H5T_MIPS_I32 rdf:type owl:NamedIndividual ,
                          hdf:IntegerDatatype ;
                 hdf:order hdf:H5T_ORDER_BE ;
                 hdf:sign hdf:H5T_SGN_2 ;
                 rdfs:label "MIPS specific 8 bit signed integer" ;
                 skos:prefLabel "MIPS specific 8 bit signed integer" .


###  http://purl.allotrope.org/ontologies/hdf5/1.8#H5T_MIPS_I64
hdf:H5T_MIPS_I64 rdf:type owl:NamedIndividual ,
                          hdf:IntegerDatatype ;
                 hdf:order hdf:H5T_ORDER_BE ;
                 hdf:sign hdf:H5T_SGN_2 ;
                 rdfs:label "MIPS specific 8 bit signed integer" ;
                 skos:prefLabel "MIPS specific 8 bit signed integer" .


###  http://purl.allotrope.org/ontologies/hdf5/1.8#H5T_MIPS_I8
hdf:H5T_MIPS_I8 rdf:type owl:NamedIndividual ,
                         hdf:IntegerDatatype ;
                hdf:order hdf:H5T_ORDER_BE ;
                hdf:sign hdf:H5T_SGN_2 ;
                rdfs:label "MIPS specific 8 bit signed integer" ;
                skos:prefLabel "MIPS specific 8 bit signed integer" .


###  http://purl.allotrope.org/ontologies/hdf5/1.8#H5T_MIPS_U16
hdf:H5T_MIPS_U16 rdf:type owl:NamedIndividual ,
                          hdf:IntegerDatatype ;
                 hdf:order hdf:H5T_ORDER_BE ;
                 hdf:sign hdf:H5T_SGN_NONE ;
                 rdfs:label "MIPS 16 bit unsigned integer" ;
                 skos:prefLabel "MIPS 16 bit unsigned integer" .


###  http://purl.allotrope.org/ontologies/hdf5/1.8#H5T_MIPS_U32
hdf:H5T_MIPS_U32 rdf:type owl:NamedIndividual ,
                          hdf:IntegerDatatype ;
                 hdf:order hdf:H5T_ORDER_BE ;
                 hdf:sign hdf:H5T_SGN_NONE ;
                 rdfs:label "MIPS 32 bit unsigned integer" ;
                 skos:prefLabel "MIPS 32 bit unsigned integer" .


###  http://purl.allotrope.org/ontologies/hdf5/1.8#H5T_MIPS_U64
hdf:H5T_MIPS_U64 rdf:type owl:NamedIndividual ,
                          hdf:IntegerDatatype ;
                 hdf:order hdf:H5T_ORDER_BE ;
                 hdf:sign hdf:H5T_SGN_NONE ;
                 rdfs:label "MIPS 64 bit unsigned integer" ;
                 skos:prefLabel "MIPS 64 bit unsigned integer" .


###  http://purl.allotrope.org/ontologies/hdf5/1.8#H5T_MIPS_U8
hdf:H5T_MIPS_U8 rdf:type owl:NamedIndividual ,
                         hdf:IntegerDatatype ;
                hdf:order hdf:H5T_ORDER_BE ;
                hdf:sign hdf:H5T_SGN_NONE ;
                rdfs:label "MIPS 8 bit unsigned integer" ;
                skos:prefLabel "MIPS 8 bit unsigned integer" .


###  http://purl.allotrope.org/ontologies/hdf5/1.8#H5T_NATIVE_CHAR
hdf:H5T_NATIVE_CHAR rdf:type owl:NamedIndividual ,
                             hdf:IntegerDatatype ;
                    rdfs:label "native signed char" ;
                    skos:prefLabel "native signed char" .


###  http://purl.allotrope.org/ontologies/hdf5/1.8#H5T_NATIVE_DOUBLE
hdf:H5T_NATIVE_DOUBLE rdf:type owl:NamedIndividual ,
                               hdf:FloatDatatype ;
                      rdfs:label "native double" ;
                      skos:prefLabel "native double" .


###  http://purl.allotrope.org/ontologies/hdf5/1.8#H5T_NATIVE_FLOAT
hdf:H5T_NATIVE_FLOAT rdf:type owl:NamedIndividual ,
                              hdf:FloatDatatype ;
                     rdfs:label "native float" ;
                     skos:prefLabel "native float" .


###  http://purl.allotrope.org/ontologies/hdf5/1.8#H5T_NATIVE_INT
hdf:H5T_NATIVE_INT rdf:type owl:NamedIndividual ,
                            hdf:IntegerDatatype ;
                   rdfs:label "native signed int" ;
                   skos:prefLabel "native signed int" .


###  http://purl.allotrope.org/ontologies/hdf5/1.8#H5T_NATIVE_LDOUBLE
hdf:H5T_NATIVE_LDOUBLE rdf:type owl:NamedIndividual ,
                                hdf:FloatDatatype ;
                       rdfs:label "native long double" ;
                       skos:prefLabel "native long double" .


###  http://purl.allotrope.org/ontologies/hdf5/1.8#H5T_NATIVE_LLONG
hdf:H5T_NATIVE_LLONG rdf:type owl:NamedIndividual ,
                              hdf:IntegerDatatype ;
                     rdfs:label "native signed long long" ;
                     skos:prefLabel "native signed long long" .


###  http://purl.allotrope.org/ontologies/hdf5/1.8#H5T_NATIVE_LONG
hdf:H5T_NATIVE_LONG rdf:type owl:NamedIndividual ,
                             hdf:IntegerDatatype ;
                    rdfs:label "native signed long" ;
                    skos:prefLabel "native signed long" .


###  http://purl.allotrope.org/ontologies/hdf5/1.8#H5T_NATIVE_SHORT
hdf:H5T_NATIVE_SHORT rdf:type owl:NamedIndividual ,
                              hdf:IntegerDatatype ;
                     rdfs:label "native signed short" ;
                     skos:prefLabel "native signed short" .


###  http://purl.allotrope.org/ontologies/hdf5/1.8#H5T_NATIVE_UCHAR
hdf:H5T_NATIVE_UCHAR rdf:type owl:NamedIndividual ,
                              hdf:IntegerDatatype ;
                     rdfs:label "native unsigned char" ;
                     skos:prefLabel "native unsigned char" .


###  http://purl.allotrope.org/ontologies/hdf5/1.8#H5T_NATIVE_UINT
hdf:H5T_NATIVE_UINT rdf:type owl:NamedIndividual ,
                             hdf:IntegerDatatype ;
                    rdfs:label "native unsigned int" ;
                    skos:prefLabel "native unsigned int" .


###  http://purl.allotrope.org/ontologies/hdf5/1.8#H5T_NATIVE_ULLONG
hdf:H5T_NATIVE_ULLONG rdf:type owl:NamedIndividual ,
                               hdf:IntegerDatatype ;
                      rdfs:label "native unsigned long long" ;
                      skos:prefLabel "native unsigned long long" .


###  http://purl.allotrope.org/ontologies/hdf5/1.8#H5T_NATIVE_ULONG
hdf:H5T_NATIVE_ULONG rdf:type owl:NamedIndividual ,
                              hdf:IntegerDatatype ;
                     rdfs:label "native unsigned long" ;
                     skos:prefLabel "native unsigned long" .


###  http://purl.allotrope.org/ontologies/hdf5/1.8#H5T_NATIVE_USHORT
hdf:H5T_NATIVE_USHORT rdf:type owl:NamedIndividual ,
                               hdf:IntegerDatatype ;
                      rdfs:label "native unsigned short" ;
                      skos:prefLabel "native unsigned short" .


###  http://purl.allotrope.org/ontologies/hdf5/1.8#H5T_NORM_IMPLIED
hdf:H5T_NORM_IMPLIED rdf:type owl:NamedIndividual ,
                              hdf:FloatingPointNormalization ;
                     rdfs:comment "MSB of mantissa isn't stored, always 1. [Allotrope]" ;
                     rdfs:label "implied" ;
                     skos:definition "MSB of mantissa isn't stored, always 1. [Allotrope]" ;
                     skos:prefLabel "implied" .


###  http://purl.allotrope.org/ontologies/hdf5/1.8#H5T_NORM_MSBSET
hdf:H5T_NORM_MSBSET rdf:type owl:NamedIndividual ,
                             hdf:FloatingPointNormalization ;
                    rdfs:comment "MSB of mantissa is always 1. [Allotrope]" ;
                    rdfs:label "msb set" ;
                    skos:definition "MSB of mantissa is always 1. [Allotrope]" ;
                    skos:prefLabel "msb set" .


###  http://purl.allotrope.org/ontologies/hdf5/1.8#H5T_NORM_NONE
hdf:H5T_NORM_NONE rdf:type owl:NamedIndividual ,
                           hdf:FloatingPointNormalization ;
                  rdfs:comment "Not normalized. [Allotrope]" ;
                  rdfs:label "none" ;
                  skos:definition "Not normalized. [Allotrope]" ;
                  skos:prefLabel "none" .


###  http://purl.allotrope.org/ontologies/hdf5/1.8#H5T_OPAQUE
hdf:H5T_OPAQUE rdf:type owl:NamedIndividual ,
                        hdf:TypeClass ;
               rdfs:label "opaque" ;
               skos:prefLabel "opaque" .


###  http://purl.allotrope.org/ontologies/hdf5/1.8#H5T_ORDER_BE
hdf:H5T_ORDER_BE rdf:type owl:NamedIndividual ,
                          hdf:Order ;
                 rdfs:label "big endian" ;
                 skos:prefLabel "big endian" .


###  http://purl.allotrope.org/ontologies/hdf5/1.8#H5T_ORDER_LE
hdf:H5T_ORDER_LE rdf:type owl:NamedIndividual ,
                          hdf:Order ;
                 rdfs:label "little endian" ;
                 skos:prefLabel "little endian" .


###  http://purl.allotrope.org/ontologies/hdf5/1.8#H5T_ORDER_MIXED
hdf:H5T_ORDER_MIXED rdf:type owl:NamedIndividual ,
                             hdf:Order ;
                    rdfs:label "mixed member order" ;
                    skos:prefLabel "mixed member order" .


###  http://purl.allotrope.org/ontologies/hdf5/1.8#H5T_ORDER_VAX
hdf:H5T_ORDER_VAX rdf:type owl:NamedIndividual ,
                           hdf:Order ;
                  rdfs:label "VAX mixed endian" ;
                  skos:prefLabel "VAX mixed endian" .


###  http://purl.allotrope.org/ontologies/hdf5/1.8#H5T_PAD_BACKGROUND
hdf:H5T_PAD_BACKGROUND rdf:type owl:NamedIndividual ,
                                hdf:Padding ;
                       rdfs:label "background value" ;
                       skos:prefLabel "background value" .


###  http://purl.allotrope.org/ontologies/hdf5/1.8#H5T_PAD_ONE
hdf:H5T_PAD_ONE rdf:type owl:NamedIndividual ,
                         hdf:Padding ;
                rdfs:label "pad one" ;
                skos:prefLabel "pad one" .


###  http://purl.allotrope.org/ontologies/hdf5/1.8#H5T_PAD_ZERO
hdf:H5T_PAD_ZERO rdf:type owl:NamedIndividual ,
                          hdf:Padding ;
                 rdfs:label "pad zero" ;
                 skos:prefLabel "pad zero" .


###  http://purl.allotrope.org/ontologies/hdf5/1.8#H5T_REFERENCE
hdf:H5T_REFERENCE rdf:type owl:NamedIndividual ,
                           hdf:TypeClass ;
                  rdfs:label "reference" ;
                  skos:prefLabel "reference" .


###  http://purl.allotrope.org/ontologies/hdf5/1.8#H5T_SGN_2
hdf:H5T_SGN_2 rdf:type owl:NamedIndividual ,
                       hdf:Sign ;
              rdfs:label "two's complement" ;
              skos:prefLabel "two's complement" .


###  http://purl.allotrope.org/ontologies/hdf5/1.8#H5T_SGN_NONE
hdf:H5T_SGN_NONE rdf:type owl:NamedIndividual ,
                          hdf:Sign ;
                 rdfs:label "unsigned" ;
                 skos:prefLabel "unsigned" .


###  http://purl.allotrope.org/ontologies/hdf5/1.8#H5T_STD_B16BE
hdf:H5T_STD_B16BE rdf:type owl:NamedIndividual ,
                           hdf:BitfieldDatatype ;
                  hdf:order hdf:H5T_ORDER_BE ;
                  rdfs:label "standard 16 bit bitfield big endian" ;
                  skos:prefLabel "standard 16 bit bitfield big endian" .


###  http://purl.allotrope.org/ontologies/hdf5/1.8#H5T_STD_B16LE
hdf:H5T_STD_B16LE rdf:type owl:NamedIndividual ,
                           hdf:BitfieldDatatype ;
                  hdf:order hdf:H5T_ORDER_LE ;
                  rdfs:label "standard 16 bit bitfield little endian" ;
                  skos:prefLabel "standard 16 bit bitfield little endian" .


###  http://purl.allotrope.org/ontologies/hdf5/1.8#H5T_STD_B32BE
hdf:H5T_STD_B32BE rdf:type owl:NamedIndividual ,
                           hdf:BitfieldDatatype ;
                  hdf:order hdf:H5T_ORDER_BE ;
                  rdfs:label "standard 32 bit bitfield big endian" ;
                  skos:prefLabel "standard 32 bit bitfield big endian" .


###  http://purl.allotrope.org/ontologies/hdf5/1.8#H5T_STD_B32LE
hdf:H5T_STD_B32LE rdf:type owl:NamedIndividual ,
                           hdf:BitfieldDatatype ;
                  hdf:order hdf:H5T_ORDER_LE ;
                  rdfs:label "standard 32 bit bitfield little endian" ;
                  skos:prefLabel "standard 32 bit bitfield little endian" .


###  http://purl.allotrope.org/ontologies/hdf5/1.8#H5T_STD_B64BE
hdf:H5T_STD_B64BE rdf:type owl:NamedIndividual ,
                           hdf:BitfieldDatatype ;
                  hdf:order hdf:H5T_ORDER_BE ;
                  rdfs:label "standard 64 bit bitfield big endian" ;
                  skos:prefLabel "standard 64 bit bitfield big endian" .


###  http://purl.allotrope.org/ontologies/hdf5/1.8#H5T_STD_B64LE
hdf:H5T_STD_B64LE rdf:type owl:NamedIndividual ,
                           hdf:BitfieldDatatype ;
                  hdf:order hdf:H5T_ORDER_LE ;
                  rdfs:label "standard 64 bit bitfield little endian" ;
                  skos:prefLabel "standard 64 bit bitfield little endian" .


###  http://purl.allotrope.org/ontologies/hdf5/1.8#H5T_STD_B8BE
hdf:H5T_STD_B8BE rdf:type owl:NamedIndividual ,
                          hdf:BitfieldDatatype ;
                 hdf:order hdf:H5T_ORDER_BE ;
                 rdfs:label "standard 8 bit bitfield big endian" ;
                 skos:prefLabel "standard 8 bit bitfield big endian" .


###  http://purl.allotrope.org/ontologies/hdf5/1.8#H5T_STD_B8LE
hdf:H5T_STD_B8LE rdf:type owl:NamedIndividual ,
                          hdf:BitfieldDatatype ;
                 hdf:order hdf:H5T_ORDER_LE ;
                 rdfs:label "standard 8 bit bitfield little endian" ;
                 skos:prefLabel "standard 8 bit bitfield little endian" .


###  http://purl.allotrope.org/ontologies/hdf5/1.8#H5T_STD_I16BE
hdf:H5T_STD_I16BE rdf:type owl:NamedIndividual ,
                           hdf:IntegerDatatype ;
                  hdf:order hdf:H5T_ORDER_BE ;
                  hdf:sign hdf:H5T_SGN_2 ;
                  rdfs:label "standard 16 bit signed integer big endian" ;
                  skos:prefLabel "standard 16 bit signed integer big endian" .


###  http://purl.allotrope.org/ontologies/hdf5/1.8#H5T_STD_I16LE
hdf:H5T_STD_I16LE rdf:type owl:NamedIndividual ,
                           hdf:IntegerDatatype ;
                  hdf:order hdf:H5T_ORDER_LE ;
                  hdf:sign hdf:H5T_SGN_2 ;
                  rdfs:label "standard 16 bit signed integer little endian" ;
                  skos:prefLabel "standard 16 bit signed integer little endian" .


###  http://purl.allotrope.org/ontologies/hdf5/1.8#H5T_STD_I32BE
hdf:H5T_STD_I32BE rdf:type owl:NamedIndividual ,
                           hdf:IntegerDatatype ;
                  hdf:order hdf:H5T_ORDER_BE ;
                  hdf:sign hdf:H5T_SGN_2 ;
                  rdfs:label "standard 32 bit signed integer big endian" ;
                  skos:prefLabel "standard 32 bit signed integer big endian" .


###  http://purl.allotrope.org/ontologies/hdf5/1.8#H5T_STD_I32LE
hdf:H5T_STD_I32LE rdf:type owl:NamedIndividual ,
                           hdf:IntegerDatatype ;
                  hdf:order hdf:H5T_ORDER_LE ;
                  hdf:sign hdf:H5T_SGN_2 ;
                  rdfs:label "standard 32 bit signed integer little endian" ;
                  skos:prefLabel "standard 32 bit signed integer little endian" .


###  http://purl.allotrope.org/ontologies/hdf5/1.8#H5T_STD_I64BE
hdf:H5T_STD_I64BE rdf:type owl:NamedIndividual ,
                           hdf:IntegerDatatype ;
                  hdf:order hdf:H5T_ORDER_BE ;
                  hdf:sign hdf:H5T_SGN_2 ;
                  rdfs:label "standard 64 bit signed integer big endian" ;
                  skos:prefLabel "standard 64 bit signed integer big endian" .


###  http://purl.allotrope.org/ontologies/hdf5/1.8#H5T_STD_I64LE
hdf:H5T_STD_I64LE rdf:type owl:NamedIndividual ,
                           hdf:IntegerDatatype ;
                  hdf:order hdf:H5T_ORDER_LE ;
                  hdf:sign hdf:H5T_SGN_2 ;
                  rdfs:label "standard 64 bit signed integer little endian" ;
                  skos:prefLabel "standard 64 bit signed integer little endian" .


###  http://purl.allotrope.org/ontologies/hdf5/1.8#H5T_STD_I8BE
hdf:H5T_STD_I8BE rdf:type owl:NamedIndividual ,
                          hdf:IntegerDatatype ;
                 hdf:order hdf:H5T_ORDER_BE ;
                 hdf:sign hdf:H5T_SGN_2 ;
                 rdfs:label "standard 8 bit signed integer big endian" ;
                 skos:prefLabel "standard 8 bit signed integer big endian" .


###  http://purl.allotrope.org/ontologies/hdf5/1.8#H5T_STD_I8LE
hdf:H5T_STD_I8LE rdf:type owl:NamedIndividual ,
                          hdf:IntegerDatatype ;
                 hdf:order hdf:H5T_ORDER_LE ;
                 hdf:sign hdf:H5T_SGN_2 ;
                 rdfs:label "standard 8 bit signed integer little endian" ;
                 skos:prefLabel "standard 8 bit signed integer little endian" .


###  http://purl.allotrope.org/ontologies/hdf5/1.8#H5T_STD_U16BE
hdf:H5T_STD_U16BE rdf:type owl:NamedIndividual ,
                           hdf:IntegerDatatype ;
                  hdf:order hdf:H5T_ORDER_BE ;
                  hdf:sign hdf:H5T_SGN_NONE ;
                  rdfs:label "standard 16 bit unsigned integer big endian" ;
                  skos:prefLabel "standard 16 bit unsigned integer big endian" .


###  http://purl.allotrope.org/ontologies/hdf5/1.8#H5T_STD_U16LE
hdf:H5T_STD_U16LE rdf:type owl:NamedIndividual ,
                           hdf:IntegerDatatype ;
                  hdf:order hdf:H5T_ORDER_LE ;
                  hdf:sign hdf:H5T_SGN_NONE ;
                  rdfs:label "standard 16 bit unsigned integer little endian" ;
                  skos:prefLabel "standard 16 bit unsigned integer little endian" .


###  http://purl.allotrope.org/ontologies/hdf5/1.8#H5T_STD_U32BE
hdf:H5T_STD_U32BE rdf:type owl:NamedIndividual ,
                           hdf:IntegerDatatype ;
                  hdf:order hdf:H5T_ORDER_BE ;
                  hdf:sign hdf:H5T_SGN_NONE ;
                  rdfs:label "standard 32 bit unsigned integer big endian" ;
                  skos:prefLabel "standard 32 bit unsigned integer big endian" .


###  http://purl.allotrope.org/ontologies/hdf5/1.8#H5T_STD_U32LE
hdf:H5T_STD_U32LE rdf:type owl:NamedIndividual ,
                           hdf:IntegerDatatype ;
                  hdf:order hdf:H5T_ORDER_LE ;
                  hdf:sign hdf:H5T_SGN_NONE ;
                  rdfs:label "standard 32 bit unsigned integer little endian" ;
                  skos:prefLabel "standard 32 bit unsigned integer little endian" .


###  http://purl.allotrope.org/ontologies/hdf5/1.8#H5T_STD_U64BE
hdf:H5T_STD_U64BE rdf:type owl:NamedIndividual ,
                           hdf:IntegerDatatype ;
                  hdf:order hdf:H5T_ORDER_BE ;
                  hdf:sign hdf:H5T_SGN_NONE ;
                  rdfs:label "standard 64 bit unsigned integer big endian" ;
                  skos:prefLabel "standard 64 bit unsigned integer big endian" .


###  http://purl.allotrope.org/ontologies/hdf5/1.8#H5T_STD_U64LE
hdf:H5T_STD_U64LE rdf:type owl:NamedIndividual ,
                           hdf:IntegerDatatype ;
                  hdf:order hdf:H5T_ORDER_LE ;
                  hdf:sign hdf:H5T_SGN_NONE ;
                  rdfs:label "standard 64 bit unsigned integer little endian" ;
                  skos:prefLabel "standard 64 bit unsigned integer little endian" .


###  http://purl.allotrope.org/ontologies/hdf5/1.8#H5T_STD_U8BE
hdf:H5T_STD_U8BE rdf:type owl:NamedIndividual ,
                          hdf:IntegerDatatype ;
                 hdf:order hdf:H5T_ORDER_BE ;
                 hdf:sign hdf:H5T_SGN_NONE ;
                 rdfs:label "standard 8 bit unsigned integer big endian" ;
                 skos:prefLabel "standard 8 bit unsigned integer big endian" .


###  http://purl.allotrope.org/ontologies/hdf5/1.8#H5T_STD_U8LE
hdf:H5T_STD_U8LE rdf:type owl:NamedIndividual ,
                          hdf:IntegerDatatype ;
                 hdf:order hdf:H5T_ORDER_LE ;
                 hdf:sign hdf:H5T_SGN_NONE ;
                 rdfs:label "standard 8 bit unsigned integer little endian" ;
                 skos:prefLabel "standard 8 bit unsigned integer little endian" .


###  http://purl.allotrope.org/ontologies/hdf5/1.8#H5T_STRING
hdf:H5T_STRING rdf:type owl:NamedIndividual ,
                        hdf:TypeClass ;
               rdfs:label "string" ;
               skos:prefLabel "string" .


###  http://purl.allotrope.org/ontologies/hdf5/1.8#H5T_STR_NULLPAD
hdf:H5T_STR_NULLPAD rdf:type owl:NamedIndividual ,
                             hdf:StringPadding ;
                    rdfs:label "pad with zeros" ;
                    skos:prefLabel "pad with zeros" .


###  http://purl.allotrope.org/ontologies/hdf5/1.8#H5T_STR_NULLTERM
hdf:H5T_STR_NULLTERM rdf:type owl:NamedIndividual ,
                              hdf:StringPadding ;
                     rdfs:comment "Null terminate as C does. [Allotrope]" ;
                     rdfs:label "null terminate" ;
                     skos:definition "Null terminate as C does. [Allotrope]" ;
                     skos:prefLabel "null terminate" .


###  http://purl.allotrope.org/ontologies/hdf5/1.8#H5T_STR_SPACEPAD
hdf:H5T_STR_SPACEPAD rdf:type owl:NamedIndividual ,
                              hdf:StringPadding ;
                     rdfs:comment "Pad with spaces as FORTRAN does. [Allotrope]" ;
                     rdfs:label "pad with spaces" ;
                     skos:definition "Pad with spaces as FORTRAN does. [Allotrope]" ;
                     skos:prefLabel "pad with spaces" .


###  http://purl.allotrope.org/ontologies/hdf5/1.8#H5T_TIME
hdf:H5T_TIME rdf:type owl:NamedIndividual ,
                      hdf:TimeDatatype ,
                      hdf:TypeClass ;
             rdfs:comment "Not yet implemented. [Allotrope]" ;
             rdfs:label "time" ;
             skos:note "Not yet implemented. [Allotrope]" ;
             skos:prefLabel "time" .


###  http://purl.allotrope.org/ontologies/hdf5/1.8#H5T_VAX_F32
hdf:H5T_VAX_F32 rdf:type owl:NamedIndividual ,
                         hdf:FloatDatatype ;
                hdf:order hdf:H5T_ORDER_VAX ;
                rdfs:label "OpenVMS specific 64 bit floating point" ;
                skos:prefLabel "OpenVMS specific 64 bit floating point" .


###  http://purl.allotrope.org/ontologies/hdf5/1.8#H5T_VAX_F64
hdf:H5T_VAX_F64 rdf:type owl:NamedIndividual ,
                         hdf:FloatDatatype ;
                hdf:order hdf:H5T_ORDER_VAX ;
                rdfs:label "OpenVMS specific 64 bit floating point" ;
                skos:prefLabel "OpenVMS specific 64 bit floating point" .


###  http://purl.allotrope.org/ontologies/hdf5/1.8#H5T_VLEN
hdf:H5T_VLEN rdf:type owl:NamedIndividual ,
                      hdf:TypeClass ;
             rdfs:label "variable length" ;
             skos:prefLabel "variable length" .


###  http://purl.allotrope.org/ontologies/hdf5/1.8#H5Z_DISABLE_EDC
hdf:H5Z_DISABLE_EDC rdf:type owl:NamedIndividual ,
                             hdf:ErrorDetectionCheck ;
                    rdfs:label "disable error detection check" ;
                    skos:prefLabel "disable error detection check" .


###  http://purl.allotrope.org/ontologies/hdf5/1.8#H5Z_ENABLE_EDC
hdf:H5Z_ENABLE_EDC rdf:type owl:NamedIndividual ,
                            hdf:ErrorDetectionCheck ;
                   rdfs:label "enable error detection check" ;
                   skos:prefLabel "enable error detection check" .


###  http://purl.allotrope.org/ontologies/hdf5/1.8#H5Z_SO_FLOAT_DSCALE
hdf:H5Z_SO_FLOAT_DSCALE rdf:type owl:NamedIndividual ,
                                 hdf:ScaleType ;
                        rdfs:comment "Floating-point type, using variable MinBits method. The scaleFactor denotes the decimal scale factor for D-scaling and can be positive, negative or zero. This is the current implementation of the library. [HDF]" ;
                        rdfs:label "floating-point dscale" ;
                        skos:definition "Floating-point type, using variable MinBits method. The scaleFactor denotes the decimal scale factor for D-scaling and can be positive, negative or zero. This is the current implementation of the library. [HDF]" ;
                        skos:prefLabel "floating-point dscale" .


###  http://purl.allotrope.org/ontologies/hdf5/1.8#H5Z_SO_FLOAT_ESCALE
hdf:H5Z_SO_FLOAT_ESCALE rdf:type owl:NamedIndividual ,
                                 hdf:ScaleType ;
                        rdfs:comment "Floating-point type, using fixed MinBits method. The scaleFactor denotes MinBits for E-scaling and must be a positive integer. This is not currently implemented by the library. [HDF]" ;
                        rdfs:label "floating-point escale" ;
                        skos:definition "Floating-point type, using fixed MinBits method. The scaleFactor denotes MinBits for E-scaling and must be a positive integer. This is not currently implemented by the library. [HDF]" ;
                        skos:prefLabel "floating-point escale" .


###  http://purl.allotrope.org/ontologies/hdf5/1.8#H5Z_SO_INT
hdf:H5Z_SO_INT rdf:type owl:NamedIndividual ,
                        hdf:ScaleType ;
               rdfs:comment "Integer type. The scaleFactor denotes MinBits and it should be a positive integer or H5Z_SO_INT_MINBITS_DEFAULT. If it is less than 0, the library will reset it to 0 since it is not implemented. [HDF]" ;
               rdfs:label "integer" ;
               skos:definition "Integer type. The scaleFactor denotes MinBits and it should be a positive integer or H5Z_SO_INT_MINBITS_DEFAULT. If it is less than 0, the library will reset it to 0 since it is not implemented. [HDF]" ;
               skos:prefLabel "integer" .


###  http://purl.allotrope.org/ontologies/hdf5/1.8#H5_SZIP_EC_OPTION_MASK
hdf:H5_SZIP_EC_OPTION_MASK rdf:type owl:NamedIndividual ,
                                    hdf:SZipCoding ;
                           rdfs:label "szip entropy coding" ;
                           skos:prefLabel "szip entropy coding" .


###  http://purl.allotrope.org/ontologies/hdf5/1.8#H5_SZIP_NN_OPTION_MASK
hdf:H5_SZIP_NN_OPTION_MASK rdf:type owl:NamedIndividual ,
                                    hdf:SZipCoding ;
                           rdfs:label "szip nearest neighbor coding" ;
                           skos:prefLabel "szip nearest neighbor coding" .


###  http://purl.allotrope.org/ontologies/hdf5/1.8#scalarDataspace
hdf:scalarDataspace rdf:type owl:NamedIndividual ,
                             hdf:ScalarDataspace ;
                    rdfs:label "scalar dataspace" ;
                    skos:prefLabel "scalar dataspace" .


###  http://purl.allotrope.org/voc/attribution
<http://purl.allotrope.org/voc/attribution> rdf:type owl:NamedIndividual ;
                                            dct:description """
These taxonomies contain material or may constitute derivative works of material which may be subject to copyright by one of the following organizations.  By using these taxonomies, you agree to the following terms and conditions applicable to its contents:
******************************************************************************
Attribution Notice for National Center for Biomedical Ontology materials.

This work contains material from the Cell Ontology and Clinical Measurement Ontology, available here: http://bioportal.bioontology.org/.
******************************************************************************
Attribution Notice for ChEBI
This work contains material from the European Bioinformatics Institute’s ChEBI database.
******************************************************************************
Attribution Notice for Quantities Units Dimensions Data Types (http://www.qudt.org/)
This work contains content from www.qudt.org and is used pursuant to a Creative Commons License available here: http://creativecommons.org/licenses/by-sa/3.0/us/legalcode. The original work may have been modified.
******************************************************************************
Copyright and Attribution Notice for Dublin Core Metadata Initiative Document
This work contains material from the following DCMI document used pursuant to a creative commons license available here: https://creativecommons.org/licenses/by/4.0/legalcode. This material may have been modified or changed.
Timestamped URL:          http://dublincore.org/documents/2012/06/14/dcmi-terms/
Date Issued:                       2012-06-14
Document Status:            This is a DCMI Recommendation.
Copyright © 1995-2015 DCMI. All Rights Reserved. DCMI liability, trademark/service mark, document use and software licensing rules apply.
******************************************************************************

""" ;
                                            dct:title "Derivative works attribution" .


###  http://purl.allotrope.org/voc/copyright
<http://purl.allotrope.org/voc/copyright> rdf:type owl:NamedIndividual ;
                                          dct:description "Copyright © 2015-2024 Allotrope Foundation" ;
                                          dct:rightsHolder <http://www.allotrope.org> ;
                                          dct:title "Copyright © 2015-2024 Allotrope Foundation" .


###  http://purl.allotrope.org/voc/creative-commons-attribution-license
<http://purl.allotrope.org/voc/creative-commons-attribution-license> rdf:type owl:NamedIndividual ;
                                                                     dct:description """This work is licensed under a Creative Commons Attribution 4.0 International License http://creativecommons.org/licenses/by/4.0/.

THESE MATERIALS ARE PROVIDED \"AS IS\" AND ALLOTROPE EXPRESSLY DISCLAIMS ALL WARRANTIES, EXPRESS, IMPLIED OR STATUTORY, INCLUDING, WITHOUT LIMITATION, THE WARRANTIES OF NON-INFRINGEMENT, TITLE, MERCHANTABILITY AND FITNESS FOR A PARTICULAR PURPOSE.

Copyright © 2015-2024 Allotrope Foundation
""" ;
                                                                     dct:rightsHolder <http://www.allotrope.org> ;
                                                                     dct:title "Creative Commons Attribution 4.0 International Public License" .


###  http://purl.allotrope.org/voc/hdf-copyright
<http://purl.allotrope.org/voc/hdf-copyright> rdf:type owl:NamedIndividual ,
                                                       dct:RightsStatement ;
                                              dct:description """
HDF5 (Hierarchical Data Format 5) Software Library and Utilities
Copyright © 2006-2018, The HDF Group.

NCSA HDF5 (Hierarchical Data Format 5) Software Library and Utilities
Copyright © 1998-2006, The Board of Trustees of the University of Illinois.

All rights reserved.
""" .


###  http://purl.allotrope.org/voc/hdf-license
<http://purl.allotrope.org/voc/hdf-license> rdf:type owl:NamedIndividual ,
                                                     dct:LicenseDocument ;
                                            dct:description """
Copyright Notice and License Terms for HDF5 (Hierarchical Data Format 5) Software Library and Utilities
HDF5 (Hierarchical Data Format 5) Software Library and Utilities Copyright © 2006-2018, The HDF Group.

NCSA HDF5 (Hierarchical Data Format 5) Software Library and Utilities Copyright © 1998-2006, The Board of Trustees of the University of Illinois.

All rights reserved.

Redistribution and use in source and binary forms, with or without modification, are permitted for any purpose (including commercial purposes) provided that the following conditions are met:

  1. Redistributions of source code must retain the above copyright notice, this list of conditions, and the following disclaimer.
  2. Redistributions in binary form must reproduce the above copyright notice, this list of conditions, and the following disclaimer in the documentation and/or materials provided with the distribution.
  3. Neither the name of The HDF Group, the name of the University, nor the name of any Contributor may be used to endorse or promote products derived from this software without specific prior written permission from The HDF Group, the University, or the Contributor, respectively.

DISCLAIMER:  THIS SOFTWARE IS PROVIDED BY THE HDF GROUP AND THE CONTRIBUTORS \"AS IS\" WITH NO WARRANTY OF ANY KIND, EITHER EXPRESSED OR IMPLIED. IN NO EVENT SHALL THE HDF GROUP OR THE CONTRIBUTORS BE LIABLE FOR ANY DAMAGES SUFFERED BY THE USERS ARISING OUT OF THE USE OF THIS SOFTWARE, EVEN IF ADVISED OF THE POSSIBILITY OF SUCH DAMAGE.  You are under no obligation whatsoever to provide any bug fixes, patches, or upgrades to the features, functionality or performance of the source code (\"Enhancements\") to anyone; however, if you choose to make your Enhancements available either publicly, or directly to The HDF Group, without imposing a separate written license agreement for such Enhancements, then you hereby grant the following license: a non-exclusive, royalty-free perpetual license to install, use, modify, prepare derivative works, incorporate into other computer software, distribute, and sublicense such enhancements or derivative works thereof, in binary and source code form.""" .


#################################################################
#    General axioms
#################################################################

[ rdf:type owl:AllDisjointClasses ;
  owl:members ( hdf:BitfieldDatatype
                hdf:FloatDatatype
                hdf:IntegerDatatype
                hdf:OpaqueDatatype
                hdf:ReferenceDatatype
                hdf:StringDatatype
                hdf:TimeDatatype
              )
] .


[ rdf:type owl:AllDifferent ;
  owl:distinctMembers ( hdf:H5D_ALLOC_TIME_DEFAULT
                        hdf:H5D_ALLOC_TIME_EARLY
                        hdf:H5D_ALLOC_TIME_INCR
                        hdf:H5D_ALLOC_TIME_LATE
                      )
] .


[ rdf:type owl:AllDifferent ;
  owl:distinctMembers ( hdf:H5D_CHUNKED
                        hdf:H5D_COMPACT
                        hdf:H5D_CONTIGUOUS
                      )
] .


[ rdf:type owl:AllDifferent ;
  owl:distinctMembers ( hdf:H5D_FILL_TIME_ALLOC
                        hdf:H5D_FILL_TIME_IFSET
                        hdf:H5D_FILL_TIME_NEVER
                      )
] .


[ rdf:type owl:AllDifferent ;
  owl:distinctMembers ( hdf:H5D_FILL_VALUE_DEFAULT
                        hdf:H5D_FILL_VALUE_UNDEFINED
                        hdf:H5D_FILL_VALUE_USER_DEFINED
                      )
] .


[ rdf:type owl:AllDifferent ;
  owl:distinctMembers ( hdf:H5FD_MPIO_CHUNK_MULTI_IO
                        hdf:H5FD_MPIO_CHUNK_ONE_IO
                      )
] .


[ rdf:type owl:AllDifferent ;
  owl:distinctMembers ( hdf:H5FD_MPIO_COLLECTIVE
                        hdf:H5FD_MPIO_INDEPENDENT
                      )
] .


[ rdf:type owl:AllDifferent ;
  owl:distinctMembers ( hdf:H5F_ACC_DEFAULT
                        hdf:H5F_ACC_RDONLY
                        hdf:H5F_ACC_RDWR
                      )
] .


[ rdf:type owl:AllDifferent ;
  owl:distinctMembers ( hdf:H5O_SHMESG_ALL_FLAG
                        hdf:H5O_SHMESG_ATTR_FLAG
                        hdf:H5O_SHMESG_DTYPE_FLAG
                        hdf:H5O_SHMESG_FILL_FLAG
                        hdf:H5O_SHMESG_NONE_FLAG
                        hdf:H5O_SHMESG_PLINE_FLAG
                        hdf:H5O_SHMESG_SDSPACE_FLAG
                      )
] .


[ rdf:type owl:AllDifferent ;
  owl:distinctMembers ( hdf:H5T_ALPHA_B16
                        hdf:H5T_ALPHA_B32
                        hdf:H5T_ALPHA_B64
                        hdf:H5T_ALPHA_B8
                        hdf:H5T_ALPHA_F32
                        hdf:H5T_ALPHA_F64
                        hdf:H5T_ALPHA_I16
                        hdf:H5T_ALPHA_I32
                        hdf:H5T_ALPHA_I64
                        hdf:H5T_ALPHA_I8
                        hdf:H5T_ALPHA_U16
                        hdf:H5T_ALPHA_U32
                        hdf:H5T_ALPHA_U64
                        hdf:H5T_ALPHA_U8
                        hdf:H5T_IEEE_F32BE
                        hdf:H5T_IEEE_F32LE
                        hdf:H5T_IEEE_F64BE
                        hdf:H5T_IEEE_F64LE
                        hdf:H5T_INTEL_B16
                        hdf:H5T_INTEL_B32
                        hdf:H5T_INTEL_B64
                        hdf:H5T_INTEL_B8
                        hdf:H5T_INTEL_F32
                        hdf:H5T_INTEL_F64
                        hdf:H5T_INTEL_I16
                        hdf:H5T_INTEL_I32
                        hdf:H5T_INTEL_I64
                        hdf:H5T_INTEL_I8
                        hdf:H5T_INTEL_U16
                        hdf:H5T_INTEL_U32
                        hdf:H5T_INTEL_U64
                        hdf:H5T_INTEL_U8
                        hdf:H5T_MIPS_B16
                        hdf:H5T_MIPS_B32
                        hdf:H5T_MIPS_B64
                        hdf:H5T_MIPS_B8
                        hdf:H5T_MIPS_F32
                        hdf:H5T_MIPS_F64
                        hdf:H5T_MIPS_I16
                        hdf:H5T_MIPS_I32
                        hdf:H5T_MIPS_I64
                        hdf:H5T_MIPS_I8
                        hdf:H5T_MIPS_U16
                        hdf:H5T_MIPS_U32
                        hdf:H5T_MIPS_U64
                        hdf:H5T_MIPS_U8
                        hdf:H5T_NATIVE_CHAR
                        hdf:H5T_NATIVE_DOUBLE
                        hdf:H5T_NATIVE_FLOAT
                        hdf:H5T_NATIVE_INT
                        hdf:H5T_NATIVE_LDOUBLE
                        hdf:H5T_NATIVE_LLONG
                        hdf:H5T_NATIVE_LONG
                        hdf:H5T_NATIVE_SHORT
                        hdf:H5T_NATIVE_UCHAR
                        hdf:H5T_NATIVE_UINT
                        hdf:H5T_NATIVE_ULLONG
                        hdf:H5T_NATIVE_ULONG
                        hdf:H5T_NATIVE_USHORT
                        hdf:H5T_STD_B16BE
                        hdf:H5T_STD_B16LE
                        hdf:H5T_STD_B32BE
                        hdf:H5T_STD_B32LE
                        hdf:H5T_STD_B64BE
                        hdf:H5T_STD_B64LE
                        hdf:H5T_STD_B8BE
                        hdf:H5T_STD_B8LE
                        hdf:H5T_STD_I16BE
                        hdf:H5T_STD_I16LE
                        hdf:H5T_STD_I32BE
                        hdf:H5T_STD_I32LE
                        hdf:H5T_STD_I64BE
                        hdf:H5T_STD_I64LE
                        hdf:H5T_STD_I8BE
                        hdf:H5T_STD_I8LE
                        hdf:H5T_STD_U16BE
                        hdf:H5T_STD_U16LE
                        hdf:H5T_STD_U32BE
                        hdf:H5T_STD_U32LE
                        hdf:H5T_STD_U64BE
                        hdf:H5T_STD_U64LE
                        hdf:H5T_STD_U8BE
                        hdf:H5T_STD_U8LE
                        hdf:H5T_TIME
                      )
] .


[ rdf:type owl:AllDifferent ;
  owl:distinctMembers ( hdf:H5T_NORM_IMPLIED
                        hdf:H5T_NORM_MSBSET
                        hdf:H5T_NORM_NONE
                      )
] .


[ rdf:type owl:AllDifferent ;
  owl:distinctMembers ( hdf:H5T_ORDER_BE
                        hdf:H5T_ORDER_LE
                        hdf:H5T_ORDER_MIXED
                        hdf:H5T_ORDER_VAX
                      )
] .


[ rdf:type owl:AllDifferent ;
  owl:distinctMembers ( hdf:H5T_PAD_BACKGROUND
                        hdf:H5T_PAD_ONE
                        hdf:H5T_PAD_ZERO
                      )
] .


[ rdf:type owl:AllDifferent ;
  owl:distinctMembers ( hdf:H5T_SGN_2
                        hdf:H5T_SGN_NONE
                      )
] .


[ rdf:type owl:AllDifferent ;
  owl:distinctMembers ( hdf:H5T_STR_NULLPAD
                        hdf:H5T_STR_NULLTERM
                        hdf:H5T_STR_SPACEPAD
                      )
] .


[ rdf:type owl:AllDifferent ;
  owl:distinctMembers ( hdf:H5Z_DISABLE_EDC
                        hdf:H5Z_ENABLE_EDC
                      )
] .


[ rdf:type owl:AllDifferent ;
  owl:distinctMembers ( hdf:H5Z_SO_FLOAT_DSCALE
                        hdf:H5Z_SO_FLOAT_ESCALE
                        hdf:H5Z_SO_INT
                      )
] .


[ rdf:type owl:AllDifferent ;
  owl:distinctMembers ( hdf:H5_SZIP_EC_OPTION_MASK
                        hdf:H5_SZIP_NN_OPTION_MASK
                      )
] .


###  Generated by the OWL API (version 5.1.19) https://github.com/owlcs/owlapi/
